Reorg of Dafny Dot sources... ... move all except current dev to a new 'old' directory.

src/dafny/Dot.dfy
@@ -8,33 +8,13 @@
 
 // ### List ###
 datatype list<A> = Nil | Cons(head: A, tail: list<A>);
-function length<A>(lst: list<A>): nat
-  ensures length(lst)==0 ==> lst.Nil?;
-  ensures length(lst)>0 ==> lst.Cons?;
-{
-  match lst
-  case Nil => 0
-  case Cons(head, tail) => 1 + length(tail)
-}
-function nth<A>(n: nat, lst: list<A>): A
-  requires n < length(lst);
-{
-  if (n==0) then lst.head else nth(n-1, lst.tail)
-}
-function slice<A>(i: nat, j: nat, lst: list<A>): list<A>
-  requires 0 <= i <= j <= length(lst);
-  decreases j-i;
-{
-  if (i==j) then Nil
-  else if (i==0) then Cons(lst.head, slice(i, j-1, lst.tail))
-  else slice(i+1, j, lst)
-}
-function snoc<A>(lst: list<A>, x: A): list<A>
-{
-  match lst
-  case Nil => Cons(x, Nil)
-  case Cons(head, tail) => Cons(head, snoc(tail, x))
-}
+
+// ### Pair ###
+datatype pair<A, B> = P(fst: A, snd: B);
+
+// ### Option ###
+datatype option<A> = None | Some(get: A);
+
 function seq2lst<A>(s: seq<A>): list<A>
 {
   if (s == []) then Nil
@@ -46,92 +26,6 @@ function lst2seq<A>(lst: list<A>): seq<A>
   case Nil => []
   case Cons(head, tail) => [head] + lst2seq(tail)
 }
-predicate same_lst_seq<A>(lst: list<A>, s: seq<A>)
-  ensures same_lst_seq(lst, s) ==> length(lst)==|s|;
-{
-  match lst
-  case Nil => s==[]
-  case Cons(head, tail) => |s|>0 && s[0]==head && same_lst_seq(tail, s[1..])
-}
-ghost method lemma_lst2seq_same<A>(lst: list<A>, s: seq<A>)
-  requires lst2seq(lst)==s;
-  ensures same_lst_seq(lst, s);
-{
-}
-ghost method lemma_same_lst_seq_forall<A>(lst: list<A>, s: seq<A>)
-  requires same_lst_seq(lst, s );
-  ensures forall n :: 0 <= n < |s| ==> s[n]==nth(n, lst);
-{
-  match lst {
-  case Nil =>
-  case Cons(head, tail) =>
-    assert s[0]==head;
-    lemma_same_lst_seq_forall(tail, s[1..]);
-  }
-}
-
-// ### Pair ###
-datatype pair<A, B> = P(fst: A, snd: B);
-
-// ### Option ###
-datatype option<A> = None | Some(get: A);
-
-// ### Partial Maps ###
-datatype partial_map<K,V> = Empty | Extend(x: K, v: V, rest: partial_map<K,V>);
-function lookup<K,V>(x: K, m: partial_map<K,V>): option<V>
-  ensures m.Empty? ==> lookup(x, m).None?;
-  ensures m.Empty? ==> !lookup(x, m).Some?;
-  ensures m.Extend? && m.x==x ==> lookup(x, m) == Some(m.v);
-  ensures m.Extend? && m.x!=x ==> lookup(x, m) == lookup(x, m.rest);
-{
-  match m
-  case Empty => None
-  case Extend(x', v, rest) => if x==x' then Some(v) else lookup(x, rest)
-}
-function dom<K,V>(m: partial_map<K,V>): seq<K>
-  ensures forall x :: x in dom(m) ==> lookup(x, m).Some?;
-  ensures m.Extend? ==> dom(m) == [m.x]+dom(m.rest);
-{
-  match m
-  case Empty => []
-  case Extend(x, v, rest) => [x]+dom(rest)
-}
-function prefixes<K,V>(m: partial_map<K,V>): seq<partial_map<K,V>>
-  ensures m in prefixes(m);
-  ensures m.Extend? ==> m.rest in prefixes(m);
-{
-  match m
-  case Empty => [m]
-  case Extend(x, v, rest) => [m]+prefixes(rest)
-}
-predicate prefix_of<K,V>(m: partial_map<K,V>, m_prev: partial_map<K,V>)
-{
-  m==m_prev || (m.Extend? && prefix_of(m.rest, m_prev))
-}
-function build<K,V>(m: partial_map<K,V>, r: partial_map<K,V>): partial_map<K,V>
-  decreases r;
-{
-  match r
-  case Empty => m
-  case Extend(x, v, rest) => build(Extend(x, v, m), rest)
-}
-function map_complement<K,V>(m: partial_map<K,V>, m_prev: partial_map<K,V>, start: partial_map<K,V>): partial_map<K,V>
-  requires prefix_of(m, m_prev);
-  //ensures build(m_prev, map_complement(m, m_prev, Empty))==m;
-  decreases m;
-{
-  if (m==m_prev) then start
-  else map_complement(m.rest, m_prev, Extend(m.x, m.v, start))
-}
-function map_fst<K,A,B>(m: partial_map<K,pair<A,B>>): partial_map<K,A>
-  ensures dom(m)==dom(map_fst(m));
-{
-  match m
-  case Empty => Empty
-  case Extend(x, v, rest) => Extend(x, v.fst, map_fst(rest))
-}
-
-// ### Sequences ###
 function max(s: seq<int>, start: int): int
   ensures max(s, start)>=start;
   ensures forall x :: x in s ==> x<=max(s, start);
@@ -140,445 +34,42 @@ function max(s: seq<int>, start: int): int
   else if (s[0] <= start) then max(s[1..], start)
   else max(s[1..], s[0])
 }
-function rev<A>(s: seq<A>): seq<A>
+function fresh_from(ids: seq<int>): int
+  ensures fresh_from(ids) !in ids;
+  ensures fresh_from(ids)>0;
 {
-  if (|s|==0) then [] else rev(s[1..])+[s[0]]
-}
-
-// ### Lemmas about utilities ###
-ghost method lemma_empty_prefix_of_any<K,V>(m: partial_map<K,V>)
-  ensures prefix_of(m, Empty);
-{
-}
-ghost method lemma_rev_beg__end<A>(s: seq<A>, x: A)
-  ensures rev([x]+s)==rev(s)+[x];
-{
-}
-ghost method lemma_rev<A>(s1: seq<A>, s2: seq<A>)
-  ensures rev(s1+s2)==rev(s2)+rev(s1);
-{
-  if (s1==[]) {
-    assert s1+s2==s2;
-  } else {
-    lemma_rev_beg__end(s1[1..], s1[0]);
-    assert rev([s1[0]]+(s1[1..]+s2))==rev(s1[1..]+s2)+[s1[0]];
-    lemma_rev(s1[1..], s2);
-    assert rev(s1[1..]+s2)+[s1[0]]==rev(s2)+rev(s1[1..])+[s1[0]];
-    lemma_rev_beg__end(s1[1..], s1[0]);
-    assert rev(s1[1..]+s2)+[s1[0]]==rev(s2)+rev(s1);
-    assert rev([s1[0]]+(s1[1..]+s2))==rev(s2)+rev(s1);
-    assert [s1[0]]+(s1[1..]+s2)==([s1[0]]+s1[1..])+s2;
-    assert [s1[0]]+s1[1..]==s1;
-    assert ([s1[0]]+s1[1..])+s2==s1+s2;
-    assert rev([s1[0]]+(s1[1..]+s2))==rev(([s1[0]]+s1[1..])+s2);
-    assert rev([s1[0]]+(s1[1..]+s2))==rev(s1+s2);
-    assert rev(s1+s2)==rev(s2)+rev(s1);
-  }
-}
-ghost method lemma_rev_end__beg<A>(s: seq<A>, x: A)
-  ensures rev(s+[x])==[x]+rev(s);
-{
-  lemma_rev(s, [x]);
-}
-ghost method lemma_rev_rev<A>(s: seq<A>)
-  ensures rev(rev(s))==s;
-{
-  if (|s|==0) {
-
-  } else {
-    lemma_rev_rev(s[1..]);
-    assert rev(rev(s[1..]))==s[1..];
-    lemma_rev_beg__end(s[1..], s[0]);
-    assert rev([s[0]]+s[1..])==rev(s[1..])+[s[0]];
-    lemma_rev_end__beg(rev(s[1..]), s[0]);
-    assert rev(rev(s[1..])+[s[0]])==[s[0]]+rev(rev(s[1..]));
-    assert [s[0]]+rev(rev(s[1..]))==[s[0]]+s[1..];
-    assert [s[0]]+s[1..]==s;
-    assert rev(rev(s))==rev(rev([s[0]]+s[1..]));
-    assert rev(rev([s[0]]+s[1..]))==[s[0]]+rev(rev(s[1..]));
-    assert [s[0]]+rev(rev(s[1..]))==[s[0]]+s[1..];
-    assert rev(rev(s))==s;
-  }
-}
-ghost method lemma_prefix_of__dom<K,V>(m: partial_map<K,V>, m_prev: partial_map<K,V>) returns (s: seq<K>)
-  requires prefix_of(m, m_prev);
-  ensures dom(m)==s+dom(m_prev);
-{
-  if (m==m_prev) {
-    s := [];
-  } else {
-    var s' := lemma_prefix_of__dom(m.rest, m_prev);
-    assert dom(m.rest)==s'+dom(m_prev);
-    s := [m.x] + s';
-    assert dom(m)==[m.x]+dom(m.rest);
-  }
-}
-ghost method lemma_map_complement_extend__dom'<K,V>(m: partial_map<K,V>, m_prev: partial_map<K,V>, start: partial_map<K,V>)
-  requires prefix_of(m, m_prev);
-  ensures dom(map_complement(m, m_prev, start))==dom(map_complement(m, m_prev, Empty))+dom(start);
-{
-}
-ghost method lemma_map_complement_extend__dom<K,V>(m: partial_map<K,V>, m_prev: partial_map<K,V>)
-  requires prefix_of(m, m_prev);
-  ensures m!=m_prev ==> dom(map_complement(m, m_prev, Empty))==dom(map_complement(m.rest, m_prev, Extend(m.x, m.v, Empty)));
-  ensures m!=m_prev ==> dom(map_complement(m, m_prev, Empty))==dom(map_complement(m.rest, m_prev, Empty))+[m.x];
-{
-  if (m!=m_prev) {
-    lemma_map_complement_extend__dom'(m.rest, m_prev, Extend(m.x, m.v, Empty));
-  }
-}
-ghost method lemma_map_complement__dom<K,V>(m: partial_map<K,V>, m_prev: partial_map<K,V>)
-  requires prefix_of(m, m_prev);
-  ensures dom(m)==rev(dom(map_complement(m, m_prev, Empty)))+dom(m_prev);
-{
-  if (m==m_prev) {
-  } else {
-    lemma_map_complement__dom(m.rest, m_prev);
-    assert dom(m.rest)==rev(dom(map_complement(m.rest, m_prev, Empty)))+dom(m_prev);
-    lemma_map_complement_extend__dom(m, m_prev);
-    assert dom(map_complement(m, m_prev, Empty))==dom(map_complement(m.rest, m_prev, Empty))+[m.x];
-    assert rev(dom(map_complement(m, m_prev, Empty)))==rev(dom(map_complement(m.rest, m_prev, Empty))+[m.x]);
-    lemma_rev_end__beg(dom(map_complement(m.rest, m_prev, Empty)), m.x);
-    assert rev(dom(map_complement(m.rest, m_prev, Empty))+[m.x])==[m.x]+rev(dom(map_complement(m.rest, m_prev, Empty)));
-  }
-}
-ghost method lemma_map_complement_prev_empty__dom<K,V>(m: partial_map<K,V>)
-  ensures prefix_of(m, Empty);
-  ensures dom(m)==rev(dom(map_complement(m, Empty, Empty)));
-  ensures rev(dom(m))==dom(map_complement(m, Empty, Empty));
-{
-  lemma_map_complement__dom(m, Empty);
-  assert dom(m)==rev(dom(map_complement(m, Empty, Empty)));
-  assert rev(dom(m))==rev(rev(dom(map_complement(m, Empty, Empty))));
-  lemma_rev_rev(dom(map_complement(m, Empty, Empty)));
-  assert rev(rev(dom(map_complement(m, Empty, Empty))))==dom(map_complement(m, Empty, Empty));
-  assert rev(dom(m))==dom(map_complement(m, Empty, Empty));
-}
-ghost method lemma_build__dom<K,V>(m: partial_map<K,V>, r: partial_map<K,V>)
-  ensures dom(build(m, r)) == rev(dom(r)) + dom(m);
-  decreases r;
-{
-  match r {
-  case Empty =>
-  case Extend(x, v, rest) =>
-    lemma_build__dom(Extend(x, v, m), rest);
-    assert dom(build(Extend(x, v, m), rest)) == rev(dom(rest)) + dom(Extend(x, v, m));
-    assert dom(Extend(x, v, m)) == [x]+dom(m);
-    lemma_rev_beg__end(dom(rest), x);
-    assert rev(dom(rest))+[x]==rev([x]+dom(rest));
-  }
-}
-ghost method lemma_prefix_of_trans<K,V>(m1: partial_map<K,V>, m2: partial_map<K,V>, m3: partial_map<K,V>)
-  requires prefix_of(m3, m2);
-  requires prefix_of(m2, m1);
-  ensures prefix_of(m3, m1);
-{
+  max(ids, 0)+1
 }
 
 // ------
 // Syntax
 // ------
 
-datatype tp = tp_sel_c(pc: tm, Lc: nat) | tp_sel_a(pa: tm, La: nat) | tp_rfn(base_tp: tp, self: nat, decls: list<decl>) | tp_and(and1: tp, and2: tp) | tp_or(or1: tp, or2: tp) | tp_top | tp_bot;
-datatype tm = tm_var(x: nat) | tm_new(y: nat, Tc: tp, init: list<def>, t': tm) | tm_sel(t: tm, l: nat) | tm_msel(o: tm, m: nat, a: tm);
-datatype decl = decl_tp_c(Lc: nat, Sc: tp, Uc: tp) | decl_tp_a(La: nat, Sa: tp, Ua: tp) | decl_tm(l: nat, T: tp) | decl_mt(m: nat, P: tp, R: tp);
+datatype tp = tp_sel(p: tm, L: nat, concrete: bool) | tp_rfn(base_tp: tp, self: nat, decls: list<decl>) | tp_and(and1: tp, and2: tp) | tp_or(or1: tp, or2: tp) | tp_top | tp_bot;
+datatype tm = tm_var(x: nat) | tm_new(y: nat, Tc: tp, init: list<def>, t': tm) | tm_sel(t: tm, l: nat) | tm_msel(o: tm, m: nat, a: tm) | tm_loc(loc: nat);
+datatype decl = decl_tp(L: nat, S: tp, U: tp, concrete: bool) | decl_tm(l: nat, T: tp) | decl_mt(m: nat, P: tp, R: tp);
 datatype def = def_tm(l: nat, t: tm) | def_mt(m: nat, param: nat, body: tm);
-datatype decls = decls_fin(decls: seq<decl>) | decls_bot;
+datatype decls = decls_fin(decls: list<decl>) | decls_bot;
 
 predicate path(t: tm)
 {
-  t.tm_var? || (t.tm_sel? && path(t.t))
+  t.tm_loc? || t.tm_var? || (t.tm_sel? && path(t.t))
 }
 
-predicate concrete(T: tp)
+predicate is_concrete(T: tp)
 {
-  (T.tp_sel_c? && path(T.pc)) ||
-  (T.tp_rfn? && concrete(T.base_tp)) ||
-  (T.tp_and? && concrete(T.and1) && concrete(T.and2)) ||
+  (T.tp_sel? && T.concrete && path(T.p)) ||
+  (T.tp_rfn? && is_concrete(T.base_tp)) ||
+  (T.tp_and? && is_concrete(T.and1) && is_concrete(T.and2)) ||
   T.tp_top?
 }
 
 function decl_label(d: decl): nat
 {
   match d
-  case decl_tp_c(Lc, Sc, Uc) => Lc
-  case decl_tp_a(La, Sa, Ua) => La
+  case decl_tp(L, S, U, concrete) => L
   case decl_tm(l, T) => l
   case decl_mt(m, P, R) => m
-}
-
-// -------------------------
-// Sorting-related functions
-// -------------------------
-
-predicate decl_lt(d1: decl, d2: decl)
-{
-  match d1
-  case decl_tp_c(Lc1, Sc1, Uc1) =>
-    (match d2
-     case decl_tp_c(Lc2, Sc2, Uc2) => Lc1<Lc2
-     case decl_tp_a(La2, Sa2, Ua2) => true
-     case decl_tm(l2, T2) => true
-     case decl_mt(m2, P2, R2) => true)
-  case decl_tp_a(La1, Sa1, Ua1) =>
-    (match d2
-     case decl_tp_c(Lc2, Sc2, Uc2) => false
-     case decl_tp_a(La2, Sa2, Ua2) => La1<La2
-     case decl_tm(l2, T2) => true
-     case decl_mt(m2, P2, R2) => true)
-  case decl_tm(l1, T1) =>
-    (match d2
-     case decl_tp_c(Lc2, Sc2, Uc2) => false
-     case decl_tp_a(La2, Sa2, Ua2) => false
-     case decl_tm(l2, T2) => l1<l2
-     case decl_mt(m2, P2, R2) => true)
-  case decl_mt(m1, P1, R1) =>
-    (match d2
-     case decl_tp_c(Lc2, Sc2, Uc2) => false
-     case decl_tp_a(La2, Sa2, Ua2) => false
-     case decl_tm(l2, T2) => false
-     case decl_mt(m2, P2, R2) => m1<m2)    
-}
-predicate decl_eq(d1: decl, d2: decl)
-  ensures d1==d2 ==> decl_eq(d1, d2);
-  ensures decl_eq(d1, d2) ==> decl_label(d1)==decl_label(d2);
-  ensures decl_eq(d1, d2) ==> d1.decl_tp_c?==d2.decl_tp_c?;
-  ensures decl_eq(d1, d2) ==> d1.decl_tp_a?==d2.decl_tp_a?;
-  ensures decl_eq(d1, d2) ==> d1.decl_tm?==d2.decl_tm?;
-  ensures decl_eq(d1, d2) ==> d1.decl_mt?==d2.decl_mt?;
-  ensures decl_eq(d1, d2) ==> !decl_lt(d1, d2) && !decl_lt(d2, d1);
-{
-  match d1
-  case decl_tp_c(Lc1, Sc1, Uc1) => d2.decl_tp_c? && d2.Lc==Lc1
-  case decl_tp_a(La1, Sa1, Ua1) => d2.decl_tp_a? && d2.La==La1
-  case decl_tm(l1, T1) => d2.decl_tm? && d2.l==l1
-  case decl_mt(m1, P1, R1) => d2.decl_mt? && d2.m==m1
-}
-predicate decl_le(d1: decl, d2: decl)
-  ensures d1==d2 ==> decl_le(d1, d2);
-{
-  decl_lt(d1, d2) || decl_eq(d1, d2)
-}
-predicate decl_seq_sorted(s: seq<decl>)
-{
-  forall m,n :: 0 <= m < n < |s| ==> decl_le(s[m], s[n])
-}
-function decl_seq_merge(s1: seq<decl>, s2: seq<decl>): seq<decl>
-{
-  if (s1 == []) then s2
-  else if (s2 == []) then s1
-  else if (decl_le(s1[0], s2[0])) then [s1[0]]+decl_seq_merge(s1[1..], s2)
-  else [s2[0]]+decl_seq_merge(s1, s2[1..])
-}
-function decl_seq_sort(s: seq<decl>): seq<decl>
-{
-  if (s == []) then s else
-    var i: nat := (|s|-1)/2;
-    decl_seq_merge(decl_seq_sort(s[..i]), decl_seq_sort(s[i+1..]))
-}
-predicate decl_lst_sorted(lst: list<decl>)
-{
-  match lst
-  case Nil => true
-  case Cons(x, tail) =>
-    (match tail
-     case Nil => true
-     case Cons(y, tail') => decl_le(x, y) && decl_lst_sorted(tail))
-}
-function decl_lst_sort(lst: list<decl>): list<decl>
-{
-  seq2lst(decl_seq_sort(lst2seq(lst)))
-}
-ghost method lemma_decl_le_trans(d1: decl, d2: decl, d3: decl)
-  requires decl_le(d1, d2);
-  requires decl_le(d2, d3);
-  ensures decl_le(d1, d3);
-{
-}
-ghost method lemma_decl_le_comparable(d1: decl, d2: decl)
-  requires !decl_le(d1, d2);
-  ensures decl_le(d2, d1);
-{
-}
-ghost method lemma_decl_seq_merging(s1: seq<decl>, s2: seq<decl>)
-  requires decl_seq_sorted(s1) && decl_seq_sorted(s2);
-  ensures decl_seq_sorted(decl_seq_merge(s1, s2));
-  ensures multiset((s1+s2)[..]) == multiset(decl_seq_merge(s1,s2)[..]);
-{
-  if (s1 == []) {}
-  else if (s2 == []) {}
-  else if (decl_le(s1[0], s2[0])) {
-    forall (n | 0 <= n < |s1|)
-      ensures decl_le(s1[0], s1[n]);
-    {
-    }
-    forall (n | 0 <= n < |s2|)
-      ensures decl_le(s1[0], s2[n]);
-    {
-      lemma_decl_le_trans(s1[0], s2[0], s2[n]);
-    }
-    var sm := decl_seq_merge(s1[1..], s2);
-    lemma_decl_seq_merging(s1[1..], s2);
-    var s := [s1[0]]+sm;
-    assert decl_le(s1[0], sm[0]);
-    forall (m,n | 0 <= m < n < |s|)
-      ensures decl_le(s[m], s[n]);
-    {
-      if (m==0) {
-        lemma_decl_le_trans(s1[0], sm[0], s[n]);
-      }
-    }
-  } else {
-    lemma_decl_le_comparable(s1[0], s2[0]);
-    forall (n | 0 <= n < |s2|)
-      ensures decl_le(s2[0], s2[n]);
-    {
-    }
-    forall (n | 0 <= n < |s1|)
-      ensures decl_le(s2[0], s1[n]);
-    {
-      lemma_decl_le_trans(s2[0], s1[0], s1[n]);
-    }
-    var sm := decl_seq_merge(s1, s2[1..]);
-    lemma_decl_seq_merging(s1, s2[1..]);
-    var s := [s2[0]]+sm;
-    assert decl_le(s2[0], sm[0]);
-    forall (m,n | 0 <= m < n < |s|)
-      ensures decl_le(s[m], s[n]);
-    {
-      if (m==0) {
-        lemma_decl_le_trans(s2[0], sm[0], s[n]);
-      }
-    }
-  }  
-}
-ghost method lemma_decl_seq_sorting(s: seq<decl>)
-  ensures decl_seq_sorted(decl_seq_sort(s));
-  ensures multiset(s[..]) == multiset(decl_seq_sort(s)[..]);
-{
-  if (s == []) {}
-  else {
-    var i: nat := (|s|-1)/2;
-    lemma_decl_seq_sorting(s[..i]);
-    lemma_decl_seq_sorting(s[i+1..]);
-    lemma_decl_seq_merging(decl_seq_sort(s[..i]), decl_seq_sort(s[i+1..]));    
-  }
-}
-predicate def_lt(d1: def, d2: def)
-{
-  match d1
-  case def_tm(l1, t1) =>
-    (match d2
-     case def_tm(l2, t2) => l1<l2
-     case def_mt(m2, param2, body2) => true)
-  case def_mt(m1, param1, body1) =>
-    (match d2
-     case def_tm(l2, t2) => false
-     case def_mt(m2, param2, body2) => m1<m2)
-}
-predicate def_eq(d1: def, d2: def)
-  ensures d1==d2 ==> def_eq(d1, d2);
-{
-  match d1
-  case def_tm(l1, t1) => d2.def_tm? && d2.l==l1
-  case def_mt(m1, param1, body1) => d2.def_mt? && d2.m==m1
-}
-predicate def_le(d1: def, d2: def)
-  ensures d1==d2 ==> def_le(d1, d2);
-{
-  def_lt(d1, d2) || def_eq(d1, d2)
-}
-predicate def_seq_sorted(s: seq<def>)
-{
-  forall m,n :: 0 <= m < n < |s| ==> def_le(s[m], s[n])
-}
-function def_seq_merge(s1: seq<def>, s2: seq<def>): seq<def>
-{
-  if (s1 == []) then s2
-  else if (s2 == []) then s1
-  else if (def_le(s1[0], s2[0])) then [s1[0]]+def_seq_merge(s1[1..], s2)
-  else [s2[0]]+def_seq_merge(s1, s2[1..])
-}
-function def_seq_sort(s: seq<def>): seq<def>
-{
-  if (s == []) then s else
-    var i: nat := (|s|-1)/2;
-    def_seq_merge(def_seq_sort(s[..i]), def_seq_sort(s[i+1..]))
-}
-ghost method lemma_def_le_trans(d1: def, d2: def, d3: def)
-  requires def_le(d1, d2);
-  requires def_le(d2, d3);
-  ensures def_le(d1, d3);
-{
-}
-ghost method lemma_def_le_comparable(d1: def, d2: def)
-  requires !def_le(d1, d2);
-  ensures def_le(d2, d1);
-{
-}
-ghost method lemma_def_seq_merging(s1: seq<def>, s2: seq<def>)
-  requires def_seq_sorted(s1) && def_seq_sorted(s2);
-  ensures def_seq_sorted(def_seq_merge(s1, s2));
-  ensures multiset((s1+s2)[..]) == multiset(def_seq_merge(s1,s2)[..]);
-{
-  if (s1 == []) {}
-  else if (s2 == []) {}
-  else if (def_le(s1[0], s2[0])) {
-    forall (n | 0 <= n < |s1|)
-      ensures def_le(s1[0], s1[n]);
-    {
-    }
-    forall (n | 0 <= n < |s2|)
-      ensures def_le(s1[0], s2[n]);
-    {
-      lemma_def_le_trans(s1[0], s2[0], s2[n]);
-    }
-    var sm := def_seq_merge(s1[1..], s2);
-    lemma_def_seq_merging(s1[1..], s2);
-    var s := [s1[0]]+sm;
-    assert def_le(s1[0], sm[0]);
-    forall (m,n | 0 <= m < n < |s|)
-      ensures def_le(s[m], s[n]);
-    {
-      if (m==0) {
-        lemma_def_le_trans(s1[0], sm[0], s[n]);
-      }
-    }
-  } else {
-    lemma_def_le_comparable(s1[0], s2[0]);
-    forall (n | 0 <= n < |s2|)
-      ensures def_le(s2[0], s2[n]);
-    {
-    }
-    forall (n | 0 <= n < |s1|)
-      ensures def_le(s2[0], s1[n]);
-    {
-      lemma_def_le_trans(s2[0], s1[0], s1[n]);
-    }
-    var sm := def_seq_merge(s1, s2[1..]);
-    lemma_def_seq_merging(s1, s2[1..]);
-    var s := [s2[0]]+sm;
-    assert def_le(s2[0], sm[0]);
-    forall (m,n | 0 <= m < n < |s|)
-      ensures def_le(s[m], s[n]);
-    {
-      if (m==0) {
-        lemma_def_le_trans(s2[0], sm[0], s[n]);
-      }
-    }
-  }  
-}
-ghost method lemma_def_seq_sorting(s: seq<def>)
-  ensures def_seq_sorted(def_seq_sort(s));
-  ensures multiset(s[..]) == multiset(def_seq_sort(s)[..]);
-{
-  if (s == []) {}
-  else {
-    var i: nat := (|s|-1)/2;
-    lemma_def_seq_sorting(s[..i]);
-    lemma_def_seq_sorting(s[i+1..]);
-    lemma_def_seq_merging(def_seq_sort(s[..i]), def_seq_sort(s[i+1..]));    
-  }
 }
 
 // ---------------------
@@ -588,41 +79,37 @@ ghost method lemma_def_seq_sorting(s: seq<def>)
 // ### Values ###
 predicate value(t: tm)
 {
-  t.tm_var?
+  t.tm_loc?
+}
+predicate syn_value(t: tm)
+{
+  t.tm_loc? || t.tm_var?
 }
 
 // ### Store ###
-datatype store = Store(m: partial_map<int,pair<tp, list<def>>>);
-function store_lookup(n: nat, s: store): list<def>
-  requires n in dom(s.m);
+datatype store = Store(m: seq<pair<tp, seq<def>>>);
+function store_lookup(loc: nat, s: store): seq<def>
+  requires loc < |s.m|;
 {
-  lookup(n, s.m).get.snd
+  s.m[loc].snd
 }
-function alloc(s: store): nat
-  ensures alloc(s) !in dom(s.m);
+function store_lookup_type(loc: nat, s: store): tp
+  requires loc < |s.m|;
 {
-  other(dom(s.m))
+  s.m[loc].fst
 }
-function other(xs: seq<int>): nat
-{
-  max(xs, -1) + 1
-}
-function def_method_lookup(m: nat, defs: list<def>): option<pair<int, tm>>
+function def_method_lookup(m: nat, defs: seq<def>): option<pair<int, tm>>
   ensures def_method_lookup(m, defs).Some? ==> def_method_lookup(m, defs).get.fst>=0;
 {
-  match defs
-  case Nil => None
-  case Cons(head, tail) =>
-    if (head.def_mt? && head.m==m) then Some(P(head.param, head.body))
-    else def_method_lookup(m, tail)
+  if (exists i :: 0 <= i < |defs| && defs[i].def_mt? && defs[i].m==m)
+  then (var i :| 0 <= i < |defs| && defs[i].def_mt? && defs[i].m==m; Some(P(defs[i].param, defs[i].body)))
+  else None
 }
-function def_field_lookup(l: nat, defs: list<def>): option<tm>
+function def_field_lookup(l: nat, defs: seq<def>): option<tm>
 {
-  match defs
-  case Nil => None
-  case Cons(head, tail) =>
-    if (head.def_tm? && head.l==l) then Some(head.t)
-    else def_field_lookup(l, tail)
+  if (exists i :: 0 <= i < |defs| && defs[i].def_tm? && defs[i].l==l)
+  then (var i :| 0 <= i < |defs| && defs[i].def_tm? && defs[i].l==l; Some(defs[i].t))
+  else None
 }
 
 // ### Size ###
@@ -640,12 +127,11 @@ function tm_size(t: tm): nat
   case tm_new(y, Tc, init, t1) => 1+tp_size(Tc)+defs_size(init)+tm_size(t1)
   case tm_sel(t1, l) => 1+tm_size(t1)
   case tm_msel(o, m, a) => 1+tm_size(o)+tm_size(a)
+  case tm_loc(loc) => 1
 }
 function tp_size(T: tp): nat
-  ensures T.tp_sel_c? ==> tp_size(T)==1+tm_size(T.pc);
-  ensures T.tp_sel_c? ==> tp_size(T)>tm_size(T.pc);
-  ensures T.tp_sel_a? ==> tp_size(T)==1+tm_size(T.pa);
-  ensures T.tp_sel_a? ==> tp_size(T)>tm_size(T.pa);
+  ensures T.tp_sel? ==> tp_size(T)==1+tm_size(T.p);
+  ensures T.tp_sel? ==> tp_size(T)>tm_size(T.p);
   ensures T.tp_rfn? ==> tp_size(T)==1+tp_size(T.base_tp)+decls_size(T.decls);
   ensures T.tp_rfn? ==> tp_size(T)>tp_size(T.base_tp);
   ensures T.tp_rfn? ==> tp_size(T)>decls_size(T.decls);
@@ -655,8 +141,7 @@ function tp_size(T: tp): nat
   ensures T.tp_or? ==> tp_size(T)>tp_size(T.or1);
 {
   match T
-  case tp_sel_c(pc, Lc) => 1+tm_size(pc)
-  case tp_sel_a(pa, La) => 1+tm_size(pa)
+  case tp_sel(p, L, concrete) => 1+tm_size(p)
   case tp_rfn(base_tp, self, decls) => 1+tp_size(base_tp)+decls_size(decls)
   case tp_and(and1, and2) => 1+tp_size(and1)+tp_size(and2)
   case tp_or(or1, or2) => 1+tp_size(or1)+tp_size(or2)
@@ -674,12 +159,9 @@ function def_size(d: def): nat
   case def_mt(m, param, body) => 1+tm_size(body)
 }
 function decl_size(d: decl): nat
-  ensures d.decl_tp_c? ==> decl_size(d)==1+tp_size(d.Sc)+tp_size(d.Uc);
-  ensures d.decl_tp_c? ==> decl_size(d)>tp_size(d.Sc);
-  ensures d.decl_tp_c? ==> decl_size(d)>tp_size(d.Uc);
-  ensures d.decl_tp_a? ==> decl_size(d)==1+tp_size(d.Sa)+tp_size(d.Ua);
-  ensures d.decl_tp_a? ==> decl_size(d)>tp_size(d.Sa);
-  ensures d.decl_tp_a? ==> decl_size(d)>tp_size(d.Ua);
+  ensures d.decl_tp? ==> decl_size(d)==1+tp_size(d.S)+tp_size(d.U);
+  ensures d.decl_tp? ==> decl_size(d)>tp_size(d.S);
+  ensures d.decl_tp? ==> decl_size(d)>tp_size(d.U);
   ensures d.decl_tm? ==> decl_size(d)==1+tp_size(d.T);
   ensures d.decl_tm? ==> decl_size(d)>tp_size(d.T);
   ensures d.decl_mt? ==> decl_size(d)==1+tp_size(d.P)+tp_size(d.R);
@@ -687,8 +169,7 @@ function decl_size(d: decl): nat
   ensures d.decl_mt? ==> decl_size(d)>tp_size(d.R);
 {
   match d
-  case decl_tp_c(Lc, Sc, Uc) => 1+tp_size(Sc)+tp_size(Uc)
-  case decl_tp_a(La, Sa, Ua) => 1+tp_size(Sa)+tp_size(Ua)
+  case decl_tp(L, S, U, concrete) => 1+tp_size(S)+tp_size(U)
   case decl_tm(l, T) => 1+tp_size(T)
   case decl_mt(m, P, R) => 1+tp_size(P)+tp_size(R)
 }
@@ -718,24 +199,24 @@ function tm_subst(x: nat, v: tm, t: tm): tm
   case tm_var(x') => if x'==x then v else t
   case tm_new(y, Tc, init, t1) =>
     if y==x then tm_new(y, tp_subst(x, v, Tc), init, t1) else
-    var y' := if (tm_fn(y, v)) then other([x]+tm_vars(v)+tm_vars(t)) else y;
-    var init' := if (y==y') then init else defs_subst(y, tm_var(y'), init);
-    var t1' := if (y==y') then t1 else tm_subst(y, tm_var(y'), t1);
+    var y' := fresh_from([x]+tm_vars(v)+tm_vars(t));
+    var init' := defs_subst(y, tm_var(y'), init);
+    var t1' := tm_subst(y, tm_var(y'), t1);
     tm_new(y', tp_subst(x, v, Tc), defs_subst(x, v, init'), tm_subst(x, v, t1'))
   case tm_sel(t1, l) => tm_sel(tm_subst(x, v, t1), l)
   case tm_msel(o, m, a) => tm_msel(tm_subst(x, v, o), m, tm_subst(x, v, a))
+  case tm_loc(loc) => t
 }
 function tp_subst(x: nat, v: tm, T: tp): tp
   decreases tp_size(T), T;
   ensures v.tm_var? ==> tp_size(T)==tp_size(tp_subst(x, v, T));
 {
   match T
-  case tp_sel_c(pc, Lc) => tp_sel_c(tm_subst(x, v, pc), Lc)
-  case tp_sel_a(pa, La) => tp_sel_a(tm_subst(x, v, pa), La)
+  case tp_sel(p, L, concrete) => tp_sel(tm_subst(x, v, p), L, concrete)
   case tp_rfn(base_tp, self, decls) =>
     if self==x then tp_rfn(tp_subst(x, v, base_tp), self, decls) else
-    var self' := if (tm_fn(self, v)) then other([x]+tm_vars(v)+tp_vars(T)) else self;
-    var decls' := if (self==self') then decls else decls_subst(self, tm_var(self'), decls);
+    var self' := fresh_from([x]+tm_vars(v)+tp_vars(T));
+    var decls' := decls_subst(self, tm_var(self'), decls);
     tp_rfn(tp_subst(x, v, base_tp), self', decls_subst(x, v, decls'))
   case tp_and(and1, and2) => tp_and(tp_subst(x, v, and1), tp_subst(x, v, and2))
   case tp_or(or1, or2) => tp_or(tp_subst(x, v, or1), tp_subst(x, v, or2))
@@ -750,7 +231,7 @@ function def_subst(x: nat, v: tm, d: def): def
   case def_tm(l, t1) => def_tm(l, tm_subst(x, v, t1))
   case def_mt(m, param, body) =>
     if param==x then d else
-    var param' := if (tm_fn(param, v)) then other([x]+tm_vars(v)+def_vars(d)) else param;
+    var param' := if (tm_fn(param, v)) then fresh_from([x]+tm_vars(v)+def_vars(d)) else param;
     var body' := if (param==param') then body else tm_subst(param, tm_var(param'), body);
     def_mt(m, param', tm_subst(x, v, body'))
 }
@@ -759,8 +240,7 @@ function decl_subst(x: nat, v: tm, d: decl): decl
   ensures v.tm_var? ==> decl_size(d)==decl_size(decl_subst(x, v, d));
 {
   match d
-  case decl_tp_c(Lc, Sc, Uc) => decl_tp_c(Lc, tp_subst(x, v, Sc), tp_subst(x, v, Uc))
-  case decl_tp_a(La, Sa, Ua) => decl_tp_a(La, tp_subst(x, v, Sa), tp_subst(x, v, Ua))
+  case decl_tp(L, S, U, concrete) => decl_tp(L, tp_subst(x, v, S), tp_subst(x, v, U), concrete)
   case decl_tm(l, T) => decl_tm(l, tp_subst(x, v, T))
   case decl_mt(m, P, R) => decl_mt(m, tp_subst(x, v, P), tp_subst(x, v, R))
 }
@@ -780,27 +260,27 @@ function decls_subst(x: nat, v: tm, decls: list<decl>): list<decl>
   case Nil => Nil
   case Cons(head, tail) => Cons(decl_subst(x, v, head), decls_subst(x, v, tail))
 }
-function decls_fin_subst(x: nat, v: tm, decls: seq<decl>): seq<decl>
-{
-  lst2seq(decls_subst(x, v, seq2lst(decls)))
-}
 
 // ### Free variables ###
 // fn(x, A) <==> x appears free in A
 
 predicate tm_fn(x: nat, t: tm)
+  ensures tm_fn(x, t) ==> x in tm_vars(t);
+  decreases t;
 {
   match t
   case tm_var(x') => x'==x
   case tm_new(y, Tc, init, t') => tp_fn(x, Tc) || (y!=x && (defs_fn(x, init) || tm_fn(x, t')))
   case tm_sel(t1, l) => tm_fn(x, t1)
   case tm_msel(o, m, a) => tm_fn(x, o) || tm_fn(x, a)
+  case tm_loc(loc) => false
 }
 predicate tp_fn(x: nat, T: tp)
+  ensures tp_fn(x, T) ==> x in tp_vars(T);
+  decreases T;
 {
   match T
-  case tp_sel_c(pc, Lc) => tm_fn(x, pc)
-  case tp_sel_a(pa, La) => tm_fn(x, pa)
+  case tp_sel(p, L, concrete) => tm_fn(x, p)
   case tp_rfn(base_tp, self, decls) => tp_fn(x, base_tp) || (self!=x && decls_fn(x, decls))
   case tp_and(and1, and2) => tp_fn(x, and1) || tp_fn(x, and2)
   case tp_or(or1, or2) => tp_fn(x, or1) || tp_fn(x, or2)
@@ -808,24 +288,31 @@ predicate tp_fn(x: nat, T: tp)
   case tp_bot => false
 }
 predicate def_fn(x: nat, d: def)
+  ensures def_fn(x, d) ==> x in def_vars(d);
+  decreases d;
 {
   match d
   case def_tm(l, t1) => tm_fn(x, t1)
   case def_mt(m, param, body) => param!=x && tm_fn(x, body)
 }
 predicate decl_fn(x: nat, d: decl)
+  ensures decl_fn(x, d) ==> x in decl_vars(d);
+  decreases d;
 {
   match d
-  case decl_tp_c(Lc, Sc, Uc) => tp_fn(x, Sc) || tp_fn(x, Uc)
-  case decl_tp_a(La, Sa, Ua) => tp_fn(x, Sa) || tp_fn(x, Ua)
+  case decl_tp(L, S, U, concrete) => tp_fn(x, S) || tp_fn(x, U)
   case decl_tm(l, T) => tp_fn(x, T)
   case decl_mt(m, P, R) => tp_fn(x, P) || tp_fn(x, R)
 }
 predicate defs_fn(x: nat, defs: list<def>)
+  ensures defs_fn(x, defs) ==> x in defs_vars(defs);
+  decreases defs;
 {
   defs.Cons? && (def_fn(x, defs.head) || defs_fn(x, defs.tail))
 }
 predicate decls_fn(x: nat, decls: list<decl>)
+  ensures decls_fn(x, decls) ==> x in decls_vars(decls);
+  decreases decls;
 {
   decls.Cons? && (decl_fn(x, decls.head) || decls_fn(x, decls.tail))
 }
@@ -839,13 +326,13 @@ function tm_vars(t: tm): seq<int>
   case tm_new(y, Tc, init, t') => [y]+tp_vars(Tc)+defs_vars(init)+tm_vars(t')
   case tm_sel(t1, l) => tm_vars(t1)
   case tm_msel(o, m, a) => tm_vars(o)+tm_vars(a)
+  case tm_loc(loc) => []
 }
 function tp_vars(T: tp): seq<int>
   ensures forall x :: x in tp_vars(T) ==> x>=0;
 {
   match T
-  case tp_sel_c(pc, Lc) => tm_vars(pc)
-  case tp_sel_a(pa, La) => tm_vars(pa)
+  case tp_sel(p, L, concrete) => tm_vars(p)
   case tp_rfn(base_tp, self, decls) => tp_vars(base_tp)+[self]+decls_vars(decls)
   case tp_and(and1, and2) => tp_vars(and1)+tp_vars(and2)
   case tp_or(or1, or2) => tp_vars(or1)+tp_vars(or2)
@@ -863,13 +350,13 @@ function decl_vars(d: decl): seq<int>
   ensures forall x :: x in decl_vars(d) ==> x>=0;
 {
   match d
-  case decl_tp_c(Lc, Sc, Uc) => tp_vars(Sc)+tp_vars(Uc)
-  case decl_tp_a(La, Sa, Ua) => tp_vars(Sa)+tp_vars(Ua)
+  case decl_tp(L, S, U, concrete) => tp_vars(S)+tp_vars(U)
   case decl_tm(l, T) => tp_vars(T)
   case decl_mt(m, P, R) => tp_vars(P)+tp_vars(R)
 }
 function defs_vars(defs: list<def>): seq<int>
   ensures forall x :: x in defs_vars(defs) ==> x>=0;
+  ensures defs.Cons? ==> defs_vars(defs)==def_vars(defs.head)+defs_vars(defs.tail);
 {
   match defs
   case Nil => []
@@ -877,6 +364,7 @@ function defs_vars(defs: list<def>): seq<int>
 }
 function decls_vars(decls: list<decl>): seq<int>
   ensures forall x :: x in decls_vars(decls) ==> x>=0;
+  ensures decls.Cons? ==> decls_vars(decls)==decl_vars(decls.head)+decls_vars(decls.tail);
 {
   match decls
   case Nil => []
@@ -885,14 +373,13 @@ function decls_vars(decls: list<decl>): seq<int>
 
 // ### Reduction ###
 function step(t: tm, s: store): option<pair<tm, store>>
-  ensures step(t, s).Some? ==> prefix_of(step(t, s).get.snd.m, s.m);
 {
   /* msel */
-  if (t.tm_msel? && t.o.tm_var? && value(t.a) && t.o.x in dom(s.m) &&
-     def_method_lookup(t.m, store_lookup(t.o.x, s)).Some?)
-  then Some(P(tm_subst(def_method_lookup(t.m, store_lookup(t.o.x, s)).get.fst,
+  if (t.tm_msel? && t.o.tm_loc? && value(t.a) && t.o.loc < |s.m| &&
+     def_method_lookup(t.m, store_lookup(t.o.loc, s)).Some?)
+  then Some(P(tm_subst(def_method_lookup(t.m, store_lookup(t.o.loc, s)).get.fst,
                        t.a,
-                       def_method_lookup(t.m, store_lookup(t.o.x, s)).get.snd),
+                       def_method_lookup(t.m, store_lookup(t.o.loc, s)).get.snd),
               s))
   /* msel1 */
   else if (t.tm_msel? && step(t.o, s).Some?)
@@ -901,16 +388,16 @@ function step(t: tm, s: store): option<pair<tm, store>>
   else if (t.tm_msel? && value(t.o) && step(t.a, s).Some?)
   then Some(P(tm_msel(t.o, t.m, step(t.a, s).get.fst), step(t.a, s).get.snd))
   /* sel */
-  else if (t.tm_sel? && t.t.tm_var? && t.t.x in dom(s.m) &&
-           def_field_lookup(t.l, store_lookup(t.t.x, s)).Some?)
-  then Some(P(def_field_lookup(t.l, store_lookup(t.t.x, s)).get, s))
+  else if (t.tm_sel? && t.t.tm_loc? && t.t.loc < |s.m| &&
+           def_field_lookup(t.l, store_lookup(t.t.loc, s)).Some?)
+  then Some(P(def_field_lookup(t.l, store_lookup(t.t.loc, s)).get, s))
   /* sel1 */
   else if (t.tm_sel? && step(t.t, s).Some?)
   then Some(P(tm_sel(step(t.t, s).get.fst, t.l), step(t.t, s).get.snd))
   /* new */
   else if (t.tm_new?)
-  then Some(P(tm_subst(t.y, tm_var(alloc(s)), t.t'),
-              Store(Extend(alloc(s), P(t.Tc, defs_subst(t.y, tm_var(alloc(s)), t.init)), s.m))))
+  then Some(P(tm_subst(t.y, tm_loc(|s.m|), t.t'),
+              Store(s.m+[P(t.Tc, lst2seq(defs_subst(t.y, tm_loc(|s.m|), t.init)))])))
   else None
 }
 
@@ -921,7 +408,6 @@ predicate irred(t: tm, s: store)
 
 // ### Multi-steps ###
 predicate mstep(t: tm, s: store, t': tm, s': store, n: nat)
-  //ensures mstep(t, s, t', s', n) ==> prefix_of(s'.m, s.m);
   decreases n;
 {
   if (n==0) then t==t' && s==s'
@@ -934,24 +420,6 @@ ghost method lemma_value__irred(t: tm, s: store)
   requires value(t);
   ensures irred(t, s);
 {
-}
-
-ghost method lemma_step__prefix(t1: tm, s1: store, t2: tm, s2: store)
-  requires step(t1, s1) == Some(P(t2, s2));
-  ensures prefix_of(s2.m, s1.m);
-{
-}
-
-ghost method lemma_mstep__prefix(t1: tm, s1: store, t2: tm, s2: store, n: nat)
-  requires mstep(t1, s1, t2, s2, n);
-  ensures prefix_of(s2.m, s1.m);
-  decreases n;
-{
-  if (n>0) {
-    lemma_step__prefix(t1, s1, step(t1, s1).get.fst, step(t1, s1).get.snd);
-    lemma_mstep__prefix(step(t1, s1).get.fst, step(t1, s1).get.snd, t2, s2, n-1);
-    lemma_prefix_of_trans(s1.m, step(t1, s1).get.snd.m, s2.m);
-  }
 }
 
 ghost method lemma_mstep_trans(t1: tm, s1: store, t2: tm, s2: store, t3: tm, s3: store, n12: nat, n23: nat)
@@ -1017,20 +485,135 @@ ghost method lemma_sel_irred__o_mstep_irred(o: tm, l: nat, t': tm, s: store, s':
 // -----------
 
 // ### Context ###
-datatype context = Context(m: partial_map<int,tp>);
-function ctx_extend(x: nat, T: tp, ctx: context): context
-  ensures ctx_extend(x, T, ctx).m == Extend(x, T, ctx.m);
-  ensures prefix_of(ctx_extend(x, T, ctx).m, ctx.m);
+datatype context = Context(m: seq<pair<int,tp>>);
+function context_extend(ctx: context, x: nat, T: tp): context
+  requires context_lookup(ctx, x).None?;
 {
-  Context(Extend(x, T, ctx.m))
+  Context([P(x, T)]+ctx.m)
+}
+function context_lookup(ctx: context, x: nat): option<tp>
+  decreases |ctx.m|;
+{
+  if (|ctx.m|==0) then None
+  else if (ctx.m[0].fst==x) then Some(ctx.m[0].snd)
+  else context_lookup(Context(ctx.m[1..]), x)
+}
+function dom(ctx: context): seq<int>
+  ensures forall x:nat :: x !in dom(ctx) ==> context_lookup(ctx, x).None?;
+  ensures forall x:nat :: x in dom(ctx) ==> context_lookup(ctx, x).Some?;
+  decreases |ctx.m|;
+{
+  if (ctx.m==[]) then [] else [ctx.m[0].fst]+dom(Context(ctx.m[1..]))
+}
+function fresh_in_context(ctx: context): nat
+  ensures context_lookup(ctx, fresh_in_context(ctx)).None?;
+{
+  fresh_from(dom(ctx))
+}
+
+// ### Orderings ###
+predicate decl_lt(d1: decl, d2: decl)
+{
+  match d1
+  case decl_tp(L1, S1, U1, concrete1) =>
+    (match d2
+     case decl_tp(L2, S2, U2, concrete2) =>
+       (concrete1 && !concrete2) || (concrete1==concrete2 && L1<L2)
+     case decl_tm(l2, T2) => true
+     case decl_mt(m2, P2, R2) => true)
+  case decl_tm(l1, T1) =>
+    (match d2
+     case decl_tp(L2, S2, U2, concrete2) => false
+     case decl_tm(l2, T2) => l1<l2
+     case decl_mt(m2, P2, R2) => true)
+  case decl_mt(m1, P1, R1) =>
+    (match d2
+     case decl_tp(L2, S2, U2, concrete2) => false
+     case decl_tm(l2, T2) => false
+     case decl_mt(m2, P2, R2) => m1<m2)    
+}
+predicate decl_eq(d1: decl, d2: decl)
+  ensures d1==d2 ==> decl_eq(d1, d2);
+  ensures decl_eq(d1, d2) ==> decl_label(d1)==decl_label(d2);
+  ensures decl_eq(d1, d2) ==> d1.decl_tp?==d2.decl_tp?;
+  ensures decl_eq(d1, d2) ==> d1.decl_tm?==d2.decl_tm?;
+  ensures decl_eq(d1, d2) ==> d1.decl_mt?==d2.decl_mt?;
+  ensures decl_eq(d1, d2) ==> !decl_lt(d1, d2) && !decl_lt(d2, d1);
+{
+  match d1
+  case decl_tp(L1, S1, U1, concrete1) => d2.decl_tp? && d2.concrete==concrete1 && d2.L==L1
+  case decl_tm(l1, T1) => d2.decl_tm? && d2.l==l1
+  case decl_mt(m1, P1, R1) => d2.decl_mt? && d2.m==m1
+}
+predicate decl_le(d1: decl, d2: decl)
+  ensures d1==d2 ==> decl_le(d1, d2);
+{
+  decl_lt(d1, d2) || decl_eq(d1, d2)
+}
+predicate decl_seq_sorted(s: seq<decl>)
+{
+  forall m,n :: 0 <= m < n < |s| ==> decl_le(s[m], s[n])
+}
+function decl_seq_merge(s1: seq<decl>, s2: seq<decl>): seq<decl>
+{
+  if (s1 == []) then s2
+  else if (s2 == []) then s1
+  else if (decl_le(s1[0], s2[0])) then [s1[0]]+decl_seq_merge(s1[1..], s2)
+  else [s2[0]]+decl_seq_merge(s1, s2[1..])
+}
+function decl_seq_sort(s: seq<decl>): seq<decl>
+{
+  if (s == []) then s else
+    var i: nat := (|s|-1)/2;
+    decl_seq_merge(decl_seq_sort(s[..i]), decl_seq_sort(s[i+1..]))
+}
+predicate def_lt(d1: def, d2: def)
+{
+  match d1
+  case def_tm(l1, t1) =>
+    (match d2
+     case def_tm(l2, t2) => l1<l2
+     case def_mt(m2, param2, body2) => true)
+  case def_mt(m1, param1, body1) =>
+    (match d2
+     case def_tm(l2, t2) => false
+     case def_mt(m2, param2, body2) => m1<m2)
+}
+predicate def_eq(d1: def, d2: def)
+  ensures d1==d2 ==> def_eq(d1, d2);
+{
+  match d1
+  case def_tm(l1, t1) => d2.def_tm? && d2.l==l1
+  case def_mt(m1, param1, body1) => d2.def_mt? && d2.m==m1
+}
+predicate def_le(d1: def, d2: def)
+  ensures d1==d2 ==> def_le(d1, d2);
+{
+  def_lt(d1, d2) || def_eq(d1, d2)
+}
+predicate def_seq_sorted(s: seq<def>)
+{
+  forall m,n :: 0 <= m < n < |s| ==> def_le(s[m], s[n])
+}
+function def_seq_merge(s1: seq<def>, s2: seq<def>): seq<def>
+{
+  if (s1 == []) then s2
+  else if (s2 == []) then s1
+  else if (def_le(s1[0], s2[0])) then [s1[0]]+def_seq_merge(s1[1..], s2)
+  else [s2[0]]+def_seq_merge(s1, s2[1..])
+}
+function def_seq_sort(s: seq<def>): seq<def>
+{
+  if (s == []) then s else
+    var i: nat := (|s|-1)/2;
+    def_seq_merge(def_seq_sort(s[..i]), def_seq_sort(s[i+1..]))
 }
 
 // ### Declaration Lattice ###
 predicate decl_bot(d: decl)
 {
   match d
-  case decl_tp_c(L, S, U) => S==tp_top && U==tp_bot
-  case decl_tp_a(L, S, U) => S==tp_top && U==tp_bot
+  case decl_tp(L, S, U, concrete) => S==tp_top && U==tp_bot
   case decl_tm(l, T) => T==tp_bot
   case decl_mt(m, S, U) => S==tp_top && U==tp_bot
 }
@@ -1040,8 +623,7 @@ function decl_and(d1: decl, d2: decl): decl
   ensures decl_eq(d2, decl_and(d1, d2));
 {
   match d1
-  case decl_tp_c(L, S, U) => decl_tp_c(L, tp_or(S, d2.Sc), tp_and(U, d2.Uc))
-  case decl_tp_a(L, S, U) => decl_tp_a(L, tp_or(S, d2.Sa), tp_and(U, d2.Ua))
+  case decl_tp(L, S, U, concrete) => decl_tp(L, tp_or(S, d2.S), tp_and(U, d2.U), concrete)
   case decl_tm(l, U) => decl_tm(l, tp_and(U, d2.T))
   case decl_mt(m, S, U) => decl_mt(m, tp_or(S, d2.P), tp_and(U, d2.R))
 }
@@ -1051,15 +633,11 @@ function decl_or(d1: decl, d2: decl): decl
   ensures decl_eq(d2, decl_or(d1, d2));
 {
   match d1
-  case decl_tp_c(L, S, U) => decl_tp_c(L, tp_and(S, d2.Sc), tp_or(U, d2.Uc))
-  case decl_tp_a(L, S, U) => decl_tp_a(L, tp_and(S, d2.Sa), tp_or(U, d2.Ua))
+  case decl_tp(L, S, U, concrete) => decl_tp(L, tp_and(S, d2.S), tp_or(U, d2.U), concrete)
   case decl_tm(l, U) => decl_tm(l, tp_or(U, d2.T))
   case decl_mt(m, S, U) => decl_mt(m, tp_and(S, d2.P), tp_or(U, d2.R))
 }
 function decls_fin_and(s1: seq<decl>, s2: seq<decl>): seq<decl>
-  requires decl_seq_sorted(s1);
-  requires decl_seq_sorted(s2);
-  //ensures decl_seq_sorted(decls_fin_and(s1, s2));
 {
         if (s1 == []) then s2
   else  if (s2 == []) then s1
@@ -1068,21 +646,15 @@ function decls_fin_and(s1: seq<decl>, s2: seq<decl>): seq<decl>
   else/*if (decl_lt(s2[0], s1[0])) then*/ [s2[0]]+decls_fin_and(s1, s2[1..])
 }
 function decls_and(Ds1: decls, Ds2: decls): decls
-  requires Ds1.decls_fin? ==> decl_seq_sorted(Ds1.decls);
-  requires Ds2.decls_fin? ==> decl_seq_sorted(Ds2.decls);
-  //ensures decls_and(Ds1, Ds2).decls_fin? ==> decl_seq_sorted(decls_and(Ds1, Ds2).decls); 
 {
   match Ds1
   case decls_bot => decls_bot
   case decls_fin(s1) =>
     (match Ds2
      case decls_bot => decls_bot
-     case decls_fin(s2) => decls_fin(decls_fin_and(s1, s2)))
+     case decls_fin(s2) => decls_fin(seq2lst(decls_fin_and(lst2seq(s1), lst2seq(s2)))))
 }
 function decls_fin_or(s1: seq<decl>, s2: seq<decl>): seq<decl>
-  requires decl_seq_sorted(s1);
-  requires decl_seq_sorted(s2);
-  //ensures decl_seq_sorted(decls_fin_or(s1, s2));
 {
         if (s1 == []) then []
   else  if (s2 == []) then []
@@ -1091,633 +663,808 @@ function decls_fin_or(s1: seq<decl>, s2: seq<decl>): seq<decl>
   else/*if (decl_lt(s2[0], s1[0])) then*/ decls_fin_or(s1, s2[1..])
 }
 function decls_or(Ds1: decls, Ds2: decls): decls
-  requires Ds1.decls_fin? ==> decl_seq_sorted(Ds1.decls);
-  requires Ds2.decls_fin? ==> decl_seq_sorted(Ds2.decls);
-  //ensures decls_or(Ds1, Ds2).decls_fin? ==> decl_seq_sorted(decls_or(Ds1, Ds2).decls); 
 {
   match Ds1
   case decls_bot => Ds2
   case decls_fin(s1) =>
     (match Ds2
      case decls_bot => Ds1
-     case decls_fin(s2) => decls_fin(decls_fin_or(s1, s2)))
+     case decls_fin(s2) => decls_fin(seq2lst(decls_fin_or(lst2seq(s1), lst2seq(s2)))))
 }
 
 // ### Typing-Related Judgments ###
 
-copredicate typing(ctx: context, t: tm, T: tp)
+predicate typing(n: nat, ctx: context, s: store, t: tm, T: tp)
+  decreases n;
 {
   match t
-  case tm_var(x) => lookup(x, ctx.m) == Some(T)
-  case tm_new(y, Tc, init, t') =>
+  case tm_var(x) => context_lookup(ctx, x)==Some(T)
+  case tm_new(y_, Tc, init_, t'_) =>
+    var y := fresh_from(dom(ctx)+tm_vars(t));
+    var init := defs_subst(y_, tm_var(y), init_);
+    var t' := tm_subst(y_, tm_var(y), t'_);
+    n>0 && is_concrete(Tc) &&
     exists Ds:decls :: Ds.decls_fin? &&
-    wfe_type(ctx, Tc) &&
-    expansion(ctx, y, Tc, Ds) && 
-    wf_init(Context(Extend(y, Tc, ctx.m)), Ds.decls, def_seq_sort(lst2seq(init))) &&
+    wfe_type(n-1, ctx, s, Tc) &&
+    expansion(n-1, ctx, s, y, Tc, Ds) && 
+    wf_init(n-1, false, context_extend(ctx, y, Tc), s, lst2seq(Ds.decls), lst2seq(init)) &&
     !tp_fn(y, T) &&
-    typing(Context(Extend(y, Tc, ctx.m)), t', T)
+    exists T' :: typing(n-1, context_extend(ctx, y, Tc), s, t', T') &&
+    subtype(n-1, context_extend(ctx, y, Tc), s, T', T)
   case tm_sel(t, l) =>
-    field_membership(ctx, t, l, T)
+    n>0 && field_membership(n-1, ctx, s, t, l, T)
   case tm_msel(o, m, a) =>
-    exists S, T' :: method_membership(ctx, o, m, S, T) &&
-    typing(ctx, a, T') &&
-    subtype(ctx, T', S)
+    n>0 && exists S, T' :: method_membership(n-1, ctx, s, o, m, S, T) &&
+    typing(n-1, ctx, s, a, T') &&
+    subtype(n-1, ctx, s, T', S)
+  case tm_loc(loc) => loc < |s.m| && store_lookup_type(loc, s)==T
 }
-copredicate wf_init(ctx: context, decls: seq<decl>, defs: seq<def>)
-  //requires decl_seq_sorted(decls);
-  //requires def_seq_sorted(defs);
+predicate wf_init(n: nat, already_in_store: bool, ctx: context, s: store, decls: seq<decl>, defs: seq<def>)
+  decreases n;
 {
-  (decls==[] && defs==[]) || (|decls|>0 && (
-    (((decls[0].decl_tp_c? && subtype(ctx, decls[0].Sc, decls[0].Uc)) ||
-      (decls[0].decl_tp_a? && subtype(ctx, decls[0].Sa, decls[0].Ua))) &&
-     wf_init(ctx, decls[1..], defs)) || (|defs|>0 && (
-    ((decls[0].decl_tm? && defs[0].def_tm? && decls[0].l==defs[0].l &&
-      value(defs[0].t) &&
-      exists T :: typing(ctx, defs[0].t, T) &&
-      subtype(ctx, T, decls[0].T)) ||
-     (decls[0].decl_mt? && defs[0].def_mt? && decls[0].m==defs[0].m &&
-      wfe_type(ctx, decls[0].P) &&
-      exists T' :: typing(Context(Extend(defs[0].param, decls[0].P, ctx.m)), defs[0].body, T') &&
-      subtype(Context(Extend(defs[0].param, decls[0].P, ctx.m)), T', decls[0].R))) &&
-     wf_init(ctx, decls[1..], defs[1..])))))
+  var p:nat := fresh_in_context(ctx);
+  n>0 && forall d :: d in decls ==> (
+  if (d.decl_tp?) then subtype(n-1, ctx, s, d.S, d.U)
+  else if (d.decl_tm?) then exists def :: def in defs && def.def_tm? && def.l==d.l && (if already_in_store then value(def.t) else syn_value(def.t)) &&
+                            exists T :: typing(n-1, ctx, s, def.t, T) && subtype(n-1, ctx, s, T, d.T)
+  else if (d.decl_mt?) then exists def :: def in defs && def.def_mt? && def.m==d.m &&
+                            exists T' :: typing(n-1, context_extend(ctx, p, d.P), s, tm_subst(def.param, tm_var(p), def.body), T') &&
+                                         subtype(n-1, context_extend(ctx, p, d.P), s, T', d.R)
+  else false)
 }
-copredicate wf_decl(ctx: context, d: decl)
+predicate wf_decl(n: nat, ctx: context, s: store, d: decl)
+  decreases n;
 {
   match d
-  case decl_tp_c(L, S, U) => wf_type(ctx, S) && wf_type(ctx, U)
-  case decl_tp_a(L, S, U) => wf_type(ctx, S) && wf_type(ctx, U)
-  case decl_tm(l, T) => wf_type(ctx, T)
-  case decl_mt(m, S, T) => wf_type(ctx, S) && wf_type(ctx, T)
+  case decl_tp(L, S, U, concrete) => n>0 && wf_type(n-1, ctx, s, S) && wf_type(n-1, ctx, s, U) &&
+    (!concrete || (S==tp_bot && is_concrete(U)))
+  case decl_tm(l, T) => n>0 && wf_type(n-1, ctx, s, T)
+  case decl_mt(m, S, T) => n>0 && wf_type(n-1, ctx, s, S) && wf_type(n-1, ctx, s, T)
 }
-copredicate wf_decls(ctx: context, Ds: list<decl>)
+predicate wf_decls(n: nat, ctx: context, s: store, Ds: seq<decl>)
+  decreases n;
 {
-  match Ds
-  case Nil => true
-  case Cons(head, tail) => wf_decl(ctx, head) && wf_decls(ctx, tail)
+  forall d :: d in Ds ==> n>0 && wf_decl(n-1, ctx, s, d)
 }
-copredicate wf_type(ctx: context, T: tp)
+predicate wf_type(n: nat, ctx: context, s: store, T: tp)
+  decreases n;
 {
   match T
-  case tp_rfn(T', z, Ds) =>
-    wf_type(ctx, T') && wf_decls(Context(Extend(z, T, ctx.m)), Ds)
-  case tp_sel_c(p, L) =>
+  case tp_rfn(T', z_, Ds_) =>
+    var z:= fresh_in_context(ctx);
+    var Ds := decls_subst(z_, tm_var(z), Ds_);
+    n>0 && wf_type(n-1, ctx, s, T') && wf_decls(n-1, context_extend(ctx, z, T), s, lst2seq(Ds))
+  case tp_sel(p, L, concrete) =>
     path(p) &&
-    exists S, U :: concrete_type_membership(ctx, p, L, S, U)
-  case tp_sel_a(p, L) =>
-    path(p) &&
-    exists S, U :: abstract_type_membership(ctx, p, L, S, U)
-  case tp_and(T1, T2) => wf_type(ctx, T1) && wf_type(ctx, T2)
-  case tp_or(T1, T2) => wf_type(ctx, T1) && wf_type(ctx, T2)
+    n>0 && exists S, U :: type_membership(n-1, ctx, s, p, L, concrete, S, U)
+  case tp_and(T1, T2) => n>0 && wf_type(n-1, ctx, s, T1) && wf_type(n-1, ctx, s, T2)
+  case tp_or(T1, T2) => n>0 && wf_type(n-1, ctx, s, T1) && wf_type(n-1, ctx, s, T2)
   case tp_top => true
   case tp_bot => true
 }
-copredicate wfe_type(ctx: context, T: tp)
+predicate wfe_type(n: nat, ctx: context, s: store, T: tp)
+  decreases n;
 {
-  wf_type(ctx, T) && exists Ds :: expansion(ctx, 0, T, Ds)
+  n>0 && wf_type(n-1, ctx, s, T) && exists Ds :: expansion(n-1, ctx, s, 0, T, Ds)
 }
-copredicate membership(ctx: context, t: tm, l: nat, d: decl)
+predicate membership(n: nat, ctx: context, s: store, t: tm, l: nat, d: decl)
+  decreases n;
 {
+  var z:nat := fresh_in_context(ctx);
   decl_label(d)==l &&
-  exists T :: typing(ctx, t, T) &&
-  forall z:nat :: !tp_fn(z, T) && z !in dom(ctx.m) && !tm_fn(z, t) ==>
+  n>0 && exists T, T' :: typing(n-1, ctx, s, t, T') &&
+  subtype(n-1, ctx, s, T', T) &&
   exists Ds ::
-  expansion(ctx, z, T, Ds) &&
+  expansion(n-1, ctx, s, z, T, Ds) &&
   ((Ds.decls_fin? &&
-     ((path(t) && exists d' :: d' in Ds.decls && d==decl_subst(z, t, d')) ||
-     (!path(t) && d in Ds.decls && !decl_fn(z, d)))) ||
+     ((path(t) && T'==T && exists d' :: d' in lst2seq(Ds.decls) && d==decl_subst(z, t, d')) ||
+      (!path(t) && d in lst2seq(Ds.decls) && !decl_fn(z, d)))) ||
    (Ds.decls_bot? && decl_bot(d)))
 }
-copredicate field_membership(ctx: context, t: tm, l: nat, T: tp)
+predicate field_membership(n: nat, ctx: context, s: store, t: tm, l: nat, T: tp)
+  decreases n;
 {
-  membership(ctx, t, l, decl_tm(l, T))
+  n>0 && membership(n-1, ctx, s, t, l, decl_tm(l, T))
 }
-copredicate method_membership(ctx: context, t: tm, m: nat, P: tp, R: tp)
+predicate method_membership(n: nat, ctx: context, s: store, t: tm, m: nat, P: tp, R: tp)
+  decreases n;
 {
-  exists d :: membership(ctx, t, m, d) &&
+  n>0 && exists d :: membership(n-1, ctx, s, t, m, d) &&
   d.decl_mt? && d.m==m && d.P==P && d.R==R
 }
-copredicate concrete_type_membership(ctx: context, t: tm, L: nat, S: tp, U: tp)
+predicate type_membership(n: nat, ctx: context, s: store, t: tm, L: nat, concrete: bool, S: tp, U: tp)
+  decreases n;
 {
-  exists d :: membership(ctx, t, L, d) &&
-  d.decl_tp_c? && d.Lc==L && d.Sc==S && d.Uc==U
+  n>0 && exists d :: membership(n-1, ctx, s, t, L, d) &&
+  d.decl_tp? && d.L==L && d.concrete==concrete && d.S==S && d.U==U
 }
-copredicate abstract_type_membership(ctx: context, t: tm, L: nat, S: tp, U: tp)
+predicate m_decl_seq_sorted(m: seq<pair<tp, decls>>)
 {
-  exists d :: membership(ctx, t, L, d) &&
-  d.decl_tp_a? && d.La==L && d.Sa==S && d.Ua==U
+  forall p :: p in m && p.snd.decls_fin? ==> decl_seq_sorted(lst2seq(p.snd.decls))
 }
-predicate m_decl_seq_sorted(m: partial_map<tp, decls>)
+function lookup<K,V>(k: K, m: seq<pair<K,V>>): option<V>
 {
-  match m
-  case Empty => true
-  case Extend(x, v, rest) => (v.decls_fin? ==> decl_seq_sorted(v.decls)) && m_decl_seq_sorted(rest)
+  if (exists v :: P(k,v) in m)
+  then (var v :| P(k, v) in m; Some(v))
+  else None
 }
-copredicate expansion(ctx: context, z: nat, T: tp, Ds: decls)
-  ensures expansion(ctx, z, T, Ds) && Ds.decls_fin? ==> decl_seq_sorted(Ds.decls);
+
+predicate expansion(n: nat, ctx: context, s: store, z: nat, T: tp, Ds: decls)
+  decreases n;
 {
-  expansion_iter(Empty, ctx, z, T, Ds)
+  n>0 && expansion_iter(n-1, [], ctx, s, z, T, Ds)
 }
-copredicate expansion_iter(m: partial_map<tp, decls>, ctx: context, z: nat, T: tp, Ds: decls)
-  requires m_decl_seq_sorted(m);
-  ensures expansion_iter(m, ctx, z, T, Ds) && Ds.decls_fin? ==> decl_seq_sorted(Ds.decls);
+predicate expansion_iter(n: nat, m: seq<pair<tp, decls>>, ctx: context, s: store, z: nat, T: tp, Ds: decls)
+  decreases n;
 {
   match T
   case tp_rfn(T', z', Ds') =>
-    exists DsT :: expansion_iter(m, ctx, z, T, DsT) &&
+    n>0 &&
+    exists DsT' :: expansion_iter(n-1, m, ctx, s, z, T', DsT') &&
     exists rfn_decls :: rfn_decls==decl_seq_sort(lst2seq(decls_subst(z', tm_var(z), Ds'))) &&
-    decl_seq_sorted(rfn_decls) &&
-    Ds==decls_and(decls_fin(rfn_decls), DsT) &&
-    (Ds.decls_fin? ==> decl_seq_sorted(Ds.decls))
-  case tp_sel_c(p, L) =>
-    (lookup(T, m).Some? && lookup(T, m).get==Ds && (Ds.decls_fin? ==> decl_seq_sorted(Ds.decls))) || 
-    (lookup(T, m).None? && exists S, U :: concrete_type_membership(ctx, p, L, S, U) && expansion_fix(T, decls_fin([]), m, ctx, z, U, Ds))
-  case tp_sel_a(p, L) =>
-    (lookup(T, m).Some? && lookup(T, m).get==Ds && (Ds.decls_fin? ==> decl_seq_sorted(Ds.decls))) || 
-    (lookup(T, m).None? && exists S, U :: abstract_type_membership(ctx, p, L, S, U) && expansion_fix(T, decls_fin([]), m, ctx, z, U, Ds))
+    Ds==decls_and(decls_fin(seq2lst(rfn_decls)), DsT')
+  case tp_sel(p, L, concrete) =>
+    (lookup(T, m).Some? && lookup(T, m).get==Ds) || 
+    (n>0 && lookup(T, m).None? && exists S, U :: type_membership(n-1, ctx, s, p, L, concrete, S, U) &&
+    expansion_fix(n-1, T, decls_fin(Nil), m, ctx, s, z, U, Ds))
   case tp_and(T1, T2) =>
-    exists Ds1, Ds2 :: expansion_iter(m, ctx, z, T1, Ds1) && expansion_iter(m, ctx, z, T2, Ds2) &&
-    Ds==decls_and(Ds1, Ds2) &&
-    (Ds.decls_fin? ==> decl_seq_sorted(Ds.decls))
+    n>0 &&
+    exists Ds1, Ds2 :: expansion_iter(n-1, m, ctx, s, z, T1, Ds1) &&
+                       expansion_iter(n-1, m, ctx, s, z, T2, Ds2) &&
+    Ds==decls_and(Ds1, Ds2)
   case tp_or(T1, T2) =>
-    exists Ds1, Ds2 :: expansion_iter(m, ctx, z, T1, Ds1) && expansion_iter(m, ctx, z, T2, Ds2) &&
-    Ds==decls_or(Ds1, Ds2) &&
-    (Ds.decls_fin? ==> decl_seq_sorted(Ds.decls))
-  case tp_top => Ds==decls_fin([])
+    n>0 &&
+    exists Ds1, Ds2 :: expansion_iter(n-1, m, ctx, s, z, T1, Ds1) &&
+                       expansion_iter(n-1, m, ctx, s, z, T2, Ds2) &&
+    Ds==decls_or(Ds1, Ds2)
+  case tp_top => Ds==decls_fin(Nil)
   case tp_bot => Ds==decls_bot
 }
-copredicate expansion_fix(selT: tp, selDs: decls, m: partial_map<tp, decls>, ctx: context, z: nat, T: tp, Ds: decls)
-  requires m_decl_seq_sorted(m);
-  requires selDs.decls_fin? ==> decl_seq_sorted(selDs.decls);
-  ensures expansion_fix(selT, selDs, m, ctx, z, T, Ds) && Ds.decls_fin? ==> decl_seq_sorted(Ds.decls);
+predicate expansion_fix(n: nat, selT: tp, selDs: decls, m: seq<pair<tp, decls>>, ctx: context, s: store, z: nat, T: tp, Ds: decls)
+  decreases n;
 {
-  (selDs==Ds && expansion_iter(Extend(selT, selDs, m), ctx, z, T, Ds)) ||
-  (selDs!=Ds && exists Da :: expansion_iter(Extend(selT, selDs, m), ctx, z, T, Da) &&
-   expansion_fix(selT, Da, m, ctx, z, T, Ds))
+  n>0 && (
+  (selDs==Ds && expansion_iter(n-1, [P(selT, selDs)]+m, ctx, s, z, T, Ds)) ||
+  (selDs!=Ds && exists Da :: expansion_iter(n-1, [P(selT, selDs)]+m, ctx, s, z, T, Da) &&
+   expansion_fix(n-1, selT, Da, m, ctx, s, z, T, Ds)))
 }
-copredicate decl_sub(ctx: context, d1: decl, d2: decl)
+predicate decl_sub(n: nat, ctx: context, s: store, d1: decl, d2: decl)
   requires decl_eq(d1, d2);
+  decreases n;
 {
   match d1
-  case decl_tp_c(L, S, U) => subtype(ctx, d2.Sc, S) && subtype(ctx, U, d2.Uc)
-  case decl_tp_a(L, S, U) => subtype(ctx, d2.Sa, S) && subtype(ctx, U, d2.Ua)
-  case decl_tm(l, U) => subtype(ctx, U, d2.T)
-  case decl_mt(m, S, U) => subtype(ctx, d2.P, S) && subtype(ctx, U, d2.R)
+  case decl_tp(L, S, U, concrete) => n>0 && subtype(n-1, ctx, s, d2.S, S) && subtype(n-1, ctx, s, U, d2.U)
+  case decl_tm(l, U) => n>0 && subtype(n-1, ctx, s, U, d2.T)
+  case decl_mt(m, S, U) => n>0 && subtype(n-1, ctx, s, d2.P, S) && subtype(n-1, ctx, s, U, d2.R)
 }
-copredicate decls_fin_sub(ctx: context, s1: seq<decl>, s2: seq<decl>)
-  requires decl_seq_sorted(s1);
-  requires decl_seq_sorted(s2);
+predicate decls_fin_sub(n: nat, ctx: context, s: store, s1: seq<decl>, s2: seq<decl>)
+  decreases n;
 {
   (s1 == [] && s2 == []) ||
-  (|s1|>0 && |s2|>0 && (
-  (decl_eq(s1[0], s2[0]) && decl_sub(ctx, s1[0], s2[0]) &&
-   decls_fin_sub(ctx, s1[1..], s2[1..])) ||
-  (decl_lt(s1[0], s2[0]) && decls_fin_sub(ctx, s1[1..], s2))))
+  (|s1|>0 && |s2|>0 && n>0 && (
+  (decl_eq(s1[0], s2[0]) && decl_sub(n-1, ctx, s, s1[0], s2[0]) &&
+   decls_fin_sub(n-1, ctx, s, s1[1..], s2[1..])) ||
+  (decl_lt(s1[0], s2[0]) && decls_fin_sub(n-1, ctx, s, s1[1..], s2))))
 }
-copredicate decls_sub(ctx: context, Ds1: decls, Ds2: decls)
-  requires Ds1.decls_fin? ==> decl_seq_sorted(Ds1.decls);
-  requires Ds2.decls_fin? ==> decl_seq_sorted(Ds2.decls);
+predicate decls_sub(n: nat, ctx: context, s: store, Ds1: decls, Ds2: decls)
+  decreases n;
 {
   match Ds1
   case decls_bot => true
   case decls_fin(s1) =>
     (match Ds2
      case decls_bot => false
-     case decls_fin(s2) => decls_fin_sub(ctx, s1, s2))
+     case decls_fin(s2) => n>0 && decls_fin_sub(n-1, ctx, s, lst2seq(s1), lst2seq(s2)))
 }
-copredicate subtype(ctx: context, S: tp, T: tp)
+predicate path_red(ctx: context, s: store, p1: tm, p2: tm)
 {
-  /* refl */    (S==T && wfe_type(ctx, T)) ||
-  /* <:-top */  (T.tp_top? && wfe_type(ctx, S)) ||
-  /* bot-<: */  (S.tp_bot? && wfe_type(ctx, T)) ||
-  /* <:-rfn */  (T.tp_rfn? && wfe_type(ctx, T) && subtype(ctx, S, T.base_tp) &&
-                 exists Ds' :: expansion(ctx, T.self, S, Ds') &&
-                 exists rfn_decls :: rfn_decls==decl_seq_sort(lst2seq(T.decls)) &&
-                 decl_seq_sorted(rfn_decls) &&
-                 decls_sub(Context(Extend(T.self, S, ctx.m)), decls_fin(rfn_decls), Ds')) ||
-  /* rfn-<: */  (S.tp_rfn? && wfe_type(ctx, S) && subtype(ctx, S.base_tp, T)) ||
-  /* <:-selc */ (T.tp_sel_c? &&
-                 exists S', U' :: concrete_type_membership(ctx, T.pc, T.Lc, S', U') &&
-                 subtype(ctx, S', U') && subtype(ctx, S, S')) ||
-  /* selc-<: */ (S.tp_sel_c? &&
-                 exists S', U' :: concrete_type_membership(ctx, S.pc, S.Lc, S', U') &&
-                 subtype(ctx, S', U') && subtype(ctx, U', T)) ||
-  /* <:-sela */ (T.tp_sel_a? &&
-                 exists S', U' :: abstract_type_membership(ctx, T.pa, T.La, S', U') &&
-                 subtype(ctx, S', U') && subtype(ctx, S, S')) ||
-  /* sela-<: */ (S.tp_sel_a? &&
-                 exists S', U' :: abstract_type_membership(ctx, S.pa, S.La, S', U') &&
-                 subtype(ctx, S', U') && subtype(ctx, U', T)) ||
-  /* <:-and */  (T.tp_and? && subtype(ctx, S, T.and1) && subtype(ctx, S, T.and2)) ||
-  /* and1-<: */ (S.tp_and? && wfe_type(ctx, S.and2) && subtype(ctx, S.and1, T)) ||
-  /* and2-<: */ (S.tp_and? && wfe_type(ctx, S.and1) && subtype(ctx, S.and2, T)) ||
-  /* <:-or1 */  (T.tp_or? && wfe_type(ctx, T.or2) && subtype(ctx, S, T.or1)) ||
-  /* <:-or2 */  (T.tp_or? && wfe_type(ctx, T.or1) && subtype(ctx, S, T.or2)) ||
-  /* or-<: */   (S.tp_or? && subtype(ctx, S.or1, T) && subtype(ctx, S.or2, T))
+  path(p1) && path(p2) && (
+  (p1.tm_sel? && p1.t.tm_loc? && p2.tm_loc? && p1.t.loc < |s.m| &&
+   def_field_lookup(p1.l, store_lookup(p1.t.loc, s)).Some? &&
+   p2==def_field_lookup(p1.l, store_lookup(p1.t.loc, s)).get) ||
+  (p1.tm_sel? && p2.tm_sel? && p1.l==p2.l && path_red(ctx, s, p1.t, p2.t)))
 }
 
-// ### Properties of typing judgments ###
-
-ghost method lemma_field_mem__expansion_decl(ctx: context, t1: tm, T1: tp, l: nat, T: tp, ctx': context, z: nat, Ds: decls)
-  requires field_membership(ctx, t1, l, T);
-  requires typing(ctx, t1, T1);
-  requires expansion(ctx', z, T1, Ds) && Ds.decls_fin?;
-  ensures exists U :: decl_tm(l, U) in Ds.decls;
+predicate subtype(n: nat, ctx: context, s: store, S: tp, T: tp)
+  decreases n;
 {
-  assume exists U :: decl_tm(l, U) in Ds.decls; // TODO...
+  var self := fresh_in_context(ctx);
+  n>0 && (
+  /* refl */    S==T ||
+  /* <:-top */  T.tp_top? ||
+  /* bot-<: */  S.tp_bot? ||
+  /* <:-rfn */  (T.tp_rfn? && subtype(n-1, ctx, s, S, T.base_tp) &&
+                 exists Ds' :: expansion(n-1, ctx, s, self, S, Ds') &&
+                 exists rfn_decls :: rfn_decls==decl_seq_sort(lst2seq(decls_subst(T.self, tm_var(self), T.decls))) &&
+                 decls_sub(n-1, context_extend(ctx, self, S), s, decls_fin(seq2lst(rfn_decls)), Ds')) ||
+  /* rfn-<: */  (S.tp_rfn? && subtype(n-1, ctx, s, S.base_tp, T)) ||
+  /* <:-sel */  (T.tp_sel? &&
+                 exists S', U' :: type_membership(n-1, ctx, s, T.p, T.L, T.concrete, S', U') &&
+                 subtype(n-1, ctx, s, S', U') && subtype(n-1, ctx, s, S, S')) ||
+  /* sel-<: */  (S.tp_sel? &&
+                 exists S', U' :: type_membership(n-1, ctx, s, S.p, S.L, S.concrete, S', U') &&
+                 subtype(n-1, ctx, s, S', U') && subtype(n-1, ctx, s, U', T)) ||
+  /* <:-and */  (T.tp_and? && subtype(n-1, ctx, s, S, T.and1) && subtype(n-1, ctx, s, S, T.and2)) ||
+  /* and1-<: */ (S.tp_and? && subtype(n-1, ctx, s, S.and1, T)) ||
+  /* and2-<: */ (S.tp_and? && subtype(n-1, ctx, s, S.and2, T)) ||
+  /* <:-or1 */  (T.tp_or? && subtype(n-1, ctx, s, S, T.or1)) ||
+  /* <:-or2 */  (T.tp_or? && subtype(n-1, ctx, s, S, T.or2)) ||
+  /* or-<: */   (S.tp_or? && subtype(n-1, ctx, s, S.or1, T) && subtype(n-1, ctx, s, S.or2, T)) ||
+  /* pathred */ (T.tp_sel? && exists p :: path_red(ctx, s, T.p, p) &&
+                 subtype(n-1, ctx, s, S, tp_sel(p, T.L, T.concrete))))
 }
 
-// -----------------
-// Logical Relations
-// -----------------
-
-predicate V(T: tp, t: tm, k: nat, ctx: context, s: store)
-  requires A(k, ctx, s);
-  decreases k, k; // weird!
+predicate typing'(ctx: context, s: store, t: tm, T: tp)
 {
-  t.tm_var? && t.x in dom(s.m) &&
-  wfe_type(ctx, T) &&
-  (exists Tc, init :: P(Tc, init) == lookup(t.x, s.m).get) &&
-  (exists Ds :: expansion(ctx, t.x, T, Ds) && Ds.decls_fin?) &&
-  forall Tc, init :: P(Tc, init) == lookup(t.x, s.m).get ==>
-  forall Ds :: expansion(ctx, t.x, T, Ds) && Ds.decls_fin? ==>
-  forall j:nat :: j<k ==> (
-    (forall Li:nat, S, U :: decl_tp_c(Li, S, U) in Ds.decls ==>
-     exists S', U' :: concrete_type_membership(ctx, t, Li, S', U') &&
-     subtype(ctx, S, S') && subtype(ctx, S', U') && subtype(ctx, U', U)) &&
-    (forall Li:nat, S, U :: decl_tp_a(Li, S, U) in Ds.decls ==>
-     exists S', U' :: abstract_type_membership(ctx, t, Li, S', U') &&
-     subtype(ctx, S, S') && subtype(ctx, S', U') && subtype(ctx, U', U)) &&
-    (forall mi:nat, S, U :: decl_mt(mi, S, U) in Ds.decls ==>
-     exists xi, ti :: def_method_lookup(mi, init) == Some(P(xi, ti)) &&
-     E(U, ti, j, ctx_extend(xi, S, ctx), s, ctx)) &&
-    (forall li:nat, U :: decl_tm(li, U) in Ds.decls ==>
-     def_field_lookup(li, init).Some? &&
-     V(U, def_field_lookup(li, init).get, j, ctx, s))
-  )
+  exists n:nat :: typing(n, ctx, s, t, T)
+}
+predicate wf_init'(already_in_store: bool, ctx: context, s: store, decls: seq<decl>, defs: seq<def>)
+{
+  exists n:nat :: wf_init(n, already_in_store, ctx, s, decls, defs)
+}
+predicate wfe_type'(ctx: context, s: store, T: tp)
+{
+  exists n:nat :: wfe_type(n, ctx, s, T)
+}
+predicate membership'(ctx: context, s: store, t: tm, l: nat, d: decl)
+{
+  exists n:nat :: membership(n, ctx, s, t, l, d)
+}
+predicate field_membership'(ctx: context, s: store, t: tm, l: nat, T: tp)
+{
+  exists n:nat :: field_membership(n, ctx, s, t, l, T)
+}
+predicate method_membership'(ctx: context, s: store, t: tm, m: nat, P: tp, R: tp)
+{
+  exists n:nat :: method_membership(n, ctx, s, t, m, P, R)
+}
+predicate expansion'(ctx: context, s: store, z: nat, T: tp, Ds: decls)
+{
+  exists n:nat :: expansion(n, ctx, s, z, T, Ds)
+}
+predicate decl_sub'(ctx: context, s: store, d1: decl, d2: decl)
+  requires decl_eq(d1, d2);
+{
+  exists n:nat :: decl_sub(n, ctx, s, d1, d2)
+}
+predicate subtype'(ctx: context, s: store, S: tp, T: tp)
+{
+  exists n:nat :: subtype(n, ctx, s, S, T)
 }
 
-predicate E(T: tp, t: tm, k: nat, ctx: context, s: store, ctx_prev: context)
-  requires A(k, ctx_prev, s);
-  requires As(k, ctx, s, ctx_prev);
-  decreases k;
+// ### Properties about typing-related judgments ###
+function typing_n(ctx: context, s: store, t: tm, T: tp): nat
+  requires typing'(ctx, s, t, T);
+  ensures typing(typing_n(ctx, s, t, T), ctx, s, t, T);
 {
-  k==0 || (
-  forall i:nat, j:nat :: i+j<k ==>
-  forall ctx', s':store :: Xs(ctx', s', k-1, ctx, s, ctx_prev) && A(k-1, ctx', s') ==>
-  forall t', s'':store :: prefix_of(s''.m, s'.m) && mstep(t, s', t', s'', j) && irred(t', s'') ==>
-  forall ctx'' :: Xc(ctx'', k-1, ctx', s'', s') && A(k-1, ctx'', s'') ==>
-  V(T, t', i, ctx'', s'')
-  )
+  var n:nat :| typing(n, ctx, s, t, T); n
+}
+function wf_init_n(already_in_store: bool, ctx: context, s: store, decls: seq<decl>, defs: seq<def>): nat
+  requires wf_init'(already_in_store, ctx, s, decls, defs);
+  ensures wf_init(wf_init_n(already_in_store, ctx, s, decls, defs), already_in_store, ctx, s, decls, defs);
+{
+  var n:nat :| wf_init(n, already_in_store, ctx, s, decls, defs); n
+}
+function wfe_type_n(ctx: context, s: store, T: tp): nat
+  requires wfe_type'(ctx, s, T);
+  ensures wfe_type(wfe_type_n(ctx, s, T), ctx, s, T);
+{
+  var n:nat :| wfe_type(n, ctx, s, T); n
+}
+function field_membership_n(ctx: context, s: store, t: tm, l: nat, T: tp): nat
+  requires field_membership'(ctx, s, t, l, T);
+  ensures field_membership(field_membership_n(ctx, s, t, l, T), ctx, s, t, l, T);
+{
+  var n:nat :| field_membership(n, ctx, s, t, l, T); n
+}
+function method_membership_n(ctx: context, s: store, t: tm, m: nat, P: tp, R: tp): nat
+  requires method_membership'(ctx, s, t, m, P, R);
+  ensures method_membership(method_membership_n(ctx, s, t, m, P, R), ctx, s, t, m, P, R);
+{
+  var n:nat :| method_membership(n, ctx, s, t, m, P, R); n
+}
+function expansion_n(ctx: context, s: store, z: nat, T: tp, Ds: decls): nat
+  requires expansion'(ctx, s, z, T, Ds);
+  ensures expansion(expansion_n(ctx, s, z, T, Ds), ctx, s, z, T, Ds);
+{
+  var n:nat :| expansion(n, ctx, s, z, T, Ds); n
+}
+function subtype_n(ctx: context, s: store, S: tp, T: tp): nat
+  requires subtype'(ctx, s, S, T);
+  ensures subtype(subtype_n(ctx, s, S, T), ctx, s, S, T);
+{
+  var n:nat :| subtype(n, ctx, s, S, T); n
 }
 
-predicate A(k: nat, ctx: context, s: store)
+ghost method lemma_typing_monotonic(n: nat, ctx: context, s: store, t: tm, T: tp)
+  requires typing(n, ctx, s, t, T);
+  ensures typing(n+1, ctx, s, t, T);
 {
-  dom(ctx.m) == dom(s.m)
-}
-predicate As(k: nat, ctx: context, s: store, ctx_prev: context)
-{
-  prefix_of(ctx.m, ctx_prev.m) && A(k, ctx_prev, s)
-}
-predicate Ac(k: nat, ctx: context, s: store, s_prev: store)
-{
-  prefix_of(s.m, s_prev.m) && A(k, ctx, s_prev)
-}
-predicate Xs(ctx': context, s': store, k: nat, ctx: context, s: store, ctx_prev: context)
-  requires As(k, ctx, s, ctx_prev);
-  decreases k;
-{
-  A(k, ctx', s') && As(k, ctx', s, ctx_prev) && Ac(k, ctx_prev, s', s) && (
-  forall x:nat :: lookup(x, ctx.m).Some? ==>
-    lookup(x, ctx'.m)==Some(lookup(x, ctx.m).get) && V(lookup(x, ctx.m).get, tm_var(x), k, ctx', s'))
-}
-predicate Xc(ctx': context, k: nat, ctx: context, s: store, s_prev: store)
-  requires Ac(k, ctx, s, s_prev);
-{
-  var s_todo := map_complement(s.m, s_prev.m, Empty);
-  var tp_todo := map_fst(s_todo);
-  ctx'.m==build(ctx.m, tp_todo)
-}
+  if (t.tm_var?) {
+    assert typing(n+1, ctx, s, t, T);
+  } else if (t.tm_new?) {
+    if (n>0) {
+      var y := fresh_from(dom(ctx)+tm_vars(t));
+      var init := defs_subst(t.y, tm_var(y), t.init);
+      var t' := tm_subst(t.y, tm_var(y), t.t');
+      var Ds:decls :| Ds.decls_fin? &&
+      wfe_type(n-1, ctx, s, t.Tc) &&
+      expansion(n-1, ctx, s, y, t.Tc, Ds) && 
+      wf_init(n-1, false, context_extend(ctx, y, t.Tc), s, lst2seq(Ds.decls), lst2seq(init)) &&
+      !tp_fn(y, T) &&
+      exists T' :: typing(n-1, context_extend(ctx, y, t.Tc), s, t', T') &&
+      subtype(n-1, context_extend(ctx, y, t.Tc), s, T', T);
 
-predicate R(ctx: context, t: tm, T: tp)
-{
-  forall k: nat ::
-      A(k, Context(Empty), Store(Empty)) &&
-      As(k, ctx, Store(Empty), Context(Empty)) &&
-      E(T, t, k, ctx, Store(Empty), Context(Empty))
-}
+      var T':tp :| typing(n-1, context_extend(ctx, y, t.Tc), s, t', T') &&
+      subtype(n-1, context_extend(ctx, y, t.Tc), s, T', T);
 
-// ### Lemmas about logical relations ###
-ghost method lemma_A_monotonic(k: nat, j: nat, ctx: context, s: store)
-  requires A(k, ctx, s);
-  requires j <= k;
-  ensures A(j, ctx, s);
-{
-}
-ghost method lemma_As_monotononic(k: nat, j: nat, ctx: context, s: store, ctx_prev: context)
-  requires As(k, ctx, s, ctx_prev);
-  requires j <= k;
-  ensures As(j, ctx, s, ctx_prev);
-{
-}
-ghost method lemma_Ac_monotononic(k: nat, j: nat, ctx: context, s: store, s_prev: store)
-  requires Ac(k, ctx, s, s_prev);
-  requires j <= k;
-  ensures Ac(j, ctx, s, s_prev);
-{
-}
-ghost method lemma_Xs_monotonic(ctx': context, s': store, k: nat, j: nat, ctx: context, s: store, ctx_prev: context)
-  requires As(k, ctx, s, ctx_prev);
-  requires As(j, ctx, s, ctx_prev);
-  requires Xs(ctx', s', k, ctx, s, ctx_prev);
-  requires j <= k;
-  ensures Xs(ctx', s', j, ctx, s, ctx_prev);
-{
-  forall (x:nat | lookup(x, ctx.m).Some?)
-    ensures lookup(x, ctx'.m)==Some(lookup(x, ctx.m).get) && V(lookup(x, ctx.m).get, tm_var(x), j, ctx', s');
-  {
-    lemma_V_monotonic(lookup(x, ctx.m).get, tm_var(x), k, j, ctx', s');
+      lemma_wfe_type_monotonic(n-1, ctx, s, t.Tc);
+      lemma_expansion_monotonic(n-1, ctx, s, y, t.Tc, Ds); 
+      lemma_wf_init_monotonic(n-1, false, context_extend(ctx, y, t.Tc), s, lst2seq(Ds.decls), lst2seq(init));
+      lemma_typing_monotonic(n-1, context_extend(ctx, y, t.Tc), s, t', T');
+      lemma_subtype_monotonic(n-1, context_extend(ctx, y, t.Tc), s, T', T);
+    }
+  } else if (t.tm_sel?) {
+    if (n>0) {
+      lemma_field_membership_monotonic(n-1, ctx, s, t.t, t.l, T);
+    }
+  } else if (t.tm_msel?) {
+    if (n>0) {
+      var S, T' :| method_membership(n-1, ctx, s, t.o, t.m, S, T) &&
+      typing(n-1, ctx, s, t.a, T') &&
+      subtype(n-1, ctx, s, T', S);
+
+      lemma_method_membership_monotonic(n-1, ctx, s, t.o, t.m, S, T);
+      lemma_typing_monotonic(n-1, ctx, s, t.a, T');
+      lemma_subtype_monotonic(n-1, ctx, s, T', S);
+
+      assert method_membership(n, ctx, s, t.o, t.m, S, T) &&
+      typing(n, ctx, s, t.a, T') &&
+      subtype(n, ctx, s, T', S);
+
+      helper_assert_exists_method_membership(n, ctx, s, t, T, S, T');
+    }
   }
 }
-ghost method lemma_Xc_monotonic(ctx': context, k: nat, j: nat, ctx: context, s: store, s_prev: store)
-  requires Ac(k, ctx, s, s_prev);
-  requires Ac(j, ctx, s, s_prev);
-  requires Xc(ctx', k, ctx, s, s_prev);
-  requires j <= k;
-  ensures Xc(ctx', j, ctx, s, s_prev);
+ghost method helper_assert_exists_method_membership(n: nat, ctx: context, s: store, t: tm, T: tp, S: tp, T': tp)
+  requires t.tm_msel?;
+  requires method_membership(n, ctx, s, t.o, t.m, S, T) &&
+      typing(n, ctx, s, t.a, T') &&
+      subtype(n, ctx, s, T', S);
+  ensures exists S, T' :: method_membership(n, ctx, s, t.o, t.m, S, T) &&
+      typing(n, ctx, s, t.a, T') &&
+      subtype(n, ctx, s, T', S);
 {
 }
-ghost method lemma_V_monotonic(T: tp, t: tm, k: nat, j: nat, ctx: context, s: store)
-  requires A(k, ctx, s);
-  requires A(j, ctx, s);
-  requires V(T, t, k, ctx, s);
-  requires j <= k;
-  ensures V(T, t, j, ctx, s);
+ghost method lemma_wf_init_monotonic(n: nat, already_in_store: bool, ctx: context, s: store, decls: seq<decl>, defs: seq<def>)
+  requires wf_init(n, already_in_store, ctx, s, decls, defs);
+  ensures wf_init(n+1, already_in_store, ctx, s, decls, defs);
 {
-  assume V(T, t, j, ctx, s); // TODO... but really follows from def.
+  assume wf_init(n+1, already_in_store, ctx, s, decls, defs); // TODO
+}
+ghost method lemma_wfe_type_monotonic(n: nat, ctx: context, s: store, T: tp)
+  requires wfe_type(n, ctx, s, T);
+  ensures wfe_type(n+1, ctx, s, T);
+{
+  assume wfe_type(n+1, ctx, s, T); // TODO
+}
+ghost method lemma_field_membership_monotonic(n: nat, ctx: context, s: store, t: tm, l: nat, T: tp)
+  requires field_membership(n, ctx, s, t, l, T);
+  ensures field_membership(n+1, ctx, s, t, l, T);
+{
+  assume field_membership(n+1, ctx, s, t, l, T); // TODO
+}
+ghost method lemma_method_membership_monotonic(n: nat, ctx: context, s: store, t: tm, m: nat, P: tp, R: tp)
+  requires method_membership(n, ctx, s, t, m, P, R);
+  ensures method_membership(n+1, ctx, s, t, m, P, R);
+{
+  assume method_membership(n+1, ctx, s, t, m, P, R); // TODO
+}
+ghost method lemma_expansion_monotonic(n: nat, ctx: context, s: store, z: nat, T: tp, Ds: decls)
+  requires expansion(n, ctx, s, z, T, Ds);
+  ensures expansion(n+1, ctx, s, z, T, Ds);
+{
+  assume expansion(n+1, ctx, s, z, T, Ds); // TODO
+}
+ghost method lemma_subtype_monotonic(n: nat, ctx: context, s: store, S: tp, T: tp)
+  requires subtype(n, ctx, s, S, T);
+  ensures subtype(n+1, ctx, s, S, T);
+{
+  assume subtype(n+1, ctx, s, S, T); // TODO
 }
 
-ghost method lemma_V_value(T: tp, t: tm, k: nat, ctx: context, s: store)
-  requires A(k, ctx, s);
-  requires V(T, t, k, ctx, s);
-  ensures value(t);
+// ----------
+// Properties
+// ----------
+
+predicate store_extends<A>(s': store, s: store)
+{
+  |s.m|<=|s'.m| && forall l:nat :: l < |s.m| ==> s.m[l]==s'.m[l]
+}
+predicate store_well_typed1(s: store, loc: nat, y: nat, Tc: tp, init: seq<def>)
+{
+    exists n:nat :: n>0 &&
+    is_concrete(Tc) &&
+    exists Ds:decls :: Ds.decls_fin? &&
+    wfe_type(n-1, Context([]), s, Tc) &&
+    expansion(n-1, Context([]), s, y, Tc, Ds) && 
+    wf_init(n-1, true, Context([]), s, lst2seq(decls_subst(y, tm_loc(loc), Ds.decls)), def_seq_sort(init))
+}
+predicate store_well_typed(s: store)
+{
+  forall l:nat :: l < |s.m| ==> store_well_typed1(s, l, fresh_from([]), store_lookup_type(l, s), store_lookup(l, s))
+}
+ghost method lemma_store_invariance_typing(n: nat, ctx: context, s: store, s': store, t: tm, T: tp)
+  requires store_extends(s', s);
+  requires typing(n, ctx, s, t, T);
+  ensures typing(n, ctx, s', t, T);
+  decreases n;
+{
+  if (t.tm_sel?) {
+    lemma_store_invariance_membership(n-2, ctx, s, s', t.t, t.l, decl_tm(t.l, T));
+  } else if (t.tm_msel?) {
+    var S, T' :| method_membership(n-1, ctx, s, t.o, t.m, S, T) &&
+    typing(n-1, ctx, s, t.a, T') &&
+    subtype(n-1, ctx, s, T', S);
+    lemma_store_invariance_membership(n-2, ctx, s, s', t.o, t.m, decl_mt(t.m, S, T));
+    lemma_store_invariance_typing(n-1, ctx, s, s', t.a, T');
+    lemma_store_invariance_subtype(n-1, ctx, s, s', T', S);
+    assert method_membership(n-1, ctx, s', t.o, t.m, S, T) &&
+    typing(n-1, ctx, s', t.a, T') &&
+    subtype(n-1, ctx, s', T', S);
+    helper_assert_exists_method_membership(n-1, ctx, s', t, T, S, T');
+  } else if (t.tm_new?) {
+    var y := fresh_from(dom(ctx)+tm_vars(t));
+    var init := defs_subst(t.y, tm_var(y), t.init);
+    var t' := tm_subst(t.y, tm_var(y), t.t');
+    var Ds:decls, T' :| Ds.decls_fin? &&
+    wfe_type(n-1, ctx, s, t.Tc) &&
+    expansion(n-1, ctx, s, y, t.Tc, Ds) && 
+    wf_init(n-1, false, context_extend(ctx, y, t.Tc), s, lst2seq(Ds.decls), lst2seq(init)) &&
+    !tp_fn(y, T) &&
+    typing(n-1, context_extend(ctx, y, t.Tc), s, t', T') &&
+    subtype(n-1, context_extend(ctx, y, t.Tc), s, T', T);
+    lemma_store_invariance_wfe_type(n-1, ctx, s, s', t.Tc);
+    lemma_store_invariance_expansion(n-1, ctx, s, s', y, t.Tc, Ds); 
+    lemma_store_invariance_wf_init(n-1, false, context_extend(ctx, y, t.Tc), s, s', lst2seq(Ds.decls), lst2seq(init));
+    lemma_store_invariance_typing(n-1, context_extend(ctx, y, t.Tc), s, s', t', T');
+    lemma_store_invariance_subtype(n-1, context_extend(ctx, y, t.Tc), s, s', T', T);
+    assert Ds.decls_fin? &&
+    wfe_type(n-1, ctx, s', t.Tc) &&
+    expansion(n-1, ctx, s', y, t.Tc, Ds) && 
+    wf_init(n-1, false, context_extend(ctx, y, t.Tc), s', lst2seq(Ds.decls), lst2seq(init)) &&
+    !tp_fn(y, T) &&
+    typing(n-1, context_extend(ctx, y, t.Tc), s', t', T') &&
+    subtype(n-1, context_extend(ctx, y, t.Tc), s', T', T);
+    helper_assert_exists_new(n-1, ctx, s', t, y, init, t', T, Ds, T');
+  } else {
+  }
+}
+ghost method helper_assert_exists_new(n: nat, ctx: context, s: store, t: tm,  y: nat, init: list<def>, t': tm, T: tp, Ds: decls, T': tp)
+  requires t.tm_new?;
+  requires context_lookup(ctx, y).None?;
+  requires Ds.decls_fin? &&
+    wfe_type(n, ctx, s, t.Tc) &&
+    expansion(n, ctx, s, y, t.Tc, Ds) && 
+    wf_init(n, false, context_extend(ctx, y, t.Tc), s, lst2seq(Ds.decls), lst2seq(init)) &&
+    !tp_fn(y, T) &&
+    typing(n, context_extend(ctx, y, t.Tc), s, t', T') &&
+    subtype(n, context_extend(ctx, y, t.Tc), s, T', T);
+  ensures exists Ds:decls, T' :: Ds.decls_fin? &&
+    wfe_type(n, ctx, s, t.Tc) &&
+    expansion(n, ctx, s, y, t.Tc, Ds) && 
+    wf_init(n, false, context_extend(ctx, y, t.Tc), s, lst2seq(Ds.decls), lst2seq(init)) &&
+    !tp_fn(y, T) &&
+    typing(n, context_extend(ctx, y, t.Tc), s, t', T') &&
+    subtype(n, context_extend(ctx, y, t.Tc), s, T', T);
 {
 }
-ghost method lemma_V_field(T1: tp, t1: tm, l: nat, T: tp, k: nat, j: nat, ctx1: context, s1: store, Tc: tp, init: list<def>, Ds: decls)
-  requires A(k, ctx1, s1);
-  requires V(T1, t1, k, ctx1, s1);
-  requires t1.tm_var?;
-  requires P(Tc, init) == lookup(t1.x, s1.m).get;
-  requires expansion(ctx1, t1.x, T1, Ds) && Ds.decls_fin?;
-  requires decl_tm(l, T) in Ds.decls;
-  requires j<k;
-  ensures def_field_lookup(l, init).Some? && V(T, def_field_lookup(l, init).get, j, ctx1, s1);
+ghost method lemma_store_invariance_membership(n: nat, ctx: context, s: store, s': store, t: tm, l: nat, d: decl)
+  requires store_extends(s', s);
+  requires membership(n, ctx, s, t, l, d);
+  ensures membership(n, ctx, s', t, l, d);
 {
-  // TODO...
-  assume def_field_lookup(l, init).Some? && V(T, def_field_lookup(l, init).get, j, ctx1, s1);
+  assume membership(n, ctx, s', t, l, d); // TODO
+}
+ghost method lemma_store_invariance_subtype(n: nat, ctx: context, s: store, s': store, S: tp, T: tp)
+  requires store_extends(s', s);
+  requires subtype(n, ctx, s, S, T);
+  ensures subtype(n, ctx, s', S, T);
+{
+  assume subtype(n, ctx, s', S, T); // TODO
+}
+ghost method lemma_store_invariance_wfe_type(n: nat, ctx: context, s: store, s': store, T: tp)
+  requires store_extends(s', s);
+  requires wfe_type(n, ctx, s, T);
+  ensures wfe_type(n, ctx, s', T);
+{
+  assume wfe_type(n, ctx, s', T); // TODO
+}
+ghost method lemma_store_invariance_expansion(n: nat, ctx: context, s: store, s': store, z: nat, T: tp, Ds: decls)
+  requires store_extends(s', s);
+  requires expansion(n, ctx, s, z, T, Ds);
+  ensures expansion(n, ctx, s', z, T, Ds);
+{
+  assume expansion(n, ctx, s', z, T, Ds);
+}
+ghost method lemma_store_invariance_wf_init(n: nat, already_in_store: bool, ctx: context, s: store, s': store, decls: seq<decl>, defs: seq<def>)
+  requires store_extends(s', s);
+  requires wf_init(n, already_in_store, ctx, s, decls, defs);
+  ensures wf_init(n, already_in_store, ctx, s', decls, defs);
+{
+  assume wf_init(n, already_in_store, ctx, s', decls, defs);
+}
+ghost method lemma_store_invariance_well_typed1(s: store, s': store, loc: nat, y: nat, Tc: tp, init: seq<def>)
+  requires store_extends(s', s);
+  requires store_well_typed1(s, loc, y, Tc, init);
+  ensures store_well_typed1(s', loc, y, Tc, init);
+{
+  var n:nat, Ds:decls :| n>0 &&
+    is_concrete(Tc) &&
+    Ds.decls_fin? &&
+    wfe_type(n-1, Context([]), s, Tc) &&
+    expansion(n-1, Context([]), s, y, Tc, Ds) && 
+    wf_init(n-1, true, Context([]), s, lst2seq(decls_subst(y, tm_loc(loc), Ds.decls)), def_seq_sort(init));
+  lemma_store_invariance_wfe_type(n-1, Context([]), s, s', Tc);
+  lemma_store_invariance_expansion(n-1, Context([]), s, s', y, Tc, Ds); 
+  lemma_store_invariance_wf_init(n-1, true, Context([]), s, s', lst2seq(decls_subst(y, tm_loc(loc), Ds.decls)), def_seq_sort(init));
+  assert n>0 &&
+    is_concrete(Tc) &&
+    Ds.decls_fin? &&
+    wfe_type(n-1, Context([]), s', Tc) &&
+    expansion(n-1, Context([]), s', y, Tc, Ds) && 
+    wf_init(n-1, true, Context([]), s', lst2seq(decls_subst(y, tm_loc(loc), Ds.decls)), def_seq_sort(init));
+  helper_assert_exists_store_well_typed1(s', loc, y, Tc, init, n, Ds);
+}
+ghost method helper_assert_exists_store_well_typed1(s: store, loc: nat, y: nat, Tc: tp, init: seq<def>, n: nat, Ds: decls)
+  requires n>0 &&
+    is_concrete(Tc) &&
+    Ds.decls_fin? &&
+    wfe_type(n-1, Context([]), s, Tc) &&
+    expansion(n-1, Context([]), s, y, Tc, Ds) && 
+    wf_init(n-1, true, Context([]), s, lst2seq(decls_subst(y, tm_loc(loc), Ds.decls)), def_seq_sort(init));
+  ensures exists n:nat, Ds:decls :: n>0 &&
+    is_concrete(Tc) &&
+    Ds.decls_fin? &&
+    wfe_type(n-1, Context([]), s, Tc) &&
+    expansion(n-1, Context([]), s, y, Tc, Ds) && 
+    wf_init(n-1, true, Context([]), s, lst2seq(decls_subst(y, tm_loc(loc), Ds.decls)), def_seq_sort(init));
+{
 }
 
-ghost method lemma_E(T: tp, t: tm, t': tm, k: nat, j: nat, i: nat,
-  s: store, s': store, s'': store,
-  ctx_prev: context, ctx: context, ctx': context, ctx'': context)
-  requires A(k, ctx_prev, s);
-  requires As(k, ctx, s, ctx_prev);
-  requires E(T, t, k, ctx, s, ctx_prev);
-  requires i+j<k;
-  requires Xs(ctx', s', k-1, ctx, s, ctx_prev) && A(k-1, ctx', s');
-  requires prefix_of(s''.m, s'.m) && mstep(t, s', t', s'', j);
-  requires Xc(ctx'', k-1, ctx', s'', s') && A(k-1, ctx'', s'');
-  ensures irred(t', s'') ==> V(T, t', i, ctx'', s'');
+ghost method lemma_store_extends_well_typed(s: store, s': store, Tc: tp, init: seq<def>)
+  requires store_well_typed(s);
+  requires s'==Store(s.m+[P(Tc, init)]);
+  requires store_well_typed1(s', |s.m|, fresh_from([]), Tc, init);
+  ensures store_extends(s', s);
+  ensures store_well_typed(s');
 {
-}
-
-ghost method lemma_Xs_lookup(x: nat, T: tp, ctx': context, s': store, k: nat, ctx: context, s: store, ctx_prev: context)
-  requires As(k, ctx, s, ctx_prev);
-  requires Xs(ctx', s', k, ctx, s, ctx_prev);
-  requires lookup(x, ctx.m) == Some(T);
-  ensures V(T, tm_var(x), k, ctx', s');
-{
-}
-ghost method lemma_unchanged_Xc(ctx': context, k: nat, ctx: context, s: store, s_prev: store)
-  requires Ac(k, ctx, s, s_prev);
-  requires Xc(ctx', k, ctx, s, s_prev);
-  requires s==s_prev;
-  ensures ctx'==ctx;
-{
-}
-ghost method lemma_Xc_unique(ctx2: context, ctx1: context, k: nat, ctx: context, s: store, s_prev: store)
-  requires Ac(k, ctx, s, s_prev);
-  requires Xc(ctx1, k, ctx, s, s_prev);
-  requires Xc(ctx2, k, ctx, s, s_prev);
-  ensures ctx1==ctx2;
-{
-}
-ghost method build_Xc(k: nat, ctx: context, s: store, s_prev: store) returns (ctx': context)
-  requires Ac(k, ctx, s, s_prev);
-  ensures Xc(ctx', k, ctx, s, s_prev);
-  ensures A(k, ctx', s);
-{
-  var s_todo := map_complement(s.m, s_prev.m, Empty);
-  lemma_map_complement__dom(s.m, s_prev.m);
-  assert  dom(s.m)==rev(dom(s_todo))+dom(s_prev.m);
-
-  var tp_todo := map_fst(s_todo);
-  assert  dom(s.m)==rev(dom(tp_todo))+dom(s_prev.m);
-
-  ctx' := Context(build(ctx.m, tp_todo));
-  lemma_build__dom(ctx.m, tp_todo);
-}
-
-ghost method theorem_fundamental_R_var(ctx: context, T: tp, x: nat, k: nat)
-  requires typing(ctx, tm_var(x), T);
-  requires A(k, Context(Empty), Store(Empty));
-  requires As(k, ctx, Store(Empty), Context(Empty));
-  ensures E(T, tm_var(x), k, ctx, Store(Empty), Context(Empty));
-{
-  var ctx_prev := Context(Empty);
-  var s := Store(Empty);
-  var t := tm_var(x);
-
-      assert lookup(x, ctx.m) == Some(T);
-      if (k>0) {
-        forall (
-          i:nat, j:nat,
-          ctx', s':store,
-          t', s'':store,
-          ctx'' |
-          i+j<k &&
-          Xs(ctx', s', k-1, ctx, s, ctx_prev) && A(k-1, ctx', s') &&
-          prefix_of(s''.m, s'.m) && mstep(t, s', t', s'', j) && irred(t', s'') &&
-          Xc(ctx'', k-1, ctx', s'', s') && A(k-1, ctx'', s''))
-          ensures V(T, t', i, ctx'', s'');
-       {
-         assert j==0;
-         assert t'==t;
-         assert s''==s';
-         lemma_unchanged_Xc(ctx'', k-1, ctx', s'', s');
-         assert ctx''==ctx';
-         lemma_Xs_lookup(x, T, ctx', s', k-1, ctx, s, ctx_prev);
-         assert V(T, t', k-1, ctx', s');
-         assert V(T, t', k-1, ctx'', s'');
-         lemma_V_monotonic(T, t', k-1, i, ctx'', s'');
-       }
-      }
-      assert E(T, t, k, ctx, Store(Empty), Context(Empty));
-}
-
-ghost method theorem_fundamental_R_sel(ctx: context, T: tp, T1: tp, t1: tm, l: nat, k: nat)
-  requires typing(ctx, tm_sel(t1, l), T);
-  requires A(k, Context(Empty), Store(Empty));
-  requires As(k, ctx, Store(Empty), Context(Empty));
-
-  requires field_membership(ctx, t1, l, T);
-  requires membership(ctx, t1, l, decl_tm(l, T));
-  requires typing(ctx, t1, T1);
-  requires E(T1, t1, k, ctx, Store(Empty), Context(Empty));
-
-  ensures E(T, tm_sel(t1, l), k, ctx, Store(Empty), Context(Empty));
-{
-  var ctx_prev := Context(Empty);
-  var s := Store(Empty);
-  var t := tm_sel(t1, l);
-
-  if (k>0) {
-    forall (
-      i:nat, j:nat,
-      ctx', s':store,
-      t', s'':store,
-      ctx'' |
-      i+j<k &&
-      Xs(ctx', s', k-1, ctx, s, ctx_prev) && A(k-1, ctx', s') &&
-      prefix_of(s''.m, s'.m) && mstep(t, s', t', s'', j) && irred(t', s'') &&
-      Xc(ctx'', k-1, ctx', s'', s') && A(k-1, ctx'', s''))
-      ensures V(T, t', i, ctx'', s'');
-    {
-      var t1', t1s, t1j := lemma_sel_irred__o_mstep_irred(t1, l, t', s', s'', j);
-      lemma_mstep__prefix(t1, s', t1', t1s, t1j);
-      var t1ctx :=  build_Xc(k-1, ctx', t1s, s');
-      lemma_E(T1, t1, t1', k, t1j, i+j-t1j, s, s', t1s, ctx_prev, ctx, ctx', t1ctx);
-      lemma_V_value(T1, t1', i+j-t1j, t1ctx, t1s);
-
-      lemma_mstep_sel(t1, l, t1', s', t1s, t1j);
-      lemma_mstep_trans'(t, s', tm_sel(t1', l), t1s, t', s'', t1j, j);
- 
-      forall (Tc, init, Ds |
-        P(Tc, init) == lookup(t1'.x, t1s.m).get &&
-        expansion(t1ctx, t1'.x, T1, Ds) && Ds.decls_fin?)
-        ensures V(T, t', i, ctx'', s'');
-      {
-        lemma_field_mem__expansion_decl(ctx, t1, T1, l, T, t1ctx, t1'.x, Ds);
-        assert exists U :: decl_tm(l, U) in Ds.decls;
-        // How do we relate U and T?
-        // This is fishy because T might have t1 as self, and U might have t1'.
-        // so certainly, they can be !=.
-        assume decl_tm(l, T) in Ds.decls;
-
-        assume j-t1j>0; // fishy: how can we guarantee that?
-        lemma_V_field(T1, t1', l, T, i+j-t1j, i, t1ctx, t1s, Tc, init, Ds);
-        assert V(T, def_field_lookup(l, init).get, i, t1ctx, t1s);
-        lemma_V_value(T, def_field_lookup(l, init).get, i, t1ctx, t1s);
-              
-        lemma_mstep_trans'(tm_sel(t1', l), t1s, def_field_lookup(l, init).get, t1s, t', s'', 1, j-t1j);
-        
-        assert def_field_lookup(l, init).get.tm_var?;
-        lemma_value__irred(def_field_lookup(l, init).get, t1s);
-        assert irred(def_field_lookup(l, init).get, t1s);
-
-        assert t'==def_field_lookup(l, init).get;
-        assert mstep(def_field_lookup(l, init).get, t1s, t', s'', 0);
-        assert s''==t1s;
-        lemma_Xc_unique(ctx'', t1ctx, k-1, ctx', s'', s');
-        assert ctx''==t1ctx;
-
-        assert V(T, def_field_lookup(l, init).get, i, t1ctx, t1s);
-        assert V(T, t', i, ctx'', s'');
-      }
-
-      assert forall Tc, init, Ds :: (
-        P(Tc, init) == lookup(t1'.x, t1s.m).get &&
-        expansion(t1ctx, t1'.x, T1, Ds) && Ds.decls_fin?) ==>
-        V(T, t', i, ctx'', s'');
-      assert exists Tc, init :: P(Tc, init) == lookup(t1'.x, t1s.m).get;
-      assert exists Ds :: expansion(t1ctx, t1'.x, T1, Ds) && Ds.decls_fin?;
-      assert exists Tc, init, Ds :: (
-        P(Tc, init) == lookup(t1'.x, t1s.m).get &&
-        expansion(t1ctx, t1'.x, T1, Ds) && Ds.decls_fin?);
-      assert V(T, t', i, ctx'', s'');
+  forall (l:nat | l < |s'.m|)
+  ensures store_well_typed1(s', l, fresh_from([]), store_lookup_type(l, s'), store_lookup(l, s'));
+  {
+    if (l == |s.m|) {
+    } else {
+      assert l < |s.m|;
+      var initl := store_lookup(l, s);
+      var Tcl := store_lookup_type(l, s); 
+      assert store_well_typed1(s, l, fresh_from([]), Tcl, initl);
+      assert store_lookup(l, s') == initl;
+      assert store_lookup_type(l, s') == Tcl;
+      lemma_store_invariance_well_typed1(s, s', l, fresh_from([]), Tcl, initl);
     }
   }
 }
 
-ghost method theorem_fundamental_R(ctx: context, t: tm, T: tp)
-  requires typing(ctx, t, T);
-  ensures R(ctx, t, T);
+predicate closed(t: tm)
+{
+  forall x: nat :: !tm_fn(x, t)
+}
+
+ghost method lemma_free_after_tm_subst(x: nat, y_: nat, y: nat, t_: tm)
+  requires x!=y_;
+  requires tm_fn(x, t_);
+  ensures tm_fn(x, tm_subst(y_, tm_var(y), t_));
+  decreases tm_size(t_);
+{
+  if (t_.tm_var?) {
+  } else if (t_.tm_loc?) {
+  } else if (t_.tm_sel?) {
+  } else if (t_.tm_msel?) {
+  } else if (t_.tm_new?) {
+    if (t_.y==y_) {
+      assert tm_subst(y_, tm_var(y), t_) == tm_new(t_.y, tp_subst(y_, tm_var(y), t_.Tc), t_.init, t_.t');
+      if (tp_fn(x, t_.Tc)) {
+        lemma_free_after_tp_subst(x, y_, y, t_.Tc);
+      }
+    } else {
+      var y' := fresh_from([y_]+tm_vars(tm_var(y))+tm_vars(t_));
+      var init' := defs_subst(t_.y, tm_var(y'), t_.init);
+      var t1' := tm_subst(t_.y, tm_var(y'), t_.t');
+      assert tm_subst(y_, tm_var(y), t_) == tm_new(y', tp_subst(y_, tm_var(y), t_.Tc), defs_subst(y_, tm_var(y), init'), tm_subst(y_, tm_var(y), t1'));
+      if (tp_fn(x, t_.Tc)) {
+       lemma_free_after_tp_subst(x, y_, y, t_.Tc);
+      } else if (defs_fn(x, t_.init)) {
+        lemma_free_after_defs_subst(x, t_.y, y', t_.init);
+        assert defs_fn(x, init');
+        lemma_free_after_defs_subst(x, y_, y, init');
+        assert defs_fn(x, defs_subst(y_, tm_var(y), init'));
+        assert tm_fn(x, tm_new(y', tp_subst(y_, tm_var(y), t_.Tc), defs_subst(y_, tm_var(y), init'), tm_subst(y_, tm_var(y), t1')));
+        assert tm_fn(x, tm_subst(y_, tm_var(y), t_));
+      } else if (tm_fn(x, t_.t')) {
+        lemma_free_after_tm_subst(x, t_.y, y', t_.t');
+        lemma_free_after_tm_subst(x, y_, y, t1');
+      } else {
+      }
+    }
+  } else {
+  }
+}
+ghost method lemma_free_after_tp_subst(x: nat, y_: nat, y: nat, T_: tp)
+  requires x!=y_;
+  requires tp_fn(x, T_);
+  ensures tp_fn(x, tp_subst(y_, tm_var(y), T_));
+{
+  assume tp_fn(x, tp_subst(y_, tm_var(y), T_)); // TODO
+}
+ghost method lemma_free_after_defs_subst(x: nat, y_: nat, y: nat, init_: list<def>)
+  requires x!=y_;
+  requires defs_fn(x, init_);
+  ensures defs_fn(x, defs_subst(y_, tm_var(y), init_));
+{
+  assume defs_fn(x, defs_subst(y_, tm_var(y), init_)); // TODO
+}
+
+
+ghost method lemma_free_in_context_typing(x:nat, n: nat, ctx: context, s: store, t: tm, T: tp)
+  requires tm_fn(x, t);
+  requires typing(n, ctx, s, t, T);
+  ensures context_lookup(ctx, x).Some?;
+  requires typing(n, ctx, s, t, T);
+{
+  if (t.tm_var?) {
+  } else if (t.tm_loc?) {
+  } else if (t.tm_sel?) {
+    assert membership(n-2, ctx, s, t.t, t.l, decl_tm(t.l, T));
+    var To :| typing(n-3, ctx, s, t.t, To);
+    lemma_free_in_context_typing(x, n-3, ctx, s, t.t, To);
+  } else if (t.tm_msel?) {
+    var S, T' :| method_membership(n-1, ctx, s, t.o, t.m, S, T) &&
+    typing(n-1, ctx, s, t.a, T') &&
+    subtype(n-1, ctx, s, T', S);
+    assert membership(n-2, ctx, s, t.o, t.m, decl_mt(t.m, S, T));
+    var To :| typing(n-3, ctx, s, t.o, To);
+    assert tm_fn(x, t.o) || tm_fn(x, t.a);
+    if (tm_fn(x, t.o)) {
+      lemma_free_in_context_typing(x, n-3, ctx, s, t.o, To);
+    }
+    if (tm_fn(x, t.a)) {
+      lemma_free_in_context_typing(x, n-1, ctx, s, t.a, T');
+    }
+  } else if (t.tm_new?) {
+    var y := fresh_from(dom(ctx)+tm_vars(t));
+    var init := defs_subst(t.y, tm_var(y), t.init);
+    var t' := tm_subst(t.y, tm_var(y), t.t');
+    if (tp_fn(x, t.Tc)) {
+     assert wfe_type(n-1, ctx, s, t.Tc);
+     lemma_free_in_context_wfe_type(x, n-1, ctx, s, t.Tc);
+    } else if (tm_fn(x, t.t')) {
+      lemma_free_after_tm_subst(x, t.y, y, t.t');
+      assert tm_fn(x, t');
+      var T' :| typing(n-1, context_extend(ctx, y, t.Tc), s, t', T');
+      lemma_free_in_context_typing(x, n-1, context_extend(ctx, y, t.Tc), s, t', T');
+    } else if (defs_fn(x, t.init)) {
+      lemma_free_after_defs_subst(x, t.y, y, t.init);
+      assert defs_fn(x, init);
+      assume context_lookup(ctx, x).Some?; // TODO (really!)
+    }
+  } else {
+  }
+}
+ghost method lemma_free_in_context_wfe_type(x: nat, n: nat, ctx: context, s: store, T: tp)
+  requires tp_fn(x, T);
+  requires wfe_type(n, ctx, s, T);
+  ensures context_lookup(ctx, x).Some?;
+  ensures wfe_type(n, ctx, s, T);
+{
+  assume context_lookup(ctx, x).Some?; // TODO (really!)
+}
+
+ghost method corollary_typable_empty__closed(n: nat, s: store, t: tm, T: tp)
+  requires typing(n, Context([]), s, t, T);
+  ensures closed(t);
+{
+  forall (x: nat)
+    ensures !tm_fn(x, t);
+  {
+    if (tm_fn(x, t)) {
+      lemma_free_in_context_typing(x, n, Context([]), s, t, T);
+      assert context_lookup(Context([]), x).Some?;
+      assert false;
+    }
+    assert !tm_fn(x, t);
+  }
+}
+
+ghost method lemma_context_invariance(n: nat, ctx: context, ctx': context, s: store, t: tm, T: tp)
+  requires typing(n, ctx, s, t, T);
+  requires forall x:nat :: tm_fn(x, t) ==> context_lookup(ctx, x) == context_lookup(ctx', x);
+  ensures typing(n, ctx', s, t, T);
   decreases t;
 {
-  var ctx_prev := Context(Empty);
-  var s := Store(Empty);
-
-  forall (k: nat)
-    ensures
-      A(k, ctx_prev, s) &&
-      As(k, ctx, s, ctx_prev) &&
-      E(T, t, k, ctx, s, ctx_prev);
-  {
-    lemma_empty_prefix_of_any(ctx.m);
-    assert As(k, ctx, s, ctx_prev);
-
-    match t {
-    case tm_var(x) =>
-      theorem_fundamental_R_var(ctx, T, x, k);
-    case tm_new(y, Tc, init, t1) =>
-      assume E(T, t, k, ctx, Store(Empty), Context(Empty)); // TODO
-    case tm_sel(t1, l) =>
-      assert field_membership(ctx, t1, l, T);
-      assert membership(ctx, t1, l, decl_tm(l, T));
-      assert exists T1 :: typing(ctx, t1, T1);
-      forall (T1 | typing(ctx, t1, T1))
-        ensures E(T, t, k, ctx, s, ctx_prev);
-      {
-        theorem_fundamental_R(ctx, t1, T1);
-        theorem_fundamental_R_sel(ctx, T, T1, t1, l, k);
-      }
-      assert forall T1 :: typing(ctx, t1, T1) ==> E(T, t, k, ctx, s, ctx_prev);
-      assert exists T1 :: typing(ctx, t1, T1);
-      assert E(T, t, k, ctx, s, ctx_prev);
-    case tm_msel(o, m, a) =>
-      assume E(T, t, k, ctx, Store(Empty), Context(Empty)); // TODO
-    }
-  }
+  assume typing(n, ctx', s, t, T); // TODO (really!)
 }
 
-// -----------
-// Type-Safety
-// -----------
-predicate type_safety(t: tm, T: tp)
+ghost method lemma_substitution_preserves_typing(ctx: context, st: store, x: nat, s: tm, S: tp, ns: nat, t: tm, T: tp, n: nat) returns (n': nat, T': tp, ns': nat)
+  requires typing(ns, Context([]), st, s, S);
+  requires context_lookup(ctx, x).None?;
+  requires typing(n, context_extend(ctx, x, S), st, t, T);
+  requires path(s);
+  ensures typing(n', ctx, st, tm_subst(x, s, t), T');
+  ensures subtype(ns', context_extend(ctx, x, S), st, T', T);
+  decreases t;
 {
-  typing(Context(Empty), t, T) ==>
-  forall t', s', n:nat :: mstep(t, Store(Empty), t', s', n) ==>
-  value(t') || step(t', s').Some?
-}
-
-ghost method corollary_type_safety(t: tm, T: tp)
-  ensures type_safety(t, T);
-{
-  if (typing(Context(Empty), t, T)) {
-    forall (t', s', n:nat | mstep(t, Store(Empty), t', s', n))
-      ensures value(t') || step(t', s').Some?;
-    {
-      theorem_fundamental_R(Context(Empty), t, T);
-      assert A(n, Context(Empty), Store(Empty));
-      assert As(n, Context(Empty), Store(Empty), Context(Empty));
-      assert E(T, t, n+1, Context(Empty), Store(Empty), Context(Empty));
-      assert Xs(Context(Empty), Store(Empty), n, Context(Empty), Store(Empty), Context(Empty));
-      assert A(n, Context(Empty), Store(Empty));
-      lemma_empty_prefix_of_any(s'.m);
-      assert prefix_of(s'.m, Store(Empty).m);
-      assert mstep(t, Store(Empty), t', s', n);
-      assert Ac(n+1, Context(Empty), s', Store(Empty));
-      var ctx' := build_Xc(n+1, Context(Empty), s', Store(Empty));
-      lemma_E(T, t, t', n+1, n, 0, Store(Empty), Store(Empty), s', Context(Empty), Context(Empty), Context(Empty), ctx');
+  if (t.tm_var?) {
+    if (t.x==x) {
+      assert tm_subst(x, s, t)==s;
+      corollary_typable_empty__closed(ns, st, s, S);
+      lemma_context_invariance(ns, Context([]), ctx, st, s, S);
+      n' := ns;
+      T' := T;
+      assert typing(n', ctx, st, tm_subst(x, s, t), T');
+      ns' := 1;
+    } else {
+      n' := 0;
+      T' := T;
+      ns' := 1;
     }
+  } else if (t.tm_loc?) {
+    n' := 0;
+    T' := T;
+    ns' := 1;
+  } else if (t.tm_sel?) {
+    assert field_membership(n-1, context_extend(ctx, x, S), st, t.t, t.l, T);
+    assert membership(n-2, context_extend(ctx, x, S), st, t.t, t.l, decl_tm(t.l, T));
+    var d := decl_tm(t.l, T);
+    var z:nat := fresh_in_context(context_extend(ctx, x, S));
+    helper_assert_membership(n-2, context_extend(ctx, x, S), st, t.t, t.l, d, z);
+    assert decl_label(d)==t.l &&
+    n-2>0 && exists To:tp, To':tp :: typing(n-3, context_extend(ctx, x, S), st, t.t, To') &&
+    subtype(n-3, context_extend(ctx, x, S), st, To', To) &&
+    exists Ds ::
+    expansion(n-3, context_extend(ctx, x, S), st, z, To, Ds) &&
+    ((Ds.decls_fin? &&
+      ((path(t.t) && To'==To && exists d' :: d' in lst2seq(Ds.decls) && d==decl_subst(z, t.t, d')) ||
+       (!path(t.t) && d in lst2seq(Ds.decls) && !decl_fn(z, d)))) ||
+     (Ds.decls_bot? && decl_bot(d)));
+    var To:tp, To':tp, Ds:decls :| typing(n-3, context_extend(ctx, x, S), st, t.t, To') &&
+    subtype(n-3, context_extend(ctx, x, S), st, To', To) &&
+    expansion(n-3, context_extend(ctx, x, S), st, z, To, Ds) &&
+    ((Ds.decls_fin? &&
+      ((path(t.t) && To'==To && exists d' :: d' in lst2seq(Ds.decls) && d==decl_subst(z, t.t, d')) ||
+       (!path(t.t) && d in lst2seq(Ds.decls) && !decl_fn(z, d)))) ||
+     (Ds.decls_bot? && decl_bot(d)));
+  } else if (t.tm_msel?) {
+  } else if (t.tm_new?) {
+  } else {
   }
+  // TODO (absolutely!)
+  assume exists n'':nat, T'':tp, ns'':nat :: typing(n'', ctx, st, tm_subst(x, s, t), T'') && subtype(ns'', context_extend(ctx, x, S), st, T'', T);
+  var n'':nat, T'':tp, ns'':nat :| typing(n'', ctx, st, tm_subst(x, s, t), T'') && subtype(ns'', context_extend(ctx, x, S), st, T'', T);
+  n' := n'';
+  T' := T'';
+  ns' := ns'';
+}
+ghost method helper_assert_membership(n: nat, ctx: context, s: store, t: tm, l: nat, d: decl, z: nat)
+  requires z == fresh_in_context(ctx);
+  requires membership(n, ctx, s, t, l, d);
+  ensures decl_label(d)==l &&
+  n>0 && exists T, T' :: typing(n-1, ctx, s, t, T') &&
+  subtype(n-1, ctx, s, T', T) &&
+  exists Ds ::
+  expansion(n-1, ctx, s, z, T, Ds) &&
+  ((Ds.decls_fin? &&
+     ((path(t) && T'==T && exists d' :: d' in lst2seq(Ds.decls) && d==decl_subst(z, t, d')) ||
+      (!path(t) && d in lst2seq(Ds.decls) && !decl_fn(z, d)))) ||
+   (Ds.decls_bot? && decl_bot(d)));
+{
 }
