src/dafny/old/Dot.dfy
@@ -1,0 +1,1723 @@
+// ============================
+// Dependent Object Types (DOT)
+// ============================
+
+// ---------
+// Utilities
+// ---------
+
+// ### List ###
+datatype list<A> = Nil | Cons(head: A, tail: list<A>);
+function length<A>(lst: list<A>): nat
+  ensures length(lst)==0 ==> lst.Nil?;
+  ensures length(lst)>0 ==> lst.Cons?;
+{
+  match lst
+  case Nil => 0
+  case Cons(head, tail) => 1 + length(tail)
+}
+function nth<A>(n: nat, lst: list<A>): A
+  requires n < length(lst);
+{
+  if (n==0) then lst.head else nth(n-1, lst.tail)
+}
+function slice<A>(i: nat, j: nat, lst: list<A>): list<A>
+  requires 0 <= i <= j <= length(lst);
+  decreases j-i;
+{
+  if (i==j) then Nil
+  else if (i==0) then Cons(lst.head, slice(i, j-1, lst.tail))
+  else slice(i+1, j, lst)
+}
+function snoc<A>(lst: list<A>, x: A): list<A>
+{
+  match lst
+  case Nil => Cons(x, Nil)
+  case Cons(head, tail) => Cons(head, snoc(tail, x))
+}
+function seq2lst<A>(s: seq<A>): list<A>
+{
+  if (s == []) then Nil
+  else Cons(s[0], seq2lst(s[1..]))
+}
+function lst2seq<A>(lst: list<A>): seq<A>
+{
+  match lst
+  case Nil => []
+  case Cons(head, tail) => [head] + lst2seq(tail)
+}
+predicate same_lst_seq<A>(lst: list<A>, s: seq<A>)
+  ensures same_lst_seq(lst, s) ==> length(lst)==|s|;
+{
+  match lst
+  case Nil => s==[]
+  case Cons(head, tail) => |s|>0 && s[0]==head && same_lst_seq(tail, s[1..])
+}
+ghost method lemma_lst2seq_same<A>(lst: list<A>, s: seq<A>)
+  requires lst2seq(lst)==s;
+  ensures same_lst_seq(lst, s);
+{
+}
+ghost method lemma_same_lst_seq_forall<A>(lst: list<A>, s: seq<A>)
+  requires same_lst_seq(lst, s );
+  ensures forall n :: 0 <= n < |s| ==> s[n]==nth(n, lst);
+{
+  match lst {
+  case Nil =>
+  case Cons(head, tail) =>
+    assert s[0]==head;
+    lemma_same_lst_seq_forall(tail, s[1..]);
+  }
+}
+
+// ### Pair ###
+datatype pair<A, B> = P(fst: A, snd: B);
+
+// ### Option ###
+datatype option<A> = None | Some(get: A);
+
+// ### Partial Maps ###
+datatype partial_map<K,V> = Empty | Extend(x: K, v: V, rest: partial_map<K,V>);
+function lookup<K,V>(x: K, m: partial_map<K,V>): option<V>
+  ensures m.Empty? ==> lookup(x, m).None?;
+  ensures m.Empty? ==> !lookup(x, m).Some?;
+  ensures m.Extend? && m.x==x ==> lookup(x, m) == Some(m.v);
+  ensures m.Extend? && m.x!=x ==> lookup(x, m) == lookup(x, m.rest);
+{
+  match m
+  case Empty => None
+  case Extend(x', v, rest) => if x==x' then Some(v) else lookup(x, rest)
+}
+function dom<K,V>(m: partial_map<K,V>): seq<K>
+  ensures forall x :: x in dom(m) ==> lookup(x, m).Some?;
+  ensures m.Extend? ==> dom(m) == [m.x]+dom(m.rest);
+{
+  match m
+  case Empty => []
+  case Extend(x, v, rest) => [x]+dom(rest)
+}
+function prefixes<K,V>(m: partial_map<K,V>): seq<partial_map<K,V>>
+  ensures m in prefixes(m);
+  ensures m.Extend? ==> m.rest in prefixes(m);
+{
+  match m
+  case Empty => [m]
+  case Extend(x, v, rest) => [m]+prefixes(rest)
+}
+predicate prefix_of<K,V>(m: partial_map<K,V>, m_prev: partial_map<K,V>)
+{
+  m==m_prev || (m.Extend? && prefix_of(m.rest, m_prev))
+}
+function build<K,V>(m: partial_map<K,V>, r: partial_map<K,V>): partial_map<K,V>
+  decreases r;
+{
+  match r
+  case Empty => m
+  case Extend(x, v, rest) => build(Extend(x, v, m), rest)
+}
+function map_complement<K,V>(m: partial_map<K,V>, m_prev: partial_map<K,V>, start: partial_map<K,V>): partial_map<K,V>
+  requires prefix_of(m, m_prev);
+  //ensures build(m_prev, map_complement(m, m_prev, Empty))==m;
+  decreases m;
+{
+  if (m==m_prev) then start
+  else map_complement(m.rest, m_prev, Extend(m.x, m.v, start))
+}
+function map_fst<K,A,B>(m: partial_map<K,pair<A,B>>): partial_map<K,A>
+  ensures dom(m)==dom(map_fst(m));
+{
+  match m
+  case Empty => Empty
+  case Extend(x, v, rest) => Extend(x, v.fst, map_fst(rest))
+}
+
+// ### Sequences ###
+function max(s: seq<int>, start: int): int
+  ensures max(s, start)>=start;
+  ensures forall x :: x in s ==> x<=max(s, start);
+{
+  if (s == []) then start
+  else if (s[0] <= start) then max(s[1..], start)
+  else max(s[1..], s[0])
+}
+function rev<A>(s: seq<A>): seq<A>
+{
+  if (|s|==0) then [] else rev(s[1..])+[s[0]]
+}
+
+// ### Lemmas about utilities ###
+ghost method lemma_empty_prefix_of_any<K,V>(m: partial_map<K,V>)
+  ensures prefix_of(m, Empty);
+{
+}
+ghost method lemma_rev_beg__end<A>(s: seq<A>, x: A)
+  ensures rev([x]+s)==rev(s)+[x];
+{
+}
+ghost method lemma_rev<A>(s1: seq<A>, s2: seq<A>)
+  ensures rev(s1+s2)==rev(s2)+rev(s1);
+{
+  if (s1==[]) {
+    assert s1+s2==s2;
+  } else {
+    lemma_rev_beg__end(s1[1..], s1[0]);
+    assert rev([s1[0]]+(s1[1..]+s2))==rev(s1[1..]+s2)+[s1[0]];
+    lemma_rev(s1[1..], s2);
+    assert rev(s1[1..]+s2)+[s1[0]]==rev(s2)+rev(s1[1..])+[s1[0]];
+    lemma_rev_beg__end(s1[1..], s1[0]);
+    assert rev(s1[1..]+s2)+[s1[0]]==rev(s2)+rev(s1);
+    assert rev([s1[0]]+(s1[1..]+s2))==rev(s2)+rev(s1);
+    assert [s1[0]]+(s1[1..]+s2)==([s1[0]]+s1[1..])+s2;
+    assert [s1[0]]+s1[1..]==s1;
+    assert ([s1[0]]+s1[1..])+s2==s1+s2;
+    assert rev([s1[0]]+(s1[1..]+s2))==rev(([s1[0]]+s1[1..])+s2);
+    assert rev([s1[0]]+(s1[1..]+s2))==rev(s1+s2);
+    assert rev(s1+s2)==rev(s2)+rev(s1);
+  }
+}
+ghost method lemma_rev_end__beg<A>(s: seq<A>, x: A)
+  ensures rev(s+[x])==[x]+rev(s);
+{
+  lemma_rev(s, [x]);
+}
+ghost method lemma_rev_rev<A>(s: seq<A>)
+  ensures rev(rev(s))==s;
+{
+  if (|s|==0) {
+
+  } else {
+    lemma_rev_rev(s[1..]);
+    assert rev(rev(s[1..]))==s[1..];
+    lemma_rev_beg__end(s[1..], s[0]);
+    assert rev([s[0]]+s[1..])==rev(s[1..])+[s[0]];
+    lemma_rev_end__beg(rev(s[1..]), s[0]);
+    assert rev(rev(s[1..])+[s[0]])==[s[0]]+rev(rev(s[1..]));
+    assert [s[0]]+rev(rev(s[1..]))==[s[0]]+s[1..];
+    assert [s[0]]+s[1..]==s;
+    assert rev(rev(s))==rev(rev([s[0]]+s[1..]));
+    assert rev(rev([s[0]]+s[1..]))==[s[0]]+rev(rev(s[1..]));
+    assert [s[0]]+rev(rev(s[1..]))==[s[0]]+s[1..];
+    assert rev(rev(s))==s;
+  }
+}
+ghost method lemma_prefix_of__dom<K,V>(m: partial_map<K,V>, m_prev: partial_map<K,V>) returns (s: seq<K>)
+  requires prefix_of(m, m_prev);
+  ensures dom(m)==s+dom(m_prev);
+{
+  if (m==m_prev) {
+    s := [];
+  } else {
+    var s' := lemma_prefix_of__dom(m.rest, m_prev);
+    assert dom(m.rest)==s'+dom(m_prev);
+    s := [m.x] + s';
+    assert dom(m)==[m.x]+dom(m.rest);
+  }
+}
+ghost method lemma_map_complement_extend__dom'<K,V>(m: partial_map<K,V>, m_prev: partial_map<K,V>, start: partial_map<K,V>)
+  requires prefix_of(m, m_prev);
+  ensures dom(map_complement(m, m_prev, start))==dom(map_complement(m, m_prev, Empty))+dom(start);
+{
+}
+ghost method lemma_map_complement_extend__dom<K,V>(m: partial_map<K,V>, m_prev: partial_map<K,V>)
+  requires prefix_of(m, m_prev);
+  ensures m!=m_prev ==> dom(map_complement(m, m_prev, Empty))==dom(map_complement(m.rest, m_prev, Extend(m.x, m.v, Empty)));
+  ensures m!=m_prev ==> dom(map_complement(m, m_prev, Empty))==dom(map_complement(m.rest, m_prev, Empty))+[m.x];
+{
+  if (m!=m_prev) {
+    lemma_map_complement_extend__dom'(m.rest, m_prev, Extend(m.x, m.v, Empty));
+  }
+}
+ghost method lemma_map_complement__dom<K,V>(m: partial_map<K,V>, m_prev: partial_map<K,V>)
+  requires prefix_of(m, m_prev);
+  ensures dom(m)==rev(dom(map_complement(m, m_prev, Empty)))+dom(m_prev);
+{
+  if (m==m_prev) {
+  } else {
+    lemma_map_complement__dom(m.rest, m_prev);
+    assert dom(m.rest)==rev(dom(map_complement(m.rest, m_prev, Empty)))+dom(m_prev);
+    lemma_map_complement_extend__dom(m, m_prev);
+    assert dom(map_complement(m, m_prev, Empty))==dom(map_complement(m.rest, m_prev, Empty))+[m.x];
+    assert rev(dom(map_complement(m, m_prev, Empty)))==rev(dom(map_complement(m.rest, m_prev, Empty))+[m.x]);
+    lemma_rev_end__beg(dom(map_complement(m.rest, m_prev, Empty)), m.x);
+    assert rev(dom(map_complement(m.rest, m_prev, Empty))+[m.x])==[m.x]+rev(dom(map_complement(m.rest, m_prev, Empty)));
+  }
+}
+ghost method lemma_map_complement_prev_empty__dom<K,V>(m: partial_map<K,V>)
+  ensures prefix_of(m, Empty);
+  ensures dom(m)==rev(dom(map_complement(m, Empty, Empty)));
+  ensures rev(dom(m))==dom(map_complement(m, Empty, Empty));
+{
+  lemma_map_complement__dom(m, Empty);
+  assert dom(m)==rev(dom(map_complement(m, Empty, Empty)));
+  assert rev(dom(m))==rev(rev(dom(map_complement(m, Empty, Empty))));
+  lemma_rev_rev(dom(map_complement(m, Empty, Empty)));
+  assert rev(rev(dom(map_complement(m, Empty, Empty))))==dom(map_complement(m, Empty, Empty));
+  assert rev(dom(m))==dom(map_complement(m, Empty, Empty));
+}
+ghost method lemma_build__dom<K,V>(m: partial_map<K,V>, r: partial_map<K,V>)
+  ensures dom(build(m, r)) == rev(dom(r)) + dom(m);
+  decreases r;
+{
+  match r {
+  case Empty =>
+  case Extend(x, v, rest) =>
+    lemma_build__dom(Extend(x, v, m), rest);
+    assert dom(build(Extend(x, v, m), rest)) == rev(dom(rest)) + dom(Extend(x, v, m));
+    assert dom(Extend(x, v, m)) == [x]+dom(m);
+    lemma_rev_beg__end(dom(rest), x);
+    assert rev(dom(rest))+[x]==rev([x]+dom(rest));
+  }
+}
+ghost method lemma_prefix_of_trans<K,V>(m1: partial_map<K,V>, m2: partial_map<K,V>, m3: partial_map<K,V>)
+  requires prefix_of(m3, m2);
+  requires prefix_of(m2, m1);
+  ensures prefix_of(m3, m1);
+{
+}
+
+// ------
+// Syntax
+// ------
+
+datatype tp = tp_sel_c(pc: tm, Lc: nat) | tp_sel_a(pa: tm, La: nat) | tp_rfn(base_tp: tp, self: nat, decls: list<decl>) | tp_and(and1: tp, and2: tp) | tp_or(or1: tp, or2: tp) | tp_top | tp_bot;
+datatype tm = tm_var(x: nat) | tm_new(y: nat, Tc: tp, init: list<def>, t': tm) | tm_sel(t: tm, l: nat) | tm_msel(o: tm, m: nat, a: tm);
+datatype decl = decl_tp_c(Lc: nat, Sc: tp, Uc: tp) | decl_tp_a(La: nat, Sa: tp, Ua: tp) | decl_tm(l: nat, T: tp) | decl_mt(m: nat, P: tp, R: tp);
+datatype def = def_tm(l: nat, t: tm) | def_mt(m: nat, param: nat, body: tm);
+datatype decls = decls_fin(decls: seq<decl>) | decls_bot;
+
+predicate path(t: tm)
+{
+  t.tm_var? || (t.tm_sel? && path(t.t))
+}
+
+predicate concrete(T: tp)
+{
+  (T.tp_sel_c? && path(T.pc)) ||
+  (T.tp_rfn? && concrete(T.base_tp)) ||
+  (T.tp_and? && concrete(T.and1) && concrete(T.and2)) ||
+  T.tp_top?
+}
+
+function decl_label(d: decl): nat
+{
+  match d
+  case decl_tp_c(Lc, Sc, Uc) => Lc
+  case decl_tp_a(La, Sa, Ua) => La
+  case decl_tm(l, T) => l
+  case decl_mt(m, P, R) => m
+}
+
+// -------------------------
+// Sorting-related functions
+// -------------------------
+
+predicate decl_lt(d1: decl, d2: decl)
+{
+  match d1
+  case decl_tp_c(Lc1, Sc1, Uc1) =>
+    (match d2
+     case decl_tp_c(Lc2, Sc2, Uc2) => Lc1<Lc2
+     case decl_tp_a(La2, Sa2, Ua2) => true
+     case decl_tm(l2, T2) => true
+     case decl_mt(m2, P2, R2) => true)
+  case decl_tp_a(La1, Sa1, Ua1) =>
+    (match d2
+     case decl_tp_c(Lc2, Sc2, Uc2) => false
+     case decl_tp_a(La2, Sa2, Ua2) => La1<La2
+     case decl_tm(l2, T2) => true
+     case decl_mt(m2, P2, R2) => true)
+  case decl_tm(l1, T1) =>
+    (match d2
+     case decl_tp_c(Lc2, Sc2, Uc2) => false
+     case decl_tp_a(La2, Sa2, Ua2) => false
+     case decl_tm(l2, T2) => l1<l2
+     case decl_mt(m2, P2, R2) => true)
+  case decl_mt(m1, P1, R1) =>
+    (match d2
+     case decl_tp_c(Lc2, Sc2, Uc2) => false
+     case decl_tp_a(La2, Sa2, Ua2) => false
+     case decl_tm(l2, T2) => false
+     case decl_mt(m2, P2, R2) => m1<m2)    
+}
+predicate decl_eq(d1: decl, d2: decl)
+  ensures d1==d2 ==> decl_eq(d1, d2);
+  ensures decl_eq(d1, d2) ==> decl_label(d1)==decl_label(d2);
+  ensures decl_eq(d1, d2) ==> d1.decl_tp_c?==d2.decl_tp_c?;
+  ensures decl_eq(d1, d2) ==> d1.decl_tp_a?==d2.decl_tp_a?;
+  ensures decl_eq(d1, d2) ==> d1.decl_tm?==d2.decl_tm?;
+  ensures decl_eq(d1, d2) ==> d1.decl_mt?==d2.decl_mt?;
+  ensures decl_eq(d1, d2) ==> !decl_lt(d1, d2) && !decl_lt(d2, d1);
+{
+  match d1
+  case decl_tp_c(Lc1, Sc1, Uc1) => d2.decl_tp_c? && d2.Lc==Lc1
+  case decl_tp_a(La1, Sa1, Ua1) => d2.decl_tp_a? && d2.La==La1
+  case decl_tm(l1, T1) => d2.decl_tm? && d2.l==l1
+  case decl_mt(m1, P1, R1) => d2.decl_mt? && d2.m==m1
+}
+predicate decl_le(d1: decl, d2: decl)
+  ensures d1==d2 ==> decl_le(d1, d2);
+{
+  decl_lt(d1, d2) || decl_eq(d1, d2)
+}
+predicate decl_seq_sorted(s: seq<decl>)
+{
+  forall m,n :: 0 <= m < n < |s| ==> decl_le(s[m], s[n])
+}
+function decl_seq_merge(s1: seq<decl>, s2: seq<decl>): seq<decl>
+{
+  if (s1 == []) then s2
+  else if (s2 == []) then s1
+  else if (decl_le(s1[0], s2[0])) then [s1[0]]+decl_seq_merge(s1[1..], s2)
+  else [s2[0]]+decl_seq_merge(s1, s2[1..])
+}
+function decl_seq_sort(s: seq<decl>): seq<decl>
+{
+  if (s == []) then s else
+    var i: nat := (|s|-1)/2;
+    decl_seq_merge(decl_seq_sort(s[..i]), decl_seq_sort(s[i+1..]))
+}
+predicate decl_lst_sorted(lst: list<decl>)
+{
+  match lst
+  case Nil => true
+  case Cons(x, tail) =>
+    (match tail
+     case Nil => true
+     case Cons(y, tail') => decl_le(x, y) && decl_lst_sorted(tail))
+}
+function decl_lst_sort(lst: list<decl>): list<decl>
+{
+  seq2lst(decl_seq_sort(lst2seq(lst)))
+}
+ghost method lemma_decl_le_trans(d1: decl, d2: decl, d3: decl)
+  requires decl_le(d1, d2);
+  requires decl_le(d2, d3);
+  ensures decl_le(d1, d3);
+{
+}
+ghost method lemma_decl_le_comparable(d1: decl, d2: decl)
+  requires !decl_le(d1, d2);
+  ensures decl_le(d2, d1);
+{
+}
+ghost method lemma_decl_seq_merging(s1: seq<decl>, s2: seq<decl>)
+  requires decl_seq_sorted(s1) && decl_seq_sorted(s2);
+  ensures decl_seq_sorted(decl_seq_merge(s1, s2));
+  ensures multiset((s1+s2)[..]) == multiset(decl_seq_merge(s1,s2)[..]);
+{
+  if (s1 == []) {}
+  else if (s2 == []) {}
+  else if (decl_le(s1[0], s2[0])) {
+    forall (n | 0 <= n < |s1|)
+      ensures decl_le(s1[0], s1[n]);
+    {
+    }
+    forall (n | 0 <= n < |s2|)
+      ensures decl_le(s1[0], s2[n]);
+    {
+      lemma_decl_le_trans(s1[0], s2[0], s2[n]);
+    }
+    var sm := decl_seq_merge(s1[1..], s2);
+    lemma_decl_seq_merging(s1[1..], s2);
+    var s := [s1[0]]+sm;
+    assert decl_le(s1[0], sm[0]);
+    forall (m,n | 0 <= m < n < |s|)
+      ensures decl_le(s[m], s[n]);
+    {
+      if (m==0) {
+        lemma_decl_le_trans(s1[0], sm[0], s[n]);
+      }
+    }
+  } else {
+    lemma_decl_le_comparable(s1[0], s2[0]);
+    forall (n | 0 <= n < |s2|)
+      ensures decl_le(s2[0], s2[n]);
+    {
+    }
+    forall (n | 0 <= n < |s1|)
+      ensures decl_le(s2[0], s1[n]);
+    {
+      lemma_decl_le_trans(s2[0], s1[0], s1[n]);
+    }
+    var sm := decl_seq_merge(s1, s2[1..]);
+    lemma_decl_seq_merging(s1, s2[1..]);
+    var s := [s2[0]]+sm;
+    assert decl_le(s2[0], sm[0]);
+    forall (m,n | 0 <= m < n < |s|)
+      ensures decl_le(s[m], s[n]);
+    {
+      if (m==0) {
+        lemma_decl_le_trans(s2[0], sm[0], s[n]);
+      }
+    }
+  }  
+}
+ghost method lemma_decl_seq_sorting(s: seq<decl>)
+  ensures decl_seq_sorted(decl_seq_sort(s));
+  ensures multiset(s[..]) == multiset(decl_seq_sort(s)[..]);
+{
+  if (s == []) {}
+  else {
+    var i: nat := (|s|-1)/2;
+    lemma_decl_seq_sorting(s[..i]);
+    lemma_decl_seq_sorting(s[i+1..]);
+    lemma_decl_seq_merging(decl_seq_sort(s[..i]), decl_seq_sort(s[i+1..]));    
+  }
+}
+predicate def_lt(d1: def, d2: def)
+{
+  match d1
+  case def_tm(l1, t1) =>
+    (match d2
+     case def_tm(l2, t2) => l1<l2
+     case def_mt(m2, param2, body2) => true)
+  case def_mt(m1, param1, body1) =>
+    (match d2
+     case def_tm(l2, t2) => false
+     case def_mt(m2, param2, body2) => m1<m2)
+}
+predicate def_eq(d1: def, d2: def)
+  ensures d1==d2 ==> def_eq(d1, d2);
+{
+  match d1
+  case def_tm(l1, t1) => d2.def_tm? && d2.l==l1
+  case def_mt(m1, param1, body1) => d2.def_mt? && d2.m==m1
+}
+predicate def_le(d1: def, d2: def)
+  ensures d1==d2 ==> def_le(d1, d2);
+{
+  def_lt(d1, d2) || def_eq(d1, d2)
+}
+predicate def_seq_sorted(s: seq<def>)
+{
+  forall m,n :: 0 <= m < n < |s| ==> def_le(s[m], s[n])
+}
+function def_seq_merge(s1: seq<def>, s2: seq<def>): seq<def>
+{
+  if (s1 == []) then s2
+  else if (s2 == []) then s1
+  else if (def_le(s1[0], s2[0])) then [s1[0]]+def_seq_merge(s1[1..], s2)
+  else [s2[0]]+def_seq_merge(s1, s2[1..])
+}
+function def_seq_sort(s: seq<def>): seq<def>
+{
+  if (s == []) then s else
+    var i: nat := (|s|-1)/2;
+    def_seq_merge(def_seq_sort(s[..i]), def_seq_sort(s[i+1..]))
+}
+ghost method lemma_def_le_trans(d1: def, d2: def, d3: def)
+  requires def_le(d1, d2);
+  requires def_le(d2, d3);
+  ensures def_le(d1, d3);
+{
+}
+ghost method lemma_def_le_comparable(d1: def, d2: def)
+  requires !def_le(d1, d2);
+  ensures def_le(d2, d1);
+{
+}
+ghost method lemma_def_seq_merging(s1: seq<def>, s2: seq<def>)
+  requires def_seq_sorted(s1) && def_seq_sorted(s2);
+  ensures def_seq_sorted(def_seq_merge(s1, s2));
+  ensures multiset((s1+s2)[..]) == multiset(def_seq_merge(s1,s2)[..]);
+{
+  if (s1 == []) {}
+  else if (s2 == []) {}
+  else if (def_le(s1[0], s2[0])) {
+    forall (n | 0 <= n < |s1|)
+      ensures def_le(s1[0], s1[n]);
+    {
+    }
+    forall (n | 0 <= n < |s2|)
+      ensures def_le(s1[0], s2[n]);
+    {
+      lemma_def_le_trans(s1[0], s2[0], s2[n]);
+    }
+    var sm := def_seq_merge(s1[1..], s2);
+    lemma_def_seq_merging(s1[1..], s2);
+    var s := [s1[0]]+sm;
+    assert def_le(s1[0], sm[0]);
+    forall (m,n | 0 <= m < n < |s|)
+      ensures def_le(s[m], s[n]);
+    {
+      if (m==0) {
+        lemma_def_le_trans(s1[0], sm[0], s[n]);
+      }
+    }
+  } else {
+    lemma_def_le_comparable(s1[0], s2[0]);
+    forall (n | 0 <= n < |s2|)
+      ensures def_le(s2[0], s2[n]);
+    {
+    }
+    forall (n | 0 <= n < |s1|)
+      ensures def_le(s2[0], s1[n]);
+    {
+      lemma_def_le_trans(s2[0], s1[0], s1[n]);
+    }
+    var sm := def_seq_merge(s1, s2[1..]);
+    lemma_def_seq_merging(s1, s2[1..]);
+    var s := [s2[0]]+sm;
+    assert def_le(s2[0], sm[0]);
+    forall (m,n | 0 <= m < n < |s|)
+      ensures def_le(s[m], s[n]);
+    {
+      if (m==0) {
+        lemma_def_le_trans(s2[0], sm[0], s[n]);
+      }
+    }
+  }  
+}
+ghost method lemma_def_seq_sorting(s: seq<def>)
+  ensures def_seq_sorted(def_seq_sort(s));
+  ensures multiset(s[..]) == multiset(def_seq_sort(s)[..]);
+{
+  if (s == []) {}
+  else {
+    var i: nat := (|s|-1)/2;
+    lemma_def_seq_sorting(s[..i]);
+    lemma_def_seq_sorting(s[i+1..]);
+    lemma_def_seq_merging(def_seq_sort(s[..i]), def_seq_sort(s[i+1..]));    
+  }
+}
+
+// ---------------------
+// Operational Semantics
+// ---------------------
+
+// ### Values ###
+predicate value(t: tm)
+{
+  t.tm_var?
+}
+
+// ### Store ###
+datatype store = Store(m: partial_map<int,pair<tp, list<def>>>);
+function store_lookup(n: nat, s: store): list<def>
+  requires n in dom(s.m);
+{
+  lookup(n, s.m).get.snd
+}
+function alloc(s: store): nat
+  ensures alloc(s) !in dom(s.m);
+{
+  other(dom(s.m))
+}
+function other(xs: seq<int>): nat
+{
+  max(xs, -1) + 1
+}
+function def_method_lookup(m: nat, defs: list<def>): option<pair<int, tm>>
+  ensures def_method_lookup(m, defs).Some? ==> def_method_lookup(m, defs).get.fst>=0;
+{
+  match defs
+  case Nil => None
+  case Cons(head, tail) =>
+    if (head.def_mt? && head.m==m) then Some(P(head.param, head.body))
+    else def_method_lookup(m, tail)
+}
+function def_field_lookup(l: nat, defs: list<def>): option<tm>
+{
+  match defs
+  case Nil => None
+  case Cons(head, tail) =>
+    if (head.def_tm? && head.l==l) then Some(head.t)
+    else def_field_lookup(l, tail)
+}
+
+// ### Size ###
+function tm_size(t: tm): nat
+  ensures t.tm_new? ==> tm_size(t)==1+tp_size(t.Tc)+defs_size(t.init)+tm_size(t.t');
+  ensures t.tm_new? ==> tm_size(t)>tp_size(t.Tc);
+  ensures t.tm_new? ==> tm_size(t)>defs_size(t.init);
+  ensures t.tm_new? ==> tm_size(t)>tm_size(t.t');
+  ensures t.tm_sel? ==> tm_size(t)==1+tm_size(t.t);
+  ensures t.tm_msel? ==> tm_size(t)==1+tm_size(t.o)+tm_size(t.a);
+  ensures t.tm_msel? ==> tm_size(t)>tm_size(t.o);
+{
+  match t
+  case tm_var(x') => 1
+  case tm_new(y, Tc, init, t1) => 1+tp_size(Tc)+defs_size(init)+tm_size(t1)
+  case tm_sel(t1, l) => 1+tm_size(t1)
+  case tm_msel(o, m, a) => 1+tm_size(o)+tm_size(a)
+}
+function tp_size(T: tp): nat
+  ensures T.tp_sel_c? ==> tp_size(T)==1+tm_size(T.pc);
+  ensures T.tp_sel_c? ==> tp_size(T)>tm_size(T.pc);
+  ensures T.tp_sel_a? ==> tp_size(T)==1+tm_size(T.pa);
+  ensures T.tp_sel_a? ==> tp_size(T)>tm_size(T.pa);
+  ensures T.tp_rfn? ==> tp_size(T)==1+tp_size(T.base_tp)+decls_size(T.decls);
+  ensures T.tp_rfn? ==> tp_size(T)>tp_size(T.base_tp);
+  ensures T.tp_rfn? ==> tp_size(T)>decls_size(T.decls);
+  ensures T.tp_and? ==> tp_size(T)==1+tp_size(T.and1)+tp_size(T.and2);
+  ensures T.tp_and? ==> tp_size(T)>tp_size(T.and1);
+  ensures T.tp_or? ==> tp_size(T)==1+tp_size(T.or1)+tp_size(T.or2);
+  ensures T.tp_or? ==> tp_size(T)>tp_size(T.or1);
+{
+  match T
+  case tp_sel_c(pc, Lc) => 1+tm_size(pc)
+  case tp_sel_a(pa, La) => 1+tm_size(pa)
+  case tp_rfn(base_tp, self, decls) => 1+tp_size(base_tp)+decls_size(decls)
+  case tp_and(and1, and2) => 1+tp_size(and1)+tp_size(and2)
+  case tp_or(or1, or2) => 1+tp_size(or1)+tp_size(or2)
+  case tp_top => 1
+  case tp_bot => 1
+}
+function def_size(d: def): nat
+  ensures d.def_tm? ==> def_size(d)==1+tm_size(d.t);
+  ensures d.def_tm? ==> def_size(d)>tm_size(d.t);
+  ensures d.def_mt? ==> def_size(d)==1+tm_size(d.body);
+  ensures d.def_mt? ==> def_size(d)>tm_size(d.body);
+{
+  match d
+  case def_tm(l, t1) => 1+tm_size(t1)
+  case def_mt(m, param, body) => 1+tm_size(body)
+}
+function decl_size(d: decl): nat
+  ensures d.decl_tp_c? ==> decl_size(d)==1+tp_size(d.Sc)+tp_size(d.Uc);
+  ensures d.decl_tp_c? ==> decl_size(d)>tp_size(d.Sc);
+  ensures d.decl_tp_c? ==> decl_size(d)>tp_size(d.Uc);
+  ensures d.decl_tp_a? ==> decl_size(d)==1+tp_size(d.Sa)+tp_size(d.Ua);
+  ensures d.decl_tp_a? ==> decl_size(d)>tp_size(d.Sa);
+  ensures d.decl_tp_a? ==> decl_size(d)>tp_size(d.Ua);
+  ensures d.decl_tm? ==> decl_size(d)==1+tp_size(d.T);
+  ensures d.decl_tm? ==> decl_size(d)>tp_size(d.T);
+  ensures d.decl_mt? ==> decl_size(d)==1+tp_size(d.P)+tp_size(d.R);
+  ensures d.decl_mt? ==> decl_size(d)>tp_size(d.P);
+  ensures d.decl_mt? ==> decl_size(d)>tp_size(d.R);
+{
+  match d
+  case decl_tp_c(Lc, Sc, Uc) => 1+tp_size(Sc)+tp_size(Uc)
+  case decl_tp_a(La, Sa, Ua) => 1+tp_size(Sa)+tp_size(Ua)
+  case decl_tm(l, T) => 1+tp_size(T)
+  case decl_mt(m, P, R) => 1+tp_size(P)+tp_size(R)
+}
+function defs_size(defs: list<def>): nat
+  ensures defs.Cons? ==> defs_size(defs)==1+def_size(defs.head)+defs_size(defs.tail);
+  ensures defs.Cons? ==> defs_size(defs)>def_size(defs.head);
+{
+  match defs
+  case Nil => 1
+  case Cons(head, tail) => 1+def_size(head)+defs_size(tail)
+}
+function decls_size(decls: list<decl>): nat
+  ensures decls.Cons? ==> decls_size(decls)==1+decl_size(decls.head)+decls_size(decls.tail);
+  ensures decls.Cons? ==> decls_size(decls)>decl_size(decls.head);
+{
+  match decls
+  case Nil => 1
+  case Cons(head, tail) => 1+decl_size(head)+decls_size(tail)
+}
+
+// ### Substitution ###
+function tm_subst(x: nat, v: tm, t: tm): tm
+  decreases tm_size(t), t;
+  ensures v.tm_var? ==> tm_size(t)==tm_size(tm_subst(x, v, t));
+{
+  match t
+  case tm_var(x') => if x'==x then v else t
+  case tm_new(y, Tc, init, t1) =>
+    if y==x then tm_new(y, tp_subst(x, v, Tc), init, t1) else
+    var y' := if (tm_fn(y, v)) then other([x]+tm_vars(v)+tm_vars(t)) else y;
+    var init' := if (y==y') then init else defs_subst(y, tm_var(y'), init);
+    var t1' := if (y==y') then t1 else tm_subst(y, tm_var(y'), t1);
+    tm_new(y', tp_subst(x, v, Tc), defs_subst(x, v, init'), tm_subst(x, v, t1'))
+  case tm_sel(t1, l) => tm_sel(tm_subst(x, v, t1), l)
+  case tm_msel(o, m, a) => tm_msel(tm_subst(x, v, o), m, tm_subst(x, v, a))
+}
+function tp_subst(x: nat, v: tm, T: tp): tp
+  decreases tp_size(T), T;
+  ensures v.tm_var? ==> tp_size(T)==tp_size(tp_subst(x, v, T));
+{
+  match T
+  case tp_sel_c(pc, Lc) => tp_sel_c(tm_subst(x, v, pc), Lc)
+  case tp_sel_a(pa, La) => tp_sel_a(tm_subst(x, v, pa), La)
+  case tp_rfn(base_tp, self, decls) =>
+    if self==x then tp_rfn(tp_subst(x, v, base_tp), self, decls) else
+    var self' := if (tm_fn(self, v)) then other([x]+tm_vars(v)+tp_vars(T)) else self;
+    var decls' := if (self==self') then decls else decls_subst(self, tm_var(self'), decls);
+    tp_rfn(tp_subst(x, v, base_tp), self', decls_subst(x, v, decls'))
+  case tp_and(and1, and2) => tp_and(tp_subst(x, v, and1), tp_subst(x, v, and2))
+  case tp_or(or1, or2) => tp_or(tp_subst(x, v, or1), tp_subst(x, v, or2))
+  case tp_top => T
+  case tp_bot => T
+}
+function def_subst(x: nat, v: tm, d: def): def
+  decreases def_size(d), d;
+  ensures v.tm_var? ==> def_size(d)==def_size(def_subst(x, v, d));
+{
+  match d
+  case def_tm(l, t1) => def_tm(l, tm_subst(x, v, t1))
+  case def_mt(m, param, body) =>
+    if param==x then d else
+    var param' := if (tm_fn(param, v)) then other([x]+tm_vars(v)+def_vars(d)) else param;
+    var body' := if (param==param') then body else tm_subst(param, tm_var(param'), body);
+    def_mt(m, param', tm_subst(x, v, body'))
+}
+function decl_subst(x: nat, v: tm, d: decl): decl
+  decreases decl_size(d), d;
+  ensures v.tm_var? ==> decl_size(d)==decl_size(decl_subst(x, v, d));
+{
+  match d
+  case decl_tp_c(Lc, Sc, Uc) => decl_tp_c(Lc, tp_subst(x, v, Sc), tp_subst(x, v, Uc))
+  case decl_tp_a(La, Sa, Ua) => decl_tp_a(La, tp_subst(x, v, Sa), tp_subst(x, v, Ua))
+  case decl_tm(l, T) => decl_tm(l, tp_subst(x, v, T))
+  case decl_mt(m, P, R) => decl_mt(m, tp_subst(x, v, P), tp_subst(x, v, R))
+}
+function defs_subst(x: nat, v: tm, defs: list<def>): list<def>
+  decreases defs_size(defs), defs;
+  ensures v.tm_var? ==> defs_size(defs)==defs_size(defs_subst(x, v, defs));
+{
+  match defs
+  case Nil => Nil
+  case Cons(head, tail) => Cons(def_subst(x, v, head), defs_subst(x, v, tail))
+}
+function decls_subst(x: nat, v: tm, decls: list<decl>): list<decl>
+  decreases decls_size(decls), decls;
+  ensures v.tm_var? ==> decls_size(decls)==decls_size(decls_subst(x, v, decls));
+{
+  match decls
+  case Nil => Nil
+  case Cons(head, tail) => Cons(decl_subst(x, v, head), decls_subst(x, v, tail))
+}
+function decls_fin_subst(x: nat, v: tm, decls: seq<decl>): seq<decl>
+{
+  lst2seq(decls_subst(x, v, seq2lst(decls)))
+}
+
+// ### Free variables ###
+// fn(x, A) <==> x appears free in A
+
+predicate tm_fn(x: nat, t: tm)
+{
+  match t
+  case tm_var(x') => x'==x
+  case tm_new(y, Tc, init, t') => tp_fn(x, Tc) || (y!=x && (defs_fn(x, init) || tm_fn(x, t')))
+  case tm_sel(t1, l) => tm_fn(x, t1)
+  case tm_msel(o, m, a) => tm_fn(x, o) || tm_fn(x, a)
+}
+predicate tp_fn(x: nat, T: tp)
+{
+  match T
+  case tp_sel_c(pc, Lc) => tm_fn(x, pc)
+  case tp_sel_a(pa, La) => tm_fn(x, pa)
+  case tp_rfn(base_tp, self, decls) => tp_fn(x, base_tp) || (self!=x && decls_fn(x, decls))
+  case tp_and(and1, and2) => tp_fn(x, and1) || tp_fn(x, and2)
+  case tp_or(or1, or2) => tp_fn(x, or1) || tp_fn(x, or2)
+  case tp_top => false
+  case tp_bot => false
+}
+predicate def_fn(x: nat, d: def)
+{
+  match d
+  case def_tm(l, t1) => tm_fn(x, t1)
+  case def_mt(m, param, body) => param!=x && tm_fn(x, body)
+}
+predicate decl_fn(x: nat, d: decl)
+{
+  match d
+  case decl_tp_c(Lc, Sc, Uc) => tp_fn(x, Sc) || tp_fn(x, Uc)
+  case decl_tp_a(La, Sa, Ua) => tp_fn(x, Sa) || tp_fn(x, Ua)
+  case decl_tm(l, T) => tp_fn(x, T)
+  case decl_mt(m, P, R) => tp_fn(x, P) || tp_fn(x, R)
+}
+predicate defs_fn(x: nat, defs: list<def>)
+{
+  defs.Cons? && (def_fn(x, defs.head) || defs_fn(x, defs.tail))
+}
+predicate decls_fn(x: nat, decls: list<decl>)
+{
+  decls.Cons? && (decl_fn(x, decls.head) || decls_fn(x, decls.tail))
+}
+
+// ### Variables ###
+function tm_vars(t: tm): seq<int>
+  ensures forall x :: x in tm_vars(t) ==> x>=0;
+{
+  match t
+  case tm_var(x') => [x']
+  case tm_new(y, Tc, init, t') => [y]+tp_vars(Tc)+defs_vars(init)+tm_vars(t')
+  case tm_sel(t1, l) => tm_vars(t1)
+  case tm_msel(o, m, a) => tm_vars(o)+tm_vars(a)
+}
+function tp_vars(T: tp): seq<int>
+  ensures forall x :: x in tp_vars(T) ==> x>=0;
+{
+  match T
+  case tp_sel_c(pc, Lc) => tm_vars(pc)
+  case tp_sel_a(pa, La) => tm_vars(pa)
+  case tp_rfn(base_tp, self, decls) => tp_vars(base_tp)+[self]+decls_vars(decls)
+  case tp_and(and1, and2) => tp_vars(and1)+tp_vars(and2)
+  case tp_or(or1, or2) => tp_vars(or1)+tp_vars(or2)
+  case tp_top => []
+  case tp_bot => []
+}
+function def_vars(d: def): seq<int>
+  ensures forall x :: x in def_vars(d) ==> x>=0;
+{
+  match d
+  case def_tm(l, t1) => tm_vars(t1)
+  case def_mt(m, param, body) => [param]+tm_vars(body)
+}
+function decl_vars(d: decl): seq<int>
+  ensures forall x :: x in decl_vars(d) ==> x>=0;
+{
+  match d
+  case decl_tp_c(Lc, Sc, Uc) => tp_vars(Sc)+tp_vars(Uc)
+  case decl_tp_a(La, Sa, Ua) => tp_vars(Sa)+tp_vars(Ua)
+  case decl_tm(l, T) => tp_vars(T)
+  case decl_mt(m, P, R) => tp_vars(P)+tp_vars(R)
+}
+function defs_vars(defs: list<def>): seq<int>
+  ensures forall x :: x in defs_vars(defs) ==> x>=0;
+{
+  match defs
+  case Nil => []
+  case Cons(head, tail) => def_vars(head)+defs_vars(tail)
+}
+function decls_vars(decls: list<decl>): seq<int>
+  ensures forall x :: x in decls_vars(decls) ==> x>=0;
+{
+  match decls
+  case Nil => []
+  case Cons(head, tail) => decl_vars(head)+decls_vars(tail)
+}
+
+// ### Reduction ###
+function step(t: tm, s: store): option<pair<tm, store>>
+  ensures step(t, s).Some? ==> prefix_of(step(t, s).get.snd.m, s.m);
+{
+  /* msel */
+  if (t.tm_msel? && t.o.tm_var? && value(t.a) && t.o.x in dom(s.m) &&
+     def_method_lookup(t.m, store_lookup(t.o.x, s)).Some?)
+  then Some(P(tm_subst(def_method_lookup(t.m, store_lookup(t.o.x, s)).get.fst,
+                       t.a,
+                       def_method_lookup(t.m, store_lookup(t.o.x, s)).get.snd),
+              s))
+  /* msel1 */
+  else if (t.tm_msel? && step(t.o, s).Some?)
+  then Some(P(tm_msel(step(t.o, s).get.fst, t.m, t.a), step(t.o, s).get.snd))
+  /* msel2 */
+  else if (t.tm_msel? && value(t.o) && step(t.a, s).Some?)
+  then Some(P(tm_msel(t.o, t.m, step(t.a, s).get.fst), step(t.a, s).get.snd))
+  /* sel */
+  else if (t.tm_sel? && t.t.tm_var? && t.t.x in dom(s.m) &&
+           def_field_lookup(t.l, store_lookup(t.t.x, s)).Some?)
+  then Some(P(def_field_lookup(t.l, store_lookup(t.t.x, s)).get, s))
+  /* sel1 */
+  else if (t.tm_sel? && step(t.t, s).Some?)
+  then Some(P(tm_sel(step(t.t, s).get.fst, t.l), step(t.t, s).get.snd))
+  /* new */
+  else if (t.tm_new?)
+  then Some(P(tm_subst(t.y, tm_var(alloc(s)), t.t'),
+              Store(Extend(alloc(s), P(t.Tc, defs_subst(t.y, tm_var(alloc(s)), t.init)), s.m))))
+  else None
+}
+
+predicate irred(t: tm, s: store)
+{
+  step(t, s).None?
+}
+
+// ### Multi-steps ###
+predicate mstep(t: tm, s: store, t': tm, s': store, n: nat)
+  //ensures mstep(t, s, t', s', n) ==> prefix_of(s'.m, s.m);
+  decreases n;
+{
+  if (n==0) then t==t' && s==s'
+  else step(t, s).Some? && mstep(step(t, s).get.fst, step(t, s).get.snd, t', s', n-1)
+}
+
+// ### Properties of Operational Semantics ###
+
+ghost method lemma_value__irred(t: tm, s: store)
+  requires value(t);
+  ensures irred(t, s);
+{
+}
+
+ghost method lemma_step__prefix(t1: tm, s1: store, t2: tm, s2: store)
+  requires step(t1, s1) == Some(P(t2, s2));
+  ensures prefix_of(s2.m, s1.m);
+{
+}
+
+ghost method lemma_mstep__prefix(t1: tm, s1: store, t2: tm, s2: store, n: nat)
+  requires mstep(t1, s1, t2, s2, n);
+  ensures prefix_of(s2.m, s1.m);
+  decreases n;
+{
+  if (n>0) {
+    lemma_step__prefix(t1, s1, step(t1, s1).get.fst, step(t1, s1).get.snd);
+    lemma_mstep__prefix(step(t1, s1).get.fst, step(t1, s1).get.snd, t2, s2, n-1);
+    lemma_prefix_of_trans(s1.m, step(t1, s1).get.snd.m, s2.m);
+  }
+}
+
+ghost method lemma_mstep_trans(t1: tm, s1: store, t2: tm, s2: store, t3: tm, s3: store, n12: nat, n23: nat)
+  requires mstep(t1, s1, t2, s2, n12);
+  requires mstep(t2, s2, t3, s3, n23);
+  ensures mstep(t1, s1, t3, s3, n12+n23);
+  decreases n12+n23;
+{
+  if (n12>0) {
+    lemma_mstep_trans(step(t1, s1).get.fst, step(t1, s1).get.snd, t2, s2, t3, s3, n12-1, n23);
+  } else if (n23>0) {
+    lemma_mstep_trans(step(t1, s1).get.fst, step(t1, s1).get.snd, step(t2, s2).get.fst, step(t2, s2).get.snd, t3, s3, n12, n23-1);
+  }
+}
+
+ghost method lemma_mstep_trans'(t1: tm, s1: store, t2: tm, s2: store, t3: tm, s3: store, n12: nat, n13: nat)
+  requires n12 <= n13;
+  requires mstep(t1, s1, t2, s2, n12);
+  requires mstep(t1, s1, t3, s3, n13);
+  ensures mstep(t2, s2, t3, s3, n13-n12);
+  decreases n12;
+{
+  if (n12>0 && n13>0) {
+    lemma_mstep_trans'(step(t1, s1).get.fst, step(t1, s1).get.snd, t2, s2, t3, s3, n12-1, n13-1);
+  }
+}
+
+// ### Congruence Lemmas ###
+
+ghost method lemma_mstep_sel(o: tm, l: nat, o': tm, s: store, s': store, oi: nat)
+  requires mstep(o, s, o', s', oi);
+  ensures mstep(tm_sel(o, l), s, tm_sel(o', l), s', oi);
+  decreases oi;
+{
+  if (oi>0) {
+    lemma_mstep_sel(step(o, s).get.fst, l, o', step(o, s).get.snd, s', oi-1);
+  }
+}
+
+ghost method lemma_sel_irred__o_mstep_irred(o: tm, l: nat, t': tm, s: store, s': store, i: nat) returns (o': tm, so': store, oi: nat)
+  requires mstep(tm_sel(o, l), s, t', s', i);
+  requires irred(t', s');
+  ensures oi<=i && mstep(o, s, o', so', oi) && irred(o', so');
+  decreases i;
+{
+  if (irred(o, s)) {
+    o' := o;
+	  so' := s;
+    oi := 0;
+  } else {
+    assert step(o, s).Some?;
+    lemma_mstep_trans'(tm_sel(o, l), s, tm_sel(step(o, s).get.fst, l), step(o, s).get.snd, t', s', 1, i);
+    var o'', so'', oi' := lemma_sel_irred__o_mstep_irred(step(o, s).get.fst, l, t', step(o, s).get.snd, s', i-1);
+    lemma_mstep_trans(o, s, step(o, s).get.fst, step(o, s).get.snd, o'', so'', 1, oi');
+    o' := o'';
+  	so' := so'';
+    oi := oi'+1;
+  }
+}
+
+// -----------
+// Type System
+// -----------
+
+// ### Context ###
+datatype context = Context(m: partial_map<int,tp>);
+function ctx_extend(x: nat, T: tp, ctx: context): context
+  ensures ctx_extend(x, T, ctx).m == Extend(x, T, ctx.m);
+  ensures prefix_of(ctx_extend(x, T, ctx).m, ctx.m);
+{
+  Context(Extend(x, T, ctx.m))
+}
+
+// ### Declaration Lattice ###
+predicate decl_bot(d: decl)
+{
+  match d
+  case decl_tp_c(L, S, U) => S==tp_top && U==tp_bot
+  case decl_tp_a(L, S, U) => S==tp_top && U==tp_bot
+  case decl_tm(l, T) => T==tp_bot
+  case decl_mt(m, S, U) => S==tp_top && U==tp_bot
+}
+function decl_and(d1: decl, d2: decl): decl
+  requires decl_eq(d1, d2);
+  ensures decl_eq(d1, decl_and(d1, d2));
+  ensures decl_eq(d2, decl_and(d1, d2));
+{
+  match d1
+  case decl_tp_c(L, S, U) => decl_tp_c(L, tp_or(S, d2.Sc), tp_and(U, d2.Uc))
+  case decl_tp_a(L, S, U) => decl_tp_a(L, tp_or(S, d2.Sa), tp_and(U, d2.Ua))
+  case decl_tm(l, U) => decl_tm(l, tp_and(U, d2.T))
+  case decl_mt(m, S, U) => decl_mt(m, tp_or(S, d2.P), tp_and(U, d2.R))
+}
+function decl_or(d1: decl, d2: decl): decl
+  requires decl_eq(d1, d2);
+  ensures decl_eq(d1, decl_or(d1, d2));
+  ensures decl_eq(d2, decl_or(d1, d2));
+{
+  match d1
+  case decl_tp_c(L, S, U) => decl_tp_c(L, tp_and(S, d2.Sc), tp_or(U, d2.Uc))
+  case decl_tp_a(L, S, U) => decl_tp_a(L, tp_and(S, d2.Sa), tp_or(U, d2.Ua))
+  case decl_tm(l, U) => decl_tm(l, tp_or(U, d2.T))
+  case decl_mt(m, S, U) => decl_mt(m, tp_and(S, d2.P), tp_or(U, d2.R))
+}
+function decls_fin_and(s1: seq<decl>, s2: seq<decl>): seq<decl>
+  requires decl_seq_sorted(s1);
+  requires decl_seq_sorted(s2);
+  //ensures decl_seq_sorted(decls_fin_and(s1, s2));
+{
+        if (s1 == []) then s2
+  else  if (s2 == []) then s1
+  else  if (decl_eq(s1[0], s2[0])) then   [decl_and(s1[0], s2[0])]+decls_fin_and(s1[1..], s2[1..])
+  else  if (decl_lt(s1[0], s2[0])) then   [s1[0]]+decls_fin_and(s1[1..], s2)
+  else/*if (decl_lt(s2[0], s1[0])) then*/ [s2[0]]+decls_fin_and(s1, s2[1..])
+}
+function decls_and(Ds1: decls, Ds2: decls): decls
+  requires Ds1.decls_fin? ==> decl_seq_sorted(Ds1.decls);
+  requires Ds2.decls_fin? ==> decl_seq_sorted(Ds2.decls);
+  //ensures decls_and(Ds1, Ds2).decls_fin? ==> decl_seq_sorted(decls_and(Ds1, Ds2).decls); 
+{
+  match Ds1
+  case decls_bot => decls_bot
+  case decls_fin(s1) =>
+    (match Ds2
+     case decls_bot => decls_bot
+     case decls_fin(s2) => decls_fin(decls_fin_and(s1, s2)))
+}
+function decls_fin_or(s1: seq<decl>, s2: seq<decl>): seq<decl>
+  requires decl_seq_sorted(s1);
+  requires decl_seq_sorted(s2);
+  //ensures decl_seq_sorted(decls_fin_or(s1, s2));
+{
+        if (s1 == []) then []
+  else  if (s2 == []) then []
+  else  if (decl_eq(s1[0], s2[0])) then   [decl_or(s1[0], s2[0])]+decls_fin_and(s1[1..], s2[1..])
+  else  if (decl_lt(s1[0], s2[0])) then   decls_fin_or(s1[1..], s2)
+  else/*if (decl_lt(s2[0], s1[0])) then*/ decls_fin_or(s1, s2[1..])
+}
+function decls_or(Ds1: decls, Ds2: decls): decls
+  requires Ds1.decls_fin? ==> decl_seq_sorted(Ds1.decls);
+  requires Ds2.decls_fin? ==> decl_seq_sorted(Ds2.decls);
+  //ensures decls_or(Ds1, Ds2).decls_fin? ==> decl_seq_sorted(decls_or(Ds1, Ds2).decls); 
+{
+  match Ds1
+  case decls_bot => Ds2
+  case decls_fin(s1) =>
+    (match Ds2
+     case decls_bot => Ds1
+     case decls_fin(s2) => decls_fin(decls_fin_or(s1, s2)))
+}
+
+// ### Typing-Related Judgments ###
+
+copredicate typing(ctx: context, t: tm, T: tp)
+{
+  match t
+  case tm_var(x) => lookup(x, ctx.m) == Some(T)
+  case tm_new(y, Tc, init, t') =>
+    exists Ds:decls :: Ds.decls_fin? &&
+    wfe_type(ctx, Tc) &&
+    expansion(ctx, y, Tc, Ds) && 
+    wf_init(Context(Extend(y, Tc, ctx.m)), Ds.decls, def_seq_sort(lst2seq(init))) &&
+    !tp_fn(y, T) &&
+    typing(Context(Extend(y, Tc, ctx.m)), t', T)
+  case tm_sel(t, l) =>
+    field_membership(ctx, t, l, T)
+  case tm_msel(o, m, a) =>
+    exists S, T' :: method_membership(ctx, o, m, S, T) &&
+    typing(ctx, a, T') &&
+    subtype(ctx, T', S)
+}
+copredicate wf_init(ctx: context, decls: seq<decl>, defs: seq<def>)
+  //requires decl_seq_sorted(decls);
+  //requires def_seq_sorted(defs);
+{
+  (decls==[] && defs==[]) || (|decls|>0 && (
+    (((decls[0].decl_tp_c? && subtype(ctx, decls[0].Sc, decls[0].Uc)) ||
+      (decls[0].decl_tp_a? && subtype(ctx, decls[0].Sa, decls[0].Ua))) &&
+     wf_init(ctx, decls[1..], defs)) || (|defs|>0 && (
+    ((decls[0].decl_tm? && defs[0].def_tm? && decls[0].l==defs[0].l &&
+      value(defs[0].t) &&
+      exists T :: typing(ctx, defs[0].t, T) &&
+      subtype(ctx, T, decls[0].T)) ||
+     (decls[0].decl_mt? && defs[0].def_mt? && decls[0].m==defs[0].m &&
+      wfe_type(ctx, decls[0].P) &&
+      exists T' :: typing(Context(Extend(defs[0].param, decls[0].P, ctx.m)), defs[0].body, T') &&
+      subtype(Context(Extend(defs[0].param, decls[0].P, ctx.m)), T', decls[0].R))) &&
+     wf_init(ctx, decls[1..], defs[1..])))))
+}
+copredicate wf_decl(ctx: context, d: decl)
+{
+  match d
+  case decl_tp_c(L, S, U) => wf_type(ctx, S) && wf_type(ctx, U)
+  case decl_tp_a(L, S, U) => wf_type(ctx, S) && wf_type(ctx, U)
+  case decl_tm(l, T) => wf_type(ctx, T)
+  case decl_mt(m, S, T) => wf_type(ctx, S) && wf_type(ctx, T)
+}
+copredicate wf_decls(ctx: context, Ds: list<decl>)
+{
+  match Ds
+  case Nil => true
+  case Cons(head, tail) => wf_decl(ctx, head) && wf_decls(ctx, tail)
+}
+copredicate wf_type(ctx: context, T: tp)
+{
+  match T
+  case tp_rfn(T', z, Ds) =>
+    wf_type(ctx, T') && wf_decls(Context(Extend(z, T, ctx.m)), Ds)
+  case tp_sel_c(p, L) =>
+    path(p) &&
+    exists S, U :: concrete_type_membership(ctx, p, L, S, U)
+  case tp_sel_a(p, L) =>
+    path(p) &&
+    exists S, U :: abstract_type_membership(ctx, p, L, S, U)
+  case tp_and(T1, T2) => wf_type(ctx, T1) && wf_type(ctx, T2)
+  case tp_or(T1, T2) => wf_type(ctx, T1) && wf_type(ctx, T2)
+  case tp_top => true
+  case tp_bot => true
+}
+copredicate wfe_type(ctx: context, T: tp)
+{
+  wf_type(ctx, T) && exists Ds :: expansion(ctx, 0, T, Ds)
+}
+copredicate membership(ctx: context, t: tm, l: nat, d: decl)
+{
+  decl_label(d)==l &&
+  exists T :: typing(ctx, t, T) &&
+  forall z:nat :: !tp_fn(z, T) && z !in dom(ctx.m) && !tm_fn(z, t) ==>
+  exists Ds ::
+  expansion(ctx, z, T, Ds) &&
+  ((Ds.decls_fin? &&
+     ((path(t) && exists d' :: d' in Ds.decls && d==decl_subst(z, t, d')) ||
+     (!path(t) && d in Ds.decls && !decl_fn(z, d)))) ||
+   (Ds.decls_bot? && decl_bot(d)))
+}
+copredicate field_membership(ctx: context, t: tm, l: nat, T: tp)
+{
+  membership(ctx, t, l, decl_tm(l, T))
+}
+copredicate method_membership(ctx: context, t: tm, m: nat, P: tp, R: tp)
+{
+  exists d :: membership(ctx, t, m, d) &&
+  d.decl_mt? && d.m==m && d.P==P && d.R==R
+}
+copredicate concrete_type_membership(ctx: context, t: tm, L: nat, S: tp, U: tp)
+{
+  exists d :: membership(ctx, t, L, d) &&
+  d.decl_tp_c? && d.Lc==L && d.Sc==S && d.Uc==U
+}
+copredicate abstract_type_membership(ctx: context, t: tm, L: nat, S: tp, U: tp)
+{
+  exists d :: membership(ctx, t, L, d) &&
+  d.decl_tp_a? && d.La==L && d.Sa==S && d.Ua==U
+}
+predicate m_decl_seq_sorted(m: partial_map<tp, decls>)
+{
+  match m
+  case Empty => true
+  case Extend(x, v, rest) => (v.decls_fin? ==> decl_seq_sorted(v.decls)) && m_decl_seq_sorted(rest)
+}
+copredicate expansion(ctx: context, z: nat, T: tp, Ds: decls)
+  ensures expansion(ctx, z, T, Ds) && Ds.decls_fin? ==> decl_seq_sorted(Ds.decls);
+{
+  expansion_iter(Empty, ctx, z, T, Ds)
+}
+copredicate expansion_iter(m: partial_map<tp, decls>, ctx: context, z: nat, T: tp, Ds: decls)
+  requires m_decl_seq_sorted(m);
+  ensures expansion_iter(m, ctx, z, T, Ds) && Ds.decls_fin? ==> decl_seq_sorted(Ds.decls);
+{
+  match T
+  case tp_rfn(T', z', Ds') =>
+    exists DsT :: expansion_iter(m, ctx, z, T, DsT) &&
+    exists rfn_decls :: rfn_decls==decl_seq_sort(lst2seq(decls_subst(z', tm_var(z), Ds'))) &&
+    decl_seq_sorted(rfn_decls) &&
+    Ds==decls_and(decls_fin(rfn_decls), DsT) &&
+    (Ds.decls_fin? ==> decl_seq_sorted(Ds.decls))
+  case tp_sel_c(p, L) =>
+    (lookup(T, m).Some? && lookup(T, m).get==Ds && (Ds.decls_fin? ==> decl_seq_sorted(Ds.decls))) || 
+    (lookup(T, m).None? && exists S, U :: concrete_type_membership(ctx, p, L, S, U) && expansion_fix(T, decls_fin([]), m, ctx, z, U, Ds))
+  case tp_sel_a(p, L) =>
+    (lookup(T, m).Some? && lookup(T, m).get==Ds && (Ds.decls_fin? ==> decl_seq_sorted(Ds.decls))) || 
+    (lookup(T, m).None? && exists S, U :: abstract_type_membership(ctx, p, L, S, U) && expansion_fix(T, decls_fin([]), m, ctx, z, U, Ds))
+  case tp_and(T1, T2) =>
+    exists Ds1, Ds2 :: expansion_iter(m, ctx, z, T1, Ds1) && expansion_iter(m, ctx, z, T2, Ds2) &&
+    Ds==decls_and(Ds1, Ds2) &&
+    (Ds.decls_fin? ==> decl_seq_sorted(Ds.decls))
+  case tp_or(T1, T2) =>
+    exists Ds1, Ds2 :: expansion_iter(m, ctx, z, T1, Ds1) && expansion_iter(m, ctx, z, T2, Ds2) &&
+    Ds==decls_or(Ds1, Ds2) &&
+    (Ds.decls_fin? ==> decl_seq_sorted(Ds.decls))
+  case tp_top => Ds==decls_fin([])
+  case tp_bot => Ds==decls_bot
+}
+copredicate expansion_fix(selT: tp, selDs: decls, m: partial_map<tp, decls>, ctx: context, z: nat, T: tp, Ds: decls)
+  requires m_decl_seq_sorted(m);
+  requires selDs.decls_fin? ==> decl_seq_sorted(selDs.decls);
+  ensures expansion_fix(selT, selDs, m, ctx, z, T, Ds) && Ds.decls_fin? ==> decl_seq_sorted(Ds.decls);
+{
+  (selDs==Ds && expansion_iter(Extend(selT, selDs, m), ctx, z, T, Ds)) ||
+  (selDs!=Ds && exists Da :: expansion_iter(Extend(selT, selDs, m), ctx, z, T, Da) &&
+   expansion_fix(selT, Da, m, ctx, z, T, Ds))
+}
+copredicate decl_sub(ctx: context, d1: decl, d2: decl)
+  requires decl_eq(d1, d2);
+{
+  match d1
+  case decl_tp_c(L, S, U) => subtype(ctx, d2.Sc, S) && subtype(ctx, U, d2.Uc)
+  case decl_tp_a(L, S, U) => subtype(ctx, d2.Sa, S) && subtype(ctx, U, d2.Ua)
+  case decl_tm(l, U) => subtype(ctx, U, d2.T)
+  case decl_mt(m, S, U) => subtype(ctx, d2.P, S) && subtype(ctx, U, d2.R)
+}
+copredicate decls_fin_sub(ctx: context, s1: seq<decl>, s2: seq<decl>)
+  requires decl_seq_sorted(s1);
+  requires decl_seq_sorted(s2);
+{
+  (s1 == [] && s2 == []) ||
+  (|s1|>0 && |s2|>0 && (
+  (decl_eq(s1[0], s2[0]) && decl_sub(ctx, s1[0], s2[0]) &&
+   decls_fin_sub(ctx, s1[1..], s2[1..])) ||
+  (decl_lt(s1[0], s2[0]) && decls_fin_sub(ctx, s1[1..], s2))))
+}
+copredicate decls_sub(ctx: context, Ds1: decls, Ds2: decls)
+  requires Ds1.decls_fin? ==> decl_seq_sorted(Ds1.decls);
+  requires Ds2.decls_fin? ==> decl_seq_sorted(Ds2.decls);
+{
+  match Ds1
+  case decls_bot => true
+  case decls_fin(s1) =>
+    (match Ds2
+     case decls_bot => false
+     case decls_fin(s2) => decls_fin_sub(ctx, s1, s2))
+}
+copredicate subtype(ctx: context, S: tp, T: tp)
+{
+  /* refl */    (S==T && wfe_type(ctx, T)) ||
+  /* <:-top */  (T.tp_top? && wfe_type(ctx, S)) ||
+  /* bot-<: */  (S.tp_bot? && wfe_type(ctx, T)) ||
+  /* <:-rfn */  (T.tp_rfn? && wfe_type(ctx, T) && subtype(ctx, S, T.base_tp) &&
+                 exists Ds' :: expansion(ctx, T.self, S, Ds') &&
+                 exists rfn_decls :: rfn_decls==decl_seq_sort(lst2seq(T.decls)) &&
+                 decl_seq_sorted(rfn_decls) &&
+                 decls_sub(Context(Extend(T.self, S, ctx.m)), decls_fin(rfn_decls), Ds')) ||
+  /* rfn-<: */  (S.tp_rfn? && wfe_type(ctx, S) && subtype(ctx, S.base_tp, T)) ||
+  /* <:-selc */ (T.tp_sel_c? &&
+                 exists S', U' :: concrete_type_membership(ctx, T.pc, T.Lc, S', U') &&
+                 subtype(ctx, S', U') && subtype(ctx, S, S')) ||
+  /* selc-<: */ (S.tp_sel_c? &&
+                 exists S', U' :: concrete_type_membership(ctx, S.pc, S.Lc, S', U') &&
+                 subtype(ctx, S', U') && subtype(ctx, U', T)) ||
+  /* <:-sela */ (T.tp_sel_a? &&
+                 exists S', U' :: abstract_type_membership(ctx, T.pa, T.La, S', U') &&
+                 subtype(ctx, S', U') && subtype(ctx, S, S')) ||
+  /* sela-<: */ (S.tp_sel_a? &&
+                 exists S', U' :: abstract_type_membership(ctx, S.pa, S.La, S', U') &&
+                 subtype(ctx, S', U') && subtype(ctx, U', T)) ||
+  /* <:-and */  (T.tp_and? && subtype(ctx, S, T.and1) && subtype(ctx, S, T.and2)) ||
+  /* and1-<: */ (S.tp_and? && wfe_type(ctx, S.and2) && subtype(ctx, S.and1, T)) ||
+  /* and2-<: */ (S.tp_and? && wfe_type(ctx, S.and1) && subtype(ctx, S.and2, T)) ||
+  /* <:-or1 */  (T.tp_or? && wfe_type(ctx, T.or2) && subtype(ctx, S, T.or1)) ||
+  /* <:-or2 */  (T.tp_or? && wfe_type(ctx, T.or1) && subtype(ctx, S, T.or2)) ||
+  /* or-<: */   (S.tp_or? && subtype(ctx, S.or1, T) && subtype(ctx, S.or2, T))
+}
+
+// ### Properties of typing judgments ###
+
+ghost method lemma_field_mem__expansion_decl(ctx: context, t1: tm, T1: tp, l: nat, T: tp, ctx': context, z: nat, Ds: decls)
+  requires field_membership(ctx, t1, l, T);
+  requires typing(ctx, t1, T1);
+  requires expansion(ctx', z, T1, Ds) && Ds.decls_fin?;
+  ensures exists U :: decl_tm(l, U) in Ds.decls;
+{
+  assume exists U :: decl_tm(l, U) in Ds.decls; // TODO...
+}
+
+// -----------------
+// Logical Relations
+// -----------------
+
+predicate V(T: tp, t: tm, k: nat, ctx: context, s: store)
+  requires A(k, ctx, s);
+  decreases k, k; // weird!
+{
+  t.tm_var? && t.x in dom(s.m) &&
+  wfe_type(ctx, T) &&
+  (exists Tc, init :: P(Tc, init) == lookup(t.x, s.m).get) &&
+  (exists Ds :: expansion(ctx, t.x, T, Ds) && Ds.decls_fin?) &&
+  forall Tc, init :: P(Tc, init) == lookup(t.x, s.m).get ==>
+  forall Ds :: expansion(ctx, t.x, T, Ds) && Ds.decls_fin? ==>
+  forall j:nat :: j<k ==> (
+    (forall Li:nat, S, U :: decl_tp_c(Li, S, U) in Ds.decls ==>
+     exists S', U' :: concrete_type_membership(ctx, t, Li, S', U') &&
+     subtype(ctx, S, S') && subtype(ctx, S', U') && subtype(ctx, U', U)) &&
+    (forall Li:nat, S, U :: decl_tp_a(Li, S, U) in Ds.decls ==>
+     exists S', U' :: abstract_type_membership(ctx, t, Li, S', U') &&
+     subtype(ctx, S, S') && subtype(ctx, S', U') && subtype(ctx, U', U)) &&
+    (forall mi:nat, S, U :: decl_mt(mi, S, U) in Ds.decls ==>
+     exists xi, ti :: def_method_lookup(mi, init) == Some(P(xi, ti)) &&
+     E(U, ti, j, ctx_extend(xi, S, ctx), s, ctx)) &&
+    (forall li:nat, U :: decl_tm(li, U) in Ds.decls ==>
+     def_field_lookup(li, init).Some? &&
+     V(U, def_field_lookup(li, init).get, j, ctx, s))
+  )
+}
+
+predicate E(T: tp, t: tm, k: nat, ctx: context, s: store, ctx_prev: context)
+  requires A(k, ctx_prev, s);
+  requires As(k, ctx, s, ctx_prev);
+  decreases k;
+{
+  k==0 || (
+  forall i:nat, j:nat :: i+j<k ==>
+  forall ctx', s':store :: Xs(ctx', s', k-1, ctx, s, ctx_prev) && A(k-1, ctx', s') ==>
+  forall t', s'':store :: prefix_of(s''.m, s'.m) && mstep(t, s', t', s'', j) && irred(t', s'') ==>
+  forall ctx'' :: Xc(ctx'', k-1, ctx', s'', s') && A(k-1, ctx'', s'') ==>
+  V(T, t', i, ctx'', s'')
+  )
+}
+
+predicate A(k: nat, ctx: context, s: store)
+{
+  dom(ctx.m) == dom(s.m)
+}
+predicate As(k: nat, ctx: context, s: store, ctx_prev: context)
+{
+  prefix_of(ctx.m, ctx_prev.m) && A(k, ctx_prev, s)
+}
+predicate Ac(k: nat, ctx: context, s: store, s_prev: store)
+{
+  prefix_of(s.m, s_prev.m) && A(k, ctx, s_prev)
+}
+predicate Xs(ctx': context, s': store, k: nat, ctx: context, s: store, ctx_prev: context)
+  requires As(k, ctx, s, ctx_prev);
+  decreases k;
+{
+  A(k, ctx', s') && As(k, ctx', s, ctx_prev) && Ac(k, ctx_prev, s', s) && (
+  forall x:nat :: lookup(x, ctx.m).Some? ==>
+    lookup(x, ctx'.m)==Some(lookup(x, ctx.m).get) && V(lookup(x, ctx.m).get, tm_var(x), k, ctx', s'))
+}
+predicate Xc(ctx': context, k: nat, ctx: context, s: store, s_prev: store)
+  requires Ac(k, ctx, s, s_prev);
+{
+  var s_todo := map_complement(s.m, s_prev.m, Empty);
+  var tp_todo := map_fst(s_todo);
+  ctx'.m==build(ctx.m, tp_todo)
+}
+
+predicate R(ctx: context, t: tm, T: tp)
+{
+  forall k: nat ::
+      A(k, Context(Empty), Store(Empty)) &&
+      As(k, ctx, Store(Empty), Context(Empty)) &&
+      E(T, t, k, ctx, Store(Empty), Context(Empty))
+}
+
+// ### Lemmas about logical relations ###
+ghost method lemma_A_monotonic(k: nat, j: nat, ctx: context, s: store)
+  requires A(k, ctx, s);
+  requires j <= k;
+  ensures A(j, ctx, s);
+{
+}
+ghost method lemma_As_monotononic(k: nat, j: nat, ctx: context, s: store, ctx_prev: context)
+  requires As(k, ctx, s, ctx_prev);
+  requires j <= k;
+  ensures As(j, ctx, s, ctx_prev);
+{
+}
+ghost method lemma_Ac_monotononic(k: nat, j: nat, ctx: context, s: store, s_prev: store)
+  requires Ac(k, ctx, s, s_prev);
+  requires j <= k;
+  ensures Ac(j, ctx, s, s_prev);
+{
+}
+ghost method lemma_Xs_monotonic(ctx': context, s': store, k: nat, j: nat, ctx: context, s: store, ctx_prev: context)
+  requires As(k, ctx, s, ctx_prev);
+  requires As(j, ctx, s, ctx_prev);
+  requires Xs(ctx', s', k, ctx, s, ctx_prev);
+  requires j <= k;
+  ensures Xs(ctx', s', j, ctx, s, ctx_prev);
+{
+  forall (x:nat | lookup(x, ctx.m).Some?)
+    ensures lookup(x, ctx'.m)==Some(lookup(x, ctx.m).get) && V(lookup(x, ctx.m).get, tm_var(x), j, ctx', s');
+  {
+    lemma_V_monotonic(lookup(x, ctx.m).get, tm_var(x), k, j, ctx', s');
+  }
+}
+ghost method lemma_Xc_monotonic(ctx': context, k: nat, j: nat, ctx: context, s: store, s_prev: store)
+  requires Ac(k, ctx, s, s_prev);
+  requires Ac(j, ctx, s, s_prev);
+  requires Xc(ctx', k, ctx, s, s_prev);
+  requires j <= k;
+  ensures Xc(ctx', j, ctx, s, s_prev);
+{
+}
+ghost method lemma_V_monotonic(T: tp, t: tm, k: nat, j: nat, ctx: context, s: store)
+  requires A(k, ctx, s);
+  requires A(j, ctx, s);
+  requires V(T, t, k, ctx, s);
+  requires j <= k;
+  ensures V(T, t, j, ctx, s);
+{
+  assume V(T, t, j, ctx, s); // TODO... but really follows from def.
+}
+
+ghost method lemma_V_value(T: tp, t: tm, k: nat, ctx: context, s: store)
+  requires A(k, ctx, s);
+  requires V(T, t, k, ctx, s);
+  ensures value(t);
+{
+}
+ghost method lemma_V_field(T1: tp, t1: tm, l: nat, T: tp, k: nat, j: nat, ctx1: context, s1: store, Tc: tp, init: list<def>, Ds: decls)
+  requires A(k, ctx1, s1);
+  requires V(T1, t1, k, ctx1, s1);
+  requires t1.tm_var?;
+  requires P(Tc, init) == lookup(t1.x, s1.m).get;
+  requires expansion(ctx1, t1.x, T1, Ds) && Ds.decls_fin?;
+  requires decl_tm(l, T) in Ds.decls;
+  requires j<k;
+  ensures def_field_lookup(l, init).Some? && V(T, def_field_lookup(l, init).get, j, ctx1, s1);
+{
+  // TODO...
+  assume def_field_lookup(l, init).Some? && V(T, def_field_lookup(l, init).get, j, ctx1, s1);
+}
+
+ghost method lemma_E(T: tp, t: tm, t': tm, k: nat, j: nat, i: nat,
+  s: store, s': store, s'': store,
+  ctx_prev: context, ctx: context, ctx': context, ctx'': context)
+  requires A(k, ctx_prev, s);
+  requires As(k, ctx, s, ctx_prev);
+  requires E(T, t, k, ctx, s, ctx_prev);
+  requires i+j<k;
+  requires Xs(ctx', s', k-1, ctx, s, ctx_prev) && A(k-1, ctx', s');
+  requires prefix_of(s''.m, s'.m) && mstep(t, s', t', s'', j);
+  requires Xc(ctx'', k-1, ctx', s'', s') && A(k-1, ctx'', s'');
+  ensures irred(t', s'') ==> V(T, t', i, ctx'', s'');
+{
+}
+
+ghost method lemma_Xs_lookup(x: nat, T: tp, ctx': context, s': store, k: nat, ctx: context, s: store, ctx_prev: context)
+  requires As(k, ctx, s, ctx_prev);
+  requires Xs(ctx', s', k, ctx, s, ctx_prev);
+  requires lookup(x, ctx.m) == Some(T);
+  ensures V(T, tm_var(x), k, ctx', s');
+{
+}
+ghost method lemma_unchanged_Xc(ctx': context, k: nat, ctx: context, s: store, s_prev: store)
+  requires Ac(k, ctx, s, s_prev);
+  requires Xc(ctx', k, ctx, s, s_prev);
+  requires s==s_prev;
+  ensures ctx'==ctx;
+{
+}
+ghost method lemma_Xc_unique(ctx2: context, ctx1: context, k: nat, ctx: context, s: store, s_prev: store)
+  requires Ac(k, ctx, s, s_prev);
+  requires Xc(ctx1, k, ctx, s, s_prev);
+  requires Xc(ctx2, k, ctx, s, s_prev);
+  ensures ctx1==ctx2;
+{
+}
+ghost method build_Xc(k: nat, ctx: context, s: store, s_prev: store) returns (ctx': context)
+  requires Ac(k, ctx, s, s_prev);
+  ensures Xc(ctx', k, ctx, s, s_prev);
+  ensures A(k, ctx', s);
+{
+  var s_todo := map_complement(s.m, s_prev.m, Empty);
+  lemma_map_complement__dom(s.m, s_prev.m);
+  assert  dom(s.m)==rev(dom(s_todo))+dom(s_prev.m);
+
+  var tp_todo := map_fst(s_todo);
+  assert  dom(s.m)==rev(dom(tp_todo))+dom(s_prev.m);
+
+  ctx' := Context(build(ctx.m, tp_todo));
+  lemma_build__dom(ctx.m, tp_todo);
+}
+
+ghost method theorem_fundamental_R_var(ctx: context, T: tp, x: nat, k: nat)
+  requires typing(ctx, tm_var(x), T);
+  requires A(k, Context(Empty), Store(Empty));
+  requires As(k, ctx, Store(Empty), Context(Empty));
+  ensures E(T, tm_var(x), k, ctx, Store(Empty), Context(Empty));
+{
+  var ctx_prev := Context(Empty);
+  var s := Store(Empty);
+  var t := tm_var(x);
+
+      assert lookup(x, ctx.m) == Some(T);
+      if (k>0) {
+        forall (
+          i:nat, j:nat,
+          ctx', s':store,
+          t', s'':store,
+          ctx'' |
+          i+j<k &&
+          Xs(ctx', s', k-1, ctx, s, ctx_prev) && A(k-1, ctx', s') &&
+          prefix_of(s''.m, s'.m) && mstep(t, s', t', s'', j) && irred(t', s'') &&
+          Xc(ctx'', k-1, ctx', s'', s') && A(k-1, ctx'', s''))
+          ensures V(T, t', i, ctx'', s'');
+       {
+         assert j==0;
+         assert t'==t;
+         assert s''==s';
+         lemma_unchanged_Xc(ctx'', k-1, ctx', s'', s');
+         assert ctx''==ctx';
+         lemma_Xs_lookup(x, T, ctx', s', k-1, ctx, s, ctx_prev);
+         assert V(T, t', k-1, ctx', s');
+         assert V(T, t', k-1, ctx'', s'');
+         lemma_V_monotonic(T, t', k-1, i, ctx'', s'');
+       }
+      }
+      assert E(T, t, k, ctx, Store(Empty), Context(Empty));
+}
+
+ghost method theorem_fundamental_R_sel(ctx: context, T: tp, T1: tp, t1: tm, l: nat, k: nat)
+  requires typing(ctx, tm_sel(t1, l), T);
+  requires A(k, Context(Empty), Store(Empty));
+  requires As(k, ctx, Store(Empty), Context(Empty));
+
+  requires field_membership(ctx, t1, l, T);
+  requires membership(ctx, t1, l, decl_tm(l, T));
+  requires typing(ctx, t1, T1);
+  requires E(T1, t1, k, ctx, Store(Empty), Context(Empty));
+
+  ensures E(T, tm_sel(t1, l), k, ctx, Store(Empty), Context(Empty));
+{
+  var ctx_prev := Context(Empty);
+  var s := Store(Empty);
+  var t := tm_sel(t1, l);
+
+  if (k>0) {
+    forall (
+      i:nat, j:nat,
+      ctx', s':store,
+      t', s'':store,
+      ctx'' |
+      i+j<k &&
+      Xs(ctx', s', k-1, ctx, s, ctx_prev) && A(k-1, ctx', s') &&
+      prefix_of(s''.m, s'.m) && mstep(t, s', t', s'', j) && irred(t', s'') &&
+      Xc(ctx'', k-1, ctx', s'', s') && A(k-1, ctx'', s''))
+      ensures V(T, t', i, ctx'', s'');
+    {
+      var t1', t1s, t1j := lemma_sel_irred__o_mstep_irred(t1, l, t', s', s'', j);
+      lemma_mstep__prefix(t1, s', t1', t1s, t1j);
+      var t1ctx :=  build_Xc(k-1, ctx', t1s, s');
+      lemma_E(T1, t1, t1', k, t1j, i+j-t1j, s, s', t1s, ctx_prev, ctx, ctx', t1ctx);
+      lemma_V_value(T1, t1', i+j-t1j, t1ctx, t1s);
+
+      lemma_mstep_sel(t1, l, t1', s', t1s, t1j);
+      lemma_mstep_trans'(t, s', tm_sel(t1', l), t1s, t', s'', t1j, j);
+ 
+      forall (Tc, init, Ds |
+        P(Tc, init) == lookup(t1'.x, t1s.m).get &&
+        expansion(t1ctx, t1'.x, T1, Ds) && Ds.decls_fin?)
+        ensures V(T, t', i, ctx'', s'');
+      {
+        lemma_field_mem__expansion_decl(ctx, t1, T1, l, T, t1ctx, t1'.x, Ds);
+        assert exists U :: decl_tm(l, U) in Ds.decls;
+        // How do we relate U and T?
+        // This is fishy because T might have t1 as self, and U might have t1'.
+        // so certainly, they can be !=.
+        assume decl_tm(l, T) in Ds.decls;
+
+        assume j-t1j>0; // fishy: how can we guarantee that?
+        lemma_V_field(T1, t1', l, T, i+j-t1j, i, t1ctx, t1s, Tc, init, Ds);
+        assert V(T, def_field_lookup(l, init).get, i, t1ctx, t1s);
+        lemma_V_value(T, def_field_lookup(l, init).get, i, t1ctx, t1s);
+              
+        lemma_mstep_trans'(tm_sel(t1', l), t1s, def_field_lookup(l, init).get, t1s, t', s'', 1, j-t1j);
+        
+        assert def_field_lookup(l, init).get.tm_var?;
+        lemma_value__irred(def_field_lookup(l, init).get, t1s);
+        assert irred(def_field_lookup(l, init).get, t1s);
+
+        assert t'==def_field_lookup(l, init).get;
+        assert mstep(def_field_lookup(l, init).get, t1s, t', s'', 0);
+        assert s''==t1s;
+        lemma_Xc_unique(ctx'', t1ctx, k-1, ctx', s'', s');
+        assert ctx''==t1ctx;
+
+        assert V(T, def_field_lookup(l, init).get, i, t1ctx, t1s);
+        assert V(T, t', i, ctx'', s'');
+      }
+
+      assert forall Tc, init, Ds :: (
+        P(Tc, init) == lookup(t1'.x, t1s.m).get &&
+        expansion(t1ctx, t1'.x, T1, Ds) && Ds.decls_fin?) ==>
+        V(T, t', i, ctx'', s'');
+      assert exists Tc, init :: P(Tc, init) == lookup(t1'.x, t1s.m).get;
+      assert exists Ds :: expansion(t1ctx, t1'.x, T1, Ds) && Ds.decls_fin?;
+      assert exists Tc, init, Ds :: (
+        P(Tc, init) == lookup(t1'.x, t1s.m).get &&
+        expansion(t1ctx, t1'.x, T1, Ds) && Ds.decls_fin?);
+      assert V(T, t', i, ctx'', s'');
+    }
+  }
+}
+
+ghost method theorem_fundamental_R(ctx: context, t: tm, T: tp)
+  requires typing(ctx, t, T);
+  ensures R(ctx, t, T);
+  decreases t;
+{
+  var ctx_prev := Context(Empty);
+  var s := Store(Empty);
+
+  forall (k: nat)
+    ensures
+      A(k, ctx_prev, s) &&
+      As(k, ctx, s, ctx_prev) &&
+      E(T, t, k, ctx, s, ctx_prev);
+  {
+    lemma_empty_prefix_of_any(ctx.m);
+    assert As(k, ctx, s, ctx_prev);
+
+    match t {
+    case tm_var(x) =>
+      theorem_fundamental_R_var(ctx, T, x, k);
+    case tm_new(y, Tc, init, t1) =>
+      assume E(T, t, k, ctx, Store(Empty), Context(Empty)); // TODO
+    case tm_sel(t1, l) =>
+      assert field_membership(ctx, t1, l, T);
+      assert membership(ctx, t1, l, decl_tm(l, T));
+      assert exists T1 :: typing(ctx, t1, T1);
+      forall (T1 | typing(ctx, t1, T1))
+        ensures E(T, t, k, ctx, s, ctx_prev);
+      {
+        theorem_fundamental_R(ctx, t1, T1);
+        theorem_fundamental_R_sel(ctx, T, T1, t1, l, k);
+      }
+      assert forall T1 :: typing(ctx, t1, T1) ==> E(T, t, k, ctx, s, ctx_prev);
+      assert exists T1 :: typing(ctx, t1, T1);
+      assert E(T, t, k, ctx, s, ctx_prev);
+    case tm_msel(o, m, a) =>
+      assume E(T, t, k, ctx, Store(Empty), Context(Empty)); // TODO
+    }
+  }
+}
+
+// -----------
+// Type-Safety
+// -----------
+predicate type_safety(t: tm, T: tp)
+{
+  typing(Context(Empty), t, T) ==>
+  forall t', s', n:nat :: mstep(t, Store(Empty), t', s', n) ==>
+  value(t') || step(t', s').Some?
+}
+
+ghost method corollary_type_safety(t: tm, T: tp)
+  ensures type_safety(t, T);
+{
+  if (typing(Context(Empty), t, T)) {
+    forall (t', s', n:nat | mstep(t, Store(Empty), t', s', n))
+      ensures value(t') || step(t', s').Some?;
+    {
+      theorem_fundamental_R(Context(Empty), t, T);
+      assert A(n, Context(Empty), Store(Empty));
+      assert As(n, Context(Empty), Store(Empty), Context(Empty));
+      assert E(T, t, n+1, Context(Empty), Store(Empty), Context(Empty));
+      assert Xs(Context(Empty), Store(Empty), n, Context(Empty), Store(Empty), Context(Empty));
+      assert A(n, Context(Empty), Store(Empty));
+      lemma_empty_prefix_of_any(s'.m);
+      assert prefix_of(s'.m, Store(Empty).m);
+      assert mstep(t, Store(Empty), t', s', n);
+      assert Ac(n+1, Context(Empty), s', Store(Empty));
+      var ctx' := build_Xc(n+1, Context(Empty), s', Store(Empty));
+      lemma_E(T, t, t', n+1, n, 0, Store(Empty), Store(Empty), s', Context(Empty), Context(Empty), Context(Empty), ctx');
+    }
+  }
+}
